<?xml version="1.0"?>
<rdf:RDF xmlns:sdmx-measure="http://purl.org/linked-data/sdmx/2009/measure#" xmlns:void="http://rdfs.org/ns/void#" xmlns:dcterms="http://purl.org/dc/terms/" xmlns:qb="http://purl.org/linked-data/cube#" xmlns:rdfindex-org="http://purl.org/weso/rdfindex/organization/" xmlns:foaf="http://xmlns.com/foaf/0.1/" xmlns:sdmx-concept="http://purl.org/linked-data/sdmx/2009/concept#" xmlns:owl="http://www.w3.org/2002/07/owl#" xmlns:xsd="http://www.w3.org/2001/XMLSchema#" xmlns:ci-indicator="http://purl.org/weso/cloudindex/indicator/" xmlns:ci-component="http://purl.org/weso/cloudindex/component/" xmlns:time="http://www.w3.org/2006/time#" xmlns:rdfindex="http://purl.org/weso/rdfindex/ontology/" xmlns:org="http://www.w3.org/ns/org#" xmlns:sdmx-dimension="http://purl.org/linked-data/sdmx/2009/dimension#" xmlns:rdfs="http://www.w3.org/2000/01/rdf-schema#" xmlns:ci-org="http://purl.org/weso/cloudindex/organization/" xmlns:rdf="http://www.w3.org/1999/02/22-rdf-syntax-ns#" xmlns:skos="http://www.w3.org/2004/02/skos/core#" xmlns:rdfindex-project="http://purl.org/weso/rdfindex/project/" xmlns:ci="http://purl.org/weso/cloudindex/" xmlns:ci-people="http://purl.org/weso/cloudindex/people/" xmlns:ci-onto="http://purl.org/weso/cloudindex/ontology/">
	<owl:Ontology rdf:about="http://purl.org/weso/cloudindex/ontology/">
		<owl:versionInfo>0.1</owl:versionInfo>
		<rdfs:label xml:lang="en">Core Cloud Index structure and computation process</rdfs:label>
		<rdfs:comment xml:lang="en">This is the first version of the The CloudIndex taxonomy for representing QoS indicators and modeling an index.</rdfs:comment>
		<dcterms:created rdf:datatype="http://www.w3.org/2001/XMLSchema#date">2012-05-20</dcterms:created>
		<rdfs:seeAlso rdf:resource="http://purl.org/weso/rdfindex/ontology/" />
		<rdfs:seeAlso>
			<rdfindex:Index rdf:about="http://purl.org/weso/cloudindex/index">
				<rdfs:label xml:lang="en">The CloudIndex</rdfs:label>
				<rdfs:comment xml:lang="en">The index of components</rdfs:comment>
				<ci-onto:defined-in rdf:resource="http://csmic.org/wp-content/uploads/2011/09/SMI-Overview-110913_v1F.pdf" />
				<ci-onto:defined-by>
					<org:Organization rdf:about="http://purl.org/weso/cloudindex/organization/CSMIC">
						<rdfs:label xml:lang="en">Service Measurement Index Version 1.0</rdfs:label>
						<rdfs:comment xml:lang="en">It is a common effort for defining a Service Measurement Index</rdfs:comment>
						<org:identifier>CSMIC</org:identifier>
						<foaf:homepage rdf:resource="http://csmic.org/" />
					</org:Organization>
				</ci-onto:defined-by>
				<rdfindex:aggregates>
					<rdf:Description>
						<rdfindex:aggregation-operator rdf:resource="http://purl.org/weso/rdfindex/ontology/OWA" />
						<rdfindex:part-of>
							<rdf:Description>
								<rdfindex:dataset>
									<rdfindex:Component rdf:about="http://purl.org/weso/cloudindex/component/Accountability">
										<rdfs:label xml:lang="en">Accountability</rdfs:label>
										<rdfs:comment xml:lang="en">This component is used to measure the properties related to the service provider
organization. These properties may be independent of the service being provided.</rdfs:comment>
										<ci-onto:defined-in rdf:resource="http://csmic.org/wp-content/uploads/2011/09/SMI-Overview-110913_v1F.pdf" />
										<ci-onto:defined-by rdf:resource="http://purl.org/weso/cloudindex/organization/CSMIC" />
										<rdfindex:weight rdf:datatype="http://www.w3.org/2001/XMLSchema#double">1</rdfindex:weight>
										<rdfindex:aggregates>
											<rdf:Description>
												<rdfindex:aggregation-operator rdf:resource="http://purl.org/weso/rdfindex/ontology/OWA" />
												<rdfindex:part-of>
													<rdf:Description>
														<rdfindex:dataset>
															<ci-onto:KPIIndicator rdf:about="http://purl.org/weso/cloudindex/indicator/Auditability">
																<rdfs:label xml:lang="en">Auditability</rdfs:label>
																<rdfs:comment xml:lang="en">The ability of a client to verify that the service provider is adhering to the standards, processes, and policies that they follow.</rdfs:comment>
																<skos:definition xml:lang="en">The ability of a client to verify that the service provider is adhering to the standards, processes, and policies that they follow.</skos:definition>
																<ci-onto:defined-in rdf:resource="http://csmic.org/wp-content/uploads/2011/09/SMI-Overview-110913_v1F.pdf" />
																<ci-onto:defined-by rdf:resource="http://purl.org/weso/cloudindex/organization/CSMIC" />
																<ci-onto:weight rdf:datatype="http://www.w3.org/2001/XMLSchema#double">1.0</ci-onto:weight>
																<ci-onto:pref-value rdf:resource="http://purl.org/weso/cloudindex/ontology/High" />
																<skos:notation>Auditability</skos:notation>
																<time:intervalStarts rdf:datatype="http://www.w3.org/2001/XMLSchema#int">2013</time:intervalStarts>
																<time:intervalFinishes rdf:datatype="http://www.w3.org/2001/XMLSchema#int">2013</time:intervalFinishes>
																<skos:broader rdf:resource="http://purl.org/weso/cloudindex/component/Accountability" />
															</ci-onto:KPIIndicator>
														</rdfindex:dataset>
														<rdfindex:weight rdf:datatype="http://www.w3.org/2001/XMLSchema#double">0.06</rdfindex:weight>
													</rdf:Description>
												</rdfindex:part-of>
												<rdfindex:part-of>
													<rdf:Description>
														<rdfindex:dataset>
															<ci-onto:KPIIndicator rdf:about="http://purl.org/weso/cloudindex/indicator/Compliance">
																<rdfs:label xml:lang="en">Compliance</rdfs:label>
																<rdfs:comment xml:lang="en">Standards, processes, and policies committed to by the service provider are followed.</rdfs:comment>
																<skos:definition xml:lang="en">Standards, processes, and policies committed to by the service provider are followed.</skos:definition>
																<ci-onto:defined-in rdf:resource="http://csmic.org/wp-content/uploads/2011/09/SMI-Overview-110913_v1F.pdf" />
																<ci-onto:defined-by rdf:resource="http://purl.org/weso/cloudindex/organization/CSMIC" />
																<ci-onto:weight rdf:datatype="http://www.w3.org/2001/XMLSchema#double">1.0</ci-onto:weight>
																<ci-onto:pref-value rdf:resource="http://purl.org/weso/cloudindex/ontology/High" />
																<skos:notation>Compliance</skos:notation>
																<time:intervalStarts rdf:datatype="http://www.w3.org/2001/XMLSchema#int">2013</time:intervalStarts>
																<time:intervalFinishes rdf:datatype="http://www.w3.org/2001/XMLSchema#int">2013</time:intervalFinishes>
																<skos:broader rdf:resource="http://purl.org/weso/cloudindex/component/Accountability" />
															</ci-onto:KPIIndicator>
														</rdfindex:dataset>
														<rdfindex:weight rdf:datatype="http://www.w3.org/2001/XMLSchema#double">0.06</rdfindex:weight>
													</rdf:Description>
												</rdfindex:part-of>
												<rdfindex:part-of>
													<rdf:Description>
														<rdfindex:dataset>
															<ci-onto:KPIIndicator rdf:about="http://purl.org/weso/cloudindex/indicator/ContractingExperience">
																<rdfs:label xml:lang="en">Contracting Experience</rdfs:label>
																<rdfs:comment xml:lang="en">Indicators of client effort and satisfaction with the process of entering into the agreements required to use a service.</rdfs:comment>
																<skos:definition xml:lang="en">Indicators of client effort and satisfaction with the process of entering into the agreements required to use a service.</skos:definition>
																<ci-onto:defined-in rdf:resource="http://csmic.org/wp-content/uploads/2011/09/SMI-Overview-110913_v1F.pdf" />
																<ci-onto:defined-by rdf:resource="http://purl.org/weso/cloudindex/organization/CSMIC" />
																<ci-onto:weight rdf:datatype="http://www.w3.org/2001/XMLSchema#double">1.0</ci-onto:weight>
																<ci-onto:pref-value rdf:resource="http://purl.org/weso/cloudindex/ontology/High" />
																<skos:notation>ContractingExperience</skos:notation>
																<time:intervalStarts rdf:datatype="http://www.w3.org/2001/XMLSchema#int">2013</time:intervalStarts>
																<time:intervalFinishes rdf:datatype="http://www.w3.org/2001/XMLSchema#int">2013</time:intervalFinishes>
																<skos:broader rdf:resource="http://purl.org/weso/cloudindex/component/Accountability" />
															</ci-onto:KPIIndicator>
														</rdfindex:dataset>
														<rdfindex:weight rdf:datatype="http://www.w3.org/2001/XMLSchema#double">0.06</rdfindex:weight>
													</rdf:Description>
												</rdfindex:part-of>
												<rdfindex:part-of>
													<rdf:Description>
														<rdfindex:dataset>
															<ci-onto:KPIIndicator rdf:about="http://purl.org/weso/cloudindex/indicator/DataOwnership">
																<rdfs:label xml:lang="en">Data Ownership</rdfs:label>
																<rdfs:comment xml:lang="en">The Level of rights a client has over client data associated with a service.</rdfs:comment>
																<skos:definition xml:lang="en">The Level of rights a client has over client data associated with a service.</skos:definition>
																<ci-onto:defined-in rdf:resource="http://csmic.org/wp-content/uploads/2011/09/SMI-Overview-110913_v1F.pdf" />
																<ci-onto:defined-by rdf:resource="http://purl.org/weso/cloudindex/organization/CSMIC" />
																<ci-onto:weight rdf:datatype="http://www.w3.org/2001/XMLSchema#double">1.0</ci-onto:weight>
																<ci-onto:pref-value rdf:resource="http://purl.org/weso/cloudindex/ontology/High" />
																<skos:notation>DataOwnership</skos:notation>
																<time:intervalStarts rdf:datatype="http://www.w3.org/2001/XMLSchema#int">2013</time:intervalStarts>
																<time:intervalFinishes rdf:datatype="http://www.w3.org/2001/XMLSchema#int">2013</time:intervalFinishes>
																<skos:broader rdf:resource="http://purl.org/weso/cloudindex/component/Accountability" />
															</ci-onto:KPIIndicator>
														</rdfindex:dataset>
														<rdfindex:weight rdf:datatype="http://www.w3.org/2001/XMLSchema#double">0.06</rdfindex:weight>
													</rdf:Description>
												</rdfindex:part-of>
												<rdfindex:part-of>
													<rdf:Description>
														<rdfindex:dataset>
															<ci-onto:KPIIndicator rdf:about="http://purl.org/weso/cloudindex/indicator/EaseDoingBusiness">
																<rdfs:label xml:lang="en">Ease of Doing Business</rdfs:label>
																<rdfs:comment xml:lang="en">Client satisfaction with the ability to do business with a service provider.</rdfs:comment>
																<skos:definition xml:lang="en">Client satisfaction with the ability to do business with a service provider.</skos:definition>
																<ci-onto:defined-in rdf:resource="http://csmic.org/wp-content/uploads/2011/09/SMI-Overview-110913_v1F.pdf" />
																<ci-onto:defined-by rdf:resource="http://purl.org/weso/cloudindex/organization/CSMIC" />
																<ci-onto:weight rdf:datatype="http://www.w3.org/2001/XMLSchema#double">1.0</ci-onto:weight>
																<ci-onto:pref-value rdf:resource="http://purl.org/weso/cloudindex/ontology/High" />
																<skos:notation>EaseDoingBusiness</skos:notation>
																<time:intervalStarts rdf:datatype="http://www.w3.org/2001/XMLSchema#int">2013</time:intervalStarts>
																<time:intervalFinishes rdf:datatype="http://www.w3.org/2001/XMLSchema#int">2013</time:intervalFinishes>
																<skos:broader rdf:resource="http://purl.org/weso/cloudindex/component/Accountability" />
															</ci-onto:KPIIndicator>
														</rdfindex:dataset>
														<rdfindex:weight rdf:datatype="http://www.w3.org/2001/XMLSchema#double">0.06</rdfindex:weight>
													</rdf:Description>
												</rdfindex:part-of>
												<rdfindex:part-of>
													<rdf:Description>
														<rdfindex:dataset>
															<ci-onto:KPIIndicator rdf:about="http://purl.org/weso/cloudindex/indicator/Governance">
																<rdfs:label xml:lang="en">Ease of Doing Business</rdfs:label>
																<rdfs:comment xml:lang="en">The processes used by the service provider to manage client expectations, issues and service performance.</rdfs:comment>
																<skos:definition xml:lang="en">The processes used by the service provider to manage client expectations, issues and service performance.</skos:definition>
																<ci-onto:defined-in rdf:resource="http://csmic.org/wp-content/uploads/2011/09/SMI-Overview-110913_v1F.pdf" />
																<ci-onto:defined-by rdf:resource="http://purl.org/weso/cloudindex/organization/CSMIC" />
																<ci-onto:weight rdf:datatype="http://www.w3.org/2001/XMLSchema#double">1.0</ci-onto:weight>
																<ci-onto:pref-value rdf:resource="http://purl.org/weso/cloudindex/ontology/High" />
																<skos:notation>Governance</skos:notation>
																<time:intervalStarts rdf:datatype="http://www.w3.org/2001/XMLSchema#int">2013</time:intervalStarts>
																<time:intervalFinishes rdf:datatype="http://www.w3.org/2001/XMLSchema#int">2013</time:intervalFinishes>
																<skos:broader rdf:resource="http://purl.org/weso/cloudindex/component/Accountability" />
															</ci-onto:KPIIndicator>
														</rdfindex:dataset>
														<rdfindex:weight rdf:datatype="http://www.w3.org/2001/XMLSchema#double">0.06</rdfindex:weight>
													</rdf:Description>
												</rdfindex:part-of>
												<rdfindex:part-of>
													<rdf:Description>
														<rdfindex:dataset>
															<ci-onto:KPIIndicator rdf:about="http://purl.org/weso/cloudindex/indicator/Ownership">
																<rdfs:label xml:lang="en">Ownership</rdfs:label>
																<rdfs:comment xml:lang="en">The level of rights a client has over software licenses, intellectual property and data associated with a service.</rdfs:comment>
																<skos:definition xml:lang="en">The level of rights a client has over software licenses, intellectual property and data associated with a service.</skos:definition>
																<ci-onto:defined-in rdf:resource="http://csmic.org/wp-content/uploads/2011/09/SMI-Overview-110913_v1F.pdf" />
																<ci-onto:defined-by rdf:resource="http://purl.org/weso/cloudindex/organization/CSMIC" />
																<ci-onto:weight rdf:datatype="http://www.w3.org/2001/XMLSchema#double">1.0</ci-onto:weight>
																<ci-onto:pref-value rdf:resource="http://purl.org/weso/cloudindex/ontology/High" />
																<skos:notation>Ownership</skos:notation>
																<time:intervalStarts rdf:datatype="http://www.w3.org/2001/XMLSchema#int">2013</time:intervalStarts>
																<time:intervalFinishes rdf:datatype="http://www.w3.org/2001/XMLSchema#int">2013</time:intervalFinishes>
																<skos:broader rdf:resource="http://purl.org/weso/cloudindex/component/Accountability" />
															</ci-onto:KPIIndicator>
														</rdfindex:dataset>
														<rdfindex:weight rdf:datatype="http://www.w3.org/2001/XMLSchema#double">0.06</rdfindex:weight>
													</rdf:Description>
												</rdfindex:part-of>
												<rdfindex:part-of>
													<rdf:Description>
														<rdfindex:dataset>
															<ci-onto:KPIIndicator rdf:about="http://purl.org/weso/cloudindex/indicator/ProviderStability">
																<rdfs:label xml:lang="en">Provider business stability</rdfs:label>
																<rdfs:comment xml:lang="en">The likelihood that the service provider will continue to exist throughout the contracted term.</rdfs:comment>
																<skos:definition xml:lang="en">The likelihood that the service provider will continue to exist throughout the contracted term.</skos:definition>
																<ci-onto:defined-in rdf:resource="http://csmic.org/wp-content/uploads/2011/09/SMI-Overview-110913_v1F.pdf" />
																<ci-onto:defined-by rdf:resource="http://purl.org/weso/cloudindex/organization/CSMIC" />
																<ci-onto:weight rdf:datatype="http://www.w3.org/2001/XMLSchema#double">1.0</ci-onto:weight>
																<ci-onto:pref-value rdf:resource="http://purl.org/weso/cloudindex/ontology/High" />
																<skos:notation>ProviderStability</skos:notation>
																<time:intervalStarts rdf:datatype="http://www.w3.org/2001/XMLSchema#int">2013</time:intervalStarts>
																<time:intervalFinishes rdf:datatype="http://www.w3.org/2001/XMLSchema#int">2013</time:intervalFinishes>
																<skos:broader rdf:resource="http://purl.org/weso/cloudindex/component/Accountability" />
															</ci-onto:KPIIndicator>
														</rdfindex:dataset>
														<rdfindex:weight rdf:datatype="http://www.w3.org/2001/XMLSchema#double">0.06</rdfindex:weight>
													</rdf:Description>
												</rdfindex:part-of>
												<rdfindex:part-of>
													<rdf:Description>
														<rdfindex:dataset>
															<ci-onto:KPIIndicator rdf:about="http://purl.org/weso/cloudindex/indicator/ProviderCertifications">
																<rdfs:label xml:lang="en">Provider Certifications</rdfs:label>
																<rdfs:comment xml:lang="en">The service provider maintains current certifications for standards relevant to their clients' requirements.</rdfs:comment>
																<skos:definition xml:lang="en">The service provider maintains current certifications for standards relevant to their clients' requirements.</skos:definition>
																<ci-onto:defined-in rdf:resource="http://csmic.org/wp-content/uploads/2011/09/SMI-Overview-110913_v1F.pdf" />
																<ci-onto:defined-by rdf:resource="http://purl.org/weso/cloudindex/organization/CSMIC" />
																<ci-onto:weight rdf:datatype="http://www.w3.org/2001/XMLSchema#double">1.0</ci-onto:weight>
																<ci-onto:pref-value rdf:resource="http://purl.org/weso/cloudindex/ontology/High" />
																<skos:notation>ProviderCertifications</skos:notation>
																<time:intervalStarts rdf:datatype="http://www.w3.org/2001/XMLSchema#int">2013</time:intervalStarts>
																<time:intervalFinishes rdf:datatype="http://www.w3.org/2001/XMLSchema#int">2013</time:intervalFinishes>
																<skos:broader rdf:resource="http://purl.org/weso/cloudindex/component/Accountability" />
															</ci-onto:KPIIndicator>
														</rdfindex:dataset>
														<rdfindex:weight rdf:datatype="http://www.w3.org/2001/XMLSchema#double">0.06</rdfindex:weight>
													</rdf:Description>
												</rdfindex:part-of>
												<rdfindex:part-of>
													<rdf:Description>
														<rdfindex:dataset>
															<ci-onto:KPIIndicator rdf:about="http://purl.org/weso/cloudindex/indicator/ProviderSLAVerification">
																<rdfs:label xml:lang="en">Provider Contract/SLA Verification</rdfs:label>
																<rdfs:comment xml:lang="en">The service provider makes available to clients SLAs adequate to manage the service and mitigate risks of service failure.</rdfs:comment>
																<skos:definition xml:lang="en">The service provider makes available to clients SLAs adequate to manage the service and mitigate risks of service failure.</skos:definition>
																<ci-onto:defined-in rdf:resource="http://csmic.org/wp-content/uploads/2011/09/SMI-Overview-110913_v1F.pdf" />
																<ci-onto:defined-by rdf:resource="http://purl.org/weso/cloudindex/organization/CSMIC" />
																<ci-onto:weight rdf:datatype="http://www.w3.org/2001/XMLSchema#double">1.0</ci-onto:weight>
																<ci-onto:pref-value rdf:resource="http://purl.org/weso/cloudindex/ontology/High" />
																<skos:notation>ProviderSLAVerification</skos:notation>
																<time:intervalStarts rdf:datatype="http://www.w3.org/2001/XMLSchema#int">2013</time:intervalStarts>
																<time:intervalFinishes rdf:datatype="http://www.w3.org/2001/XMLSchema#int">2013</time:intervalFinishes>
																<skos:broader rdf:resource="http://purl.org/weso/cloudindex/component/Accountability" />
															</ci-onto:KPIIndicator>
														</rdfindex:dataset>
														<rdfindex:weight rdf:datatype="http://www.w3.org/2001/XMLSchema#double">0.06</rdfindex:weight>
													</rdf:Description>
												</rdfindex:part-of>
												<rdfindex:part-of>
													<rdf:Description>
														<rdfindex:dataset>
															<ci-onto:KPIIndicator rdf:about="http://purl.org/weso/cloudindex/indicator/ProviderEthics">
																<rdfs:label xml:lang="en">Provider Ethicality</rdfs:label>
																<rdfs:comment xml:lang="en">Ethicality refers to the manner in which the service provider conducts business; it includes business practices and ethics outside the scope of regulatory compliance. Ethicality includes fair practices with suppliers, customers, and employees.</rdfs:comment>
																<skos:definition xml:lang="en">Ethicality refers to the manner in which the service provider conducts business; it includes business practices and ethics outside the scope of regulatory compliance. Ethicality includes fair practices with suppliers, customers, and employees.</skos:definition>
																<ci-onto:defined-in rdf:resource="http://csmic.org/wp-content/uploads/2011/09/SMI-Overview-110913_v1F.pdf" />
																<ci-onto:defined-by rdf:resource="http://purl.org/weso/cloudindex/organization/CSMIC" />
																<ci-onto:weight rdf:datatype="http://www.w3.org/2001/XMLSchema#double">1.0</ci-onto:weight>
																<ci-onto:pref-value rdf:resource="http://purl.org/weso/cloudindex/ontology/High" />
																<skos:notation>ProviderEthics</skos:notation>
																<time:intervalStarts rdf:datatype="http://www.w3.org/2001/XMLSchema#int">2013</time:intervalStarts>
																<time:intervalFinishes rdf:datatype="http://www.w3.org/2001/XMLSchema#int">2013</time:intervalFinishes>
																<skos:broader rdf:resource="http://purl.org/weso/cloudindex/component/Accountability" />
															</ci-onto:KPIIndicator>
														</rdfindex:dataset>
														<rdfindex:weight rdf:datatype="http://www.w3.org/2001/XMLSchema#double">0.06</rdfindex:weight>
													</rdf:Description>
												</rdfindex:part-of>
												<rdfindex:part-of>
													<rdf:Description>
														<rdfindex:dataset>
															<ci-onto:KPIIndicator rdf:about="http://purl.org/weso/cloudindex/indicator/ProviderPersonnelRequirements">
																<rdfs:label xml:lang="en">Provider Personnel Requirements</rdfs:label>
																<rdfs:comment xml:lang="en">The extent to which service provider personnel have the skills, experience, education, and certifications required to effectively deliver a service.</rdfs:comment>
																<skos:definition xml:lang="en">The extent to which service provider personnel have the skills, experience, education, and certifications required to effectively deliver a service.</skos:definition>
																<ci-onto:defined-in rdf:resource="http://csmic.org/wp-content/uploads/2011/09/SMI-Overview-110913_v1F.pdf" />
																<ci-onto:defined-by rdf:resource="http://purl.org/weso/cloudindex/organization/CSMIC" />
																<ci-onto:weight rdf:datatype="http://www.w3.org/2001/XMLSchema#double">1.0</ci-onto:weight>
																<ci-onto:pref-value rdf:resource="http://purl.org/weso/cloudindex/ontology/High" />
																<skos:notation>ProviderPersonnelRequirements</skos:notation>
																<time:intervalStarts rdf:datatype="http://www.w3.org/2001/XMLSchema#int">2013</time:intervalStarts>
																<time:intervalFinishes rdf:datatype="http://www.w3.org/2001/XMLSchema#int">2013</time:intervalFinishes>
																<skos:broader rdf:resource="http://purl.org/weso/cloudindex/component/Accountability" />
															</ci-onto:KPIIndicator>
														</rdfindex:dataset>
														<rdfindex:weight rdf:datatype="http://www.w3.org/2001/XMLSchema#double">0.06</rdfindex:weight>
													</rdf:Description>
												</rdfindex:part-of>
												<rdfindex:part-of>
													<rdf:Description>
														<rdfindex:dataset>
															<ci-onto:KPIIndicator rdf:about="http://purl.org/weso/cloudindex/indicator/ProviderSupplyChain">
																<rdfs:label xml:lang="en">Provider Supply Chain</rdfs:label>
																<rdfs:comment xml:lang="en">The service provider ensures that any SLAs that must be supported by its suppliers are supported.</rdfs:comment>
																<skos:definition xml:lang="en">The service provider ensures that any SLAs that must be supported by its suppliers are supported.</skos:definition>
																<ci-onto:defined-in rdf:resource="http://csmic.org/wp-content/uploads/2011/09/SMI-Overview-110913_v1F.pdf" />
																<ci-onto:defined-by rdf:resource="http://purl.org/weso/cloudindex/organization/CSMIC" />
																<ci-onto:weight rdf:datatype="http://www.w3.org/2001/XMLSchema#double">1.0</ci-onto:weight>
																<ci-onto:pref-value rdf:resource="http://purl.org/weso/cloudindex/ontology/High" />
																<skos:notation>ProviderSupplyChain</skos:notation>
																<time:intervalStarts rdf:datatype="http://www.w3.org/2001/XMLSchema#int">2013</time:intervalStarts>
																<time:intervalFinishes rdf:datatype="http://www.w3.org/2001/XMLSchema#int">2013</time:intervalFinishes>
																<skos:broader rdf:resource="http://purl.org/weso/cloudindex/component/Accountability" />
															</ci-onto:KPIIndicator>
														</rdfindex:dataset>
														<rdfindex:weight rdf:datatype="http://www.w3.org/2001/XMLSchema#double">0.06</rdfindex:weight>
													</rdf:Description>
												</rdfindex:part-of>
												<rdfindex:part-of>
													<rdf:Description>
														<rdfindex:dataset>
															<ci-onto:KPIIndicator rdf:about="http://purl.org/weso/cloudindex/indicator/ProviderSecurityCapabilities">
																<rdfs:label xml:lang="en">Security Capabilities</rdfs:label>
																<rdfs:comment xml:lang="en">The capabilities of service providers to ensure application, data, and infrastructure securiy based on the security requirements of the client.</rdfs:comment>
																<skos:definition xml:lang="en">The capabilities of service providers to ensure application, data, and infrastructure securiy based on the security requirements of the client.</skos:definition>
																<ci-onto:defined-in rdf:resource="http://csmic.org/wp-content/uploads/2011/09/SMI-Overview-110913_v1F.pdf" />
																<ci-onto:defined-by rdf:resource="http://purl.org/weso/cloudindex/organization/CSMIC" />
																<ci-onto:weight rdf:datatype="http://www.w3.org/2001/XMLSchema#double">1.0</ci-onto:weight>
																<ci-onto:pref-value rdf:resource="http://purl.org/weso/cloudindex/ontology/High" />
																<skos:notation>ProviderSecurityCapabilities</skos:notation>
																<time:intervalStarts rdf:datatype="http://www.w3.org/2001/XMLSchema#int">2013</time:intervalStarts>
																<time:intervalFinishes rdf:datatype="http://www.w3.org/2001/XMLSchema#int">2013</time:intervalFinishes>
																<skos:broader rdf:resource="http://purl.org/weso/cloudindex/component/Accountability" />
															</ci-onto:KPIIndicator>
														</rdfindex:dataset>
														<rdfindex:weight rdf:datatype="http://www.w3.org/2001/XMLSchema#double">0.06</rdfindex:weight>
													</rdf:Description>
												</rdfindex:part-of>
												<rdfindex:part-of>
													<rdf:Description>
														<rdfindex:dataset>
															<ci-onto:KPIIndicator rdf:about="http://purl.org/weso/cloudindex/indicator/Sustainability">
																<rdfs:label xml:lang="en">Sustainability</rdfs:label>
																<rdfs:comment xml:lang="en">The impact on the economy, society and the environment of the service provider.</rdfs:comment>
																<skos:definition xml:lang="en">The impact on the economy, society and the environment of the service provider.</skos:definition>
																<ci-onto:defined-in rdf:resource="http://csmic.org/wp-content/uploads/2011/09/SMI-Overview-110913_v1F.pdf" />
																<ci-onto:defined-by rdf:resource="http://purl.org/weso/cloudindex/organization/CSMIC" />
																<ci-onto:weight rdf:datatype="http://www.w3.org/2001/XMLSchema#double">1.0</ci-onto:weight>
																<ci-onto:pref-value rdf:resource="http://purl.org/weso/cloudindex/ontology/High" />
																<skos:notation>Sustainability</skos:notation>
																<time:intervalStarts rdf:datatype="http://www.w3.org/2001/XMLSchema#int">2013</time:intervalStarts>
																<time:intervalFinishes rdf:datatype="http://www.w3.org/2001/XMLSchema#int">2013</time:intervalFinishes>
																<skos:broader rdf:resource="http://purl.org/weso/cloudindex/component/Accountability" />
															</ci-onto:KPIIndicator>
														</rdfindex:dataset>
														<rdfindex:weight rdf:datatype="http://www.w3.org/2001/XMLSchema#double">0.06</rdfindex:weight>
													</rdf:Description>
												</rdfindex:part-of>
											</rdf:Description>
										</rdfindex:aggregates>
										<qb:structure rdf:resource="http://purl.org/weso/cloudindex/AccountabilityDSD" />
										<skos:narrower rdf:resource="http://purl.org/weso/cloudindex/indicator/Auditability" />
										<skos:narrower rdf:resource="http://purl.org/weso/cloudindex/indicator/Compliance" />
										<skos:narrower rdf:resource="http://purl.org/weso/cloudindex/indicator/ContractingExperience" />
										<skos:narrower rdf:resource="http://purl.org/weso/cloudindex/indicator/DataOwnership" />
										<skos:narrower rdf:resource="http://purl.org/weso/cloudindex/indicator/EaseDoingBusiness" />
										<skos:narrower rdf:resource="http://purl.org/weso/cloudindex/indicator/Governance" />
										<skos:narrower rdf:resource="http://purl.org/weso/cloudindex/indicator/Ownership" />
										<skos:narrower rdf:resource="http://purl.org/weso/cloudindex/indicator/ProviderStability" />
										<skos:narrower rdf:resource="http://purl.org/weso/cloudindex/indicator/ProviderCertifications" />
										<skos:narrower rdf:resource="http://purl.org/weso/cloudindex/indicator/ProviderSLAVerification" />
										<skos:narrower rdf:resource="http://purl.org/weso/cloudindex/indicator/ProviderEthics" />
										<skos:narrower rdf:resource="http://purl.org/weso/cloudindex/indicator/ProviderPersonnelRequirements" />
										<skos:narrower rdf:resource="http://purl.org/weso/cloudindex/indicator/ProviderSupplyChain" />
										<skos:narrower rdf:resource="http://purl.org/weso/cloudindex/indicator/ProviderSecurityCapabilities" />
										<skos:narrower rdf:resource="http://purl.org/weso/cloudindex/indicator/Sustainability" />
									</rdfindex:Component>
								</rdfindex:dataset>
								<rdfindex:weight rdf:datatype="http://www.w3.org/2001/XMLSchema#double">0.14</rdfindex:weight>
							</rdf:Description>
						</rdfindex:part-of>
						<rdfindex:part-of>
							<rdf:Description>
								<rdfindex:dataset>
									<rdfindex:Component rdf:about="http://purl.org/weso/cloudindex/component/Agility">
										<rdfs:label xml:lang="en">Agility</rdfs:label>
										<rdfs:comment xml:lang="en">Indicates the impact of a service upon a client's ability to change direction, strategy, or tactics quickly
and with minimal disruption.</rdfs:comment>
										<ci-onto:defined-in rdf:resource="http://csmic.org/wp-content/uploads/2011/09/SMI-Overview-110913_v1F.pdf" />
										<ci-onto:defined-by rdf:resource="http://purl.org/weso/cloudindex/organization/CSMIC" />
										<ci-onto:weight rdf:datatype="http://www.w3.org/2001/XMLSchema#double">1</ci-onto:weight>
										<rdfindex:aggregates>
											<rdf:Description>
												<rdfindex:aggregation-operator rdf:resource="http://purl.org/weso/rdfindex/ontology/OWA" />
												<rdfindex:part-of>
													<rdf:Description>
														<rdfindex:dataset>
															<ci-onto:KPIIndicator rdf:about="http://purl.org/weso/cloudindex/indicator/Adaptability">
																<rdfs:label xml:lang="en">Adaptability</rdfs:label>
																<rdfs:comment xml:lang="en">The ability of the service provider to adjust to changes in client requirements.</rdfs:comment>
																<skos:definition xml:lang="en">The ability of the service provider to adjust to changes in client requirements.</skos:definition>
																<ci-onto:defined-in rdf:resource="http://csmic.org/wp-content/uploads/2011/09/SMI-Overview-110913_v1F.pdf" />
																<ci-onto:defined-by rdf:resource="http://purl.org/weso/cloudindex/organization/CSMIC" />
																<ci-onto:weight rdf:datatype="http://www.w3.org/2001/XMLSchema#double">1.0</ci-onto:weight>
																<ci-onto:pref-value rdf:resource="http://purl.org/weso/cloudindex/ontology/High" />
																<skos:notation>Adaptability</skos:notation>
																<time:intervalStarts rdf:datatype="http://www.w3.org/2001/XMLSchema#int">2013</time:intervalStarts>
																<time:intervalFinishes rdf:datatype="http://www.w3.org/2001/XMLSchema#int">2013</time:intervalFinishes>
																<skos:broader rdf:resource="http://purl.org/weso/cloudindex/component/Agility" />
															</ci-onto:KPIIndicator>
														</rdfindex:dataset>
														<rdfindex:weight rdf:datatype="http://www.w3.org/2001/XMLSchema#double">0.14</rdfindex:weight>
													</rdf:Description>
												</rdfindex:part-of>
												<rdfindex:part-of>
													<rdf:Description>
														<rdfindex:dataset>
															<ci-onto:KPIIndicator rdf:about="http://purl.org/weso/cloudindex/indicator/Capacity">
																<rdfs:label xml:lang="en">Capacity</rdfs:label>
																<rdfs:comment xml:lang="en">The maximum amount of a service that a service provider can deliver while meeting agreed SLAs.</rdfs:comment>
																<skos:definition xml:lang="en">The maximum amount of a service that a service provider can deliver while meeting agreed SLAs.</skos:definition>
																<ci-onto:defined-in rdf:resource="http://csmic.org/wp-content/uploads/2011/09/SMI-Overview-110913_v1F.pdf" />
																<ci-onto:defined-by rdf:resource="http://purl.org/weso/cloudindex/organization/CSMIC" />
																<ci-onto:weight rdf:datatype="http://www.w3.org/2001/XMLSchema#double">1.0</ci-onto:weight>
																<ci-onto:pref-value rdf:resource="http://purl.org/weso/cloudindex/ontology/High" />
																<skos:notation>Capacity</skos:notation>
																<time:intervalStarts rdf:datatype="http://www.w3.org/2001/XMLSchema#int">2013</time:intervalStarts>
																<time:intervalFinishes rdf:datatype="http://www.w3.org/2001/XMLSchema#int">2013</time:intervalFinishes>
																<skos:broader rdf:resource="http://purl.org/weso/cloudindex/component/Agility" />
															</ci-onto:KPIIndicator>
														</rdfindex:dataset>
														<rdfindex:weight rdf:datatype="http://www.w3.org/2001/XMLSchema#double">0.14</rdfindex:weight>
													</rdf:Description>
												</rdfindex:part-of>
												<rdfindex:part-of>
													<rdf:Description>
														<rdfindex:dataset>
															<ci-onto:KPIIndicator rdf:about="http://purl.org/weso/cloudindex/indicator/Elasticity">
																<rdfs:label xml:lang="en">Elasticity</rdfs:label>
																<rdfs:comment xml:lang="en">The ability of a service to adjust its resource consumption to meet demand.</rdfs:comment>
																<skos:definition xml:lang="en">The ability of a service to adjust its resource consumption to meet demand.</skos:definition>
																<ci-onto:defined-in rdf:resource="http://csmic.org/wp-content/uploads/2011/09/SMI-Overview-110913_v1F.pdf" />
																<ci-onto:defined-by rdf:resource="http://purl.org/weso/cloudindex/organization/CSMIC" />
																<ci-onto:weight rdf:datatype="http://www.w3.org/2001/XMLSchema#double">1.0</ci-onto:weight>
																<ci-onto:pref-value rdf:resource="http://purl.org/weso/cloudindex/ontology/High" />
																<skos:notation>Elasticity</skos:notation>
																<time:intervalStarts rdf:datatype="http://www.w3.org/2001/XMLSchema#int">2013</time:intervalStarts>
																<time:intervalFinishes rdf:datatype="http://www.w3.org/2001/XMLSchema#int">2013</time:intervalFinishes>
																<skos:broader rdf:resource="http://purl.org/weso/cloudindex/component/Agility" />
															</ci-onto:KPIIndicator>
														</rdfindex:dataset>
														<rdfindex:weight rdf:datatype="http://www.w3.org/2001/XMLSchema#double">0.14</rdfindex:weight>
													</rdf:Description>
												</rdfindex:part-of>
												<rdfindex:part-of>
													<rdf:Description>
														<rdfindex:dataset>
															<ci-onto:KPIIndicator rdf:about="http://purl.org/weso/cloudindex/indicator/Extensibility">
																<rdfs:label xml:lang="en">Extensibility</rdfs:label>
																<rdfs:comment xml:lang="en">The ability to add new features or services to existing services.</rdfs:comment>
																<skos:definition xml:lang="en">The ability to add new features or services to existing services.</skos:definition>
																<ci-onto:defined-in rdf:resource="http://csmic.org/wp-content/uploads/2011/09/SMI-Overview-110913_v1F.pdf" />
																<ci-onto:defined-by rdf:resource="http://purl.org/weso/cloudindex/organization/CSMIC" />
																<ci-onto:weight rdf:datatype="http://www.w3.org/2001/XMLSchema#double">1.0</ci-onto:weight>
																<ci-onto:pref-value rdf:resource="http://purl.org/weso/cloudindex/ontology/High" />
																<skos:notation>Extensibility</skos:notation>
																<time:intervalStarts rdf:datatype="http://www.w3.org/2001/XMLSchema#int">2013</time:intervalStarts>
																<time:intervalFinishes rdf:datatype="http://www.w3.org/2001/XMLSchema#int">2013</time:intervalFinishes>
																<skos:broader rdf:resource="http://purl.org/weso/cloudindex/component/Agility" />
															</ci-onto:KPIIndicator>
														</rdfindex:dataset>
														<rdfindex:weight rdf:datatype="http://www.w3.org/2001/XMLSchema#double">0.14</rdfindex:weight>
													</rdf:Description>
												</rdfindex:part-of>
												<rdfindex:part-of>
													<rdf:Description>
														<rdfindex:dataset>
															<ci-onto:KPIIndicator rdf:about="http://purl.org/weso/cloudindex/indicator/Flexibility">
																<rdfs:label xml:lang="en">Flexibility</rdfs:label>
																<rdfs:comment xml:lang="en">The ability to add or remove predefined features from a service.</rdfs:comment>
																<skos:definition xml:lang="en">The ability to add or remove predefined features from a service.</skos:definition>
																<ci-onto:defined-in rdf:resource="http://csmic.org/wp-content/uploads/2011/09/SMI-Overview-110913_v1F.pdf" />
																<ci-onto:defined-by rdf:resource="http://purl.org/weso/cloudindex/organization/CSMIC" />
																<ci-onto:weight rdf:datatype="http://www.w3.org/2001/XMLSchema#double">1.0</ci-onto:weight>
																<ci-onto:pref-value rdf:resource="http://purl.org/weso/cloudindex/ontology/High" />
																<skos:notation>Flexibility</skos:notation>
																<time:intervalStarts rdf:datatype="http://www.w3.org/2001/XMLSchema#int">2013</time:intervalStarts>
																<time:intervalFinishes rdf:datatype="http://www.w3.org/2001/XMLSchema#int">2013</time:intervalFinishes>
																<skos:broader rdf:resource="http://purl.org/weso/cloudindex/component/Agility" />
															</ci-onto:KPIIndicator>
														</rdfindex:dataset>
														<rdfindex:weight rdf:datatype="http://www.w3.org/2001/XMLSchema#double">0.14</rdfindex:weight>
													</rdf:Description>
												</rdfindex:part-of>
												<rdfindex:part-of>
													<rdf:Description>
														<rdfindex:dataset>
															<ci-onto:KPIIndicator rdf:about="http://purl.org/weso/cloudindex/indicator/Portability">
																<rdfs:label xml:lang="en">Portability</rdfs:label>
																<rdfs:comment xml:lang="en">The ability of a client to easily move a service from one service provider to another with minimal disruption.</rdfs:comment>
																<skos:definition xml:lang="en">The ability of a client to easily move a service from one service provider to another with minimal disruption.</skos:definition>
																<ci-onto:defined-in rdf:resource="http://csmic.org/wp-content/uploads/2011/09/SMI-Overview-110913_v1F.pdf" />
																<ci-onto:defined-by rdf:resource="http://purl.org/weso/cloudindex/organization/CSMIC" />
																<ci-onto:weight rdf:datatype="http://www.w3.org/2001/XMLSchema#double">1.0</ci-onto:weight>
																<ci-onto:pref-value rdf:resource="http://purl.org/weso/cloudindex/ontology/High" />
																<skos:notation>Portability</skos:notation>
																<time:intervalStarts rdf:datatype="http://www.w3.org/2001/XMLSchema#int">2013</time:intervalStarts>
																<time:intervalFinishes rdf:datatype="http://www.w3.org/2001/XMLSchema#int">2013</time:intervalFinishes>
																<skos:broader rdf:resource="http://purl.org/weso/cloudindex/component/Agility" />
															</ci-onto:KPIIndicator>
														</rdfindex:dataset>
														<rdfindex:weight rdf:datatype="http://www.w3.org/2001/XMLSchema#double">0.14</rdfindex:weight>
													</rdf:Description>
												</rdfindex:part-of>
												<rdfindex:part-of>
													<rdf:Description>
														<rdfindex:dataset>
															<ci-onto:KPIIndicator rdf:about="http://purl.org/weso/cloudindex/indicator/Scalability">
																<rdfs:label xml:lang="en">Scalability</rdfs:label>
																<rdfs:comment xml:lang="en">The ability of a service provider to increase or decrease the amount of service available to meet client requirements.</rdfs:comment>
																<skos:definition xml:lang="en">The ability of a service provider to increase or decrease the amount of service available to meet client requirements.</skos:definition>
																<ci-onto:defined-in rdf:resource="http://csmic.org/wp-content/uploads/2011/09/SMI-Overview-110913_v1F.pdf" />
																<ci-onto:defined-by rdf:resource="http://purl.org/weso/cloudindex/organization/CSMIC" />
																<ci-onto:weight rdf:datatype="http://www.w3.org/2001/XMLSchema#double">1.0</ci-onto:weight>
																<ci-onto:pref-value rdf:resource="http://purl.org/weso/cloudindex/ontology/High" />
																<skos:notation>Scalability</skos:notation>
																<time:intervalStarts rdf:datatype="http://www.w3.org/2001/XMLSchema#int">2013</time:intervalStarts>
																<time:intervalFinishes rdf:datatype="http://www.w3.org/2001/XMLSchema#int">2013</time:intervalFinishes>
																<skos:broader rdf:resource="http://purl.org/weso/cloudindex/component/Agility" />
															</ci-onto:KPIIndicator>
														</rdfindex:dataset>
														<rdfindex:weight rdf:datatype="http://www.w3.org/2001/XMLSchema#double">0.14</rdfindex:weight>
													</rdf:Description>
												</rdfindex:part-of>
											</rdf:Description>
										</rdfindex:aggregates>
										<qb:structure rdf:resource="http://purl.org/weso/cloudindex/AgilityDSD" />
										<skos:narrower rdf:resource="http://purl.org/weso/cloudindex/indicator/Adaptability" />
										<skos:narrower rdf:resource="http://purl.org/weso/cloudindex/indicator/Capacity" />
										<skos:narrower rdf:resource="http://purl.org/weso/cloudindex/indicator/Elasticity" />
										<skos:narrower rdf:resource="http://purl.org/weso/cloudindex/indicator/Extensibility" />
										<skos:narrower rdf:resource="http://purl.org/weso/cloudindex/indicator/Flexibility" />
										<skos:narrower rdf:resource="http://purl.org/weso/cloudindex/indicator/Portability" />
										<skos:narrower rdf:resource="http://purl.org/weso/cloudindex/indicator/Scalability" />
									</rdfindex:Component>
								</rdfindex:dataset>
								<rdfindex:weight rdf:datatype="http://www.w3.org/2001/XMLSchema#double">0.14</rdfindex:weight>
							</rdf:Description>
						</rdfindex:part-of>
						<rdfindex:part-of>
							<rdf:Description>
								<rdfindex:dataset>
									<rdfindex:Component rdf:about="http://purl.org/weso/cloudindex/component/Assurance">
										<rdfs:label xml:lang="en">Assurance</rdfs:label>
										<rdfs:comment xml:lang="en">This category includes key attributes that indicate how likely it is that the service will be available as
specified.</rdfs:comment>
										<ci-onto:defined-in rdf:resource="http://csmic.org/wp-content/uploads/2011/09/SMI-Overview-110913_v1F.pdf" />
										<ci-onto:defined-by rdf:resource="http://purl.org/weso/cloudindex/organization/CSMIC" />
										<ci-onto:weight rdf:datatype="http://www.w3.org/2001/XMLSchema#double">1</ci-onto:weight>
										<rdfindex:aggregates>
											<rdf:Description>
												<rdfindex:aggregation-operator rdf:resource="http://purl.org/weso/rdfindex/ontology/OWA" />
												<rdfindex:part-of>
													<rdf:Description>
														<rdfindex:dataset>
															<ci-onto:KPIIndicator rdf:about="http://purl.org/weso/cloudindex/indicator/Availability">
																<rdfs:label xml:lang="en">Availability</rdfs:label>
																<rdfs:comment xml:lang="en">The amount of time that a client can make use of a service.</rdfs:comment>
																<skos:definition xml:lang="en">The amount of time that a client can make use of a service.</skos:definition>
																<ci-onto:defined-in rdf:resource="http://csmic.org/wp-content/uploads/2011/09/SMI-Overview-110913_v1F.pdf" />
																<ci-onto:defined-by rdf:resource="http://purl.org/weso/cloudindex/organization/CSMIC" />
																<ci-onto:weight rdf:datatype="http://www.w3.org/2001/XMLSchema#double">1.0</ci-onto:weight>
																<ci-onto:pref-value rdf:resource="http://purl.org/weso/cloudindex/ontology/High" />
																<skos:notation>Availability</skos:notation>
																<time:intervalStarts rdf:datatype="http://www.w3.org/2001/XMLSchema#int">2013</time:intervalStarts>
																<time:intervalFinishes rdf:datatype="http://www.w3.org/2001/XMLSchema#int">2013</time:intervalFinishes>
																<skos:broader rdf:resource="http://purl.org/weso/cloudindex/component/Assurance" />
															</ci-onto:KPIIndicator>
														</rdfindex:dataset>
														<rdfindex:weight rdf:datatype="http://www.w3.org/2001/XMLSchema#double">0.14</rdfindex:weight>
													</rdf:Description>
												</rdfindex:part-of>
												<rdfindex:part-of>
													<rdf:Description>
														<rdfindex:dataset>
															<ci-onto:KPIIndicator rdf:about="http://purl.org/weso/cloudindex/indicator/Maintainability">
																<rdfs:label xml:lang="en">Maintainability</rdfs:label>
																<rdfs:comment xml:lang="en">Maintainability refers to the ability for the service provider to make modifications to the service to keep the service in a condition of good repair.</rdfs:comment>
																<skos:definition xml:lang="en">Maintainability refers to the ability for the service provider to make modifications to the service to keep the service in a condition of good repair.</skos:definition>
																<ci-onto:defined-in rdf:resource="http://csmic.org/wp-content/uploads/2011/09/SMI-Overview-110913_v1F.pdf" />
																<ci-onto:defined-by rdf:resource="http://purl.org/weso/cloudindex/organization/CSMIC" />
																<ci-onto:weight rdf:datatype="http://www.w3.org/2001/XMLSchema#double">1.0</ci-onto:weight>
																<ci-onto:pref-value rdf:resource="http://purl.org/weso/cloudindex/ontology/High" />
																<skos:notation>Maintainability</skos:notation>
																<time:intervalStarts rdf:datatype="http://www.w3.org/2001/XMLSchema#int">2013</time:intervalStarts>
																<time:intervalFinishes rdf:datatype="http://www.w3.org/2001/XMLSchema#int">2013</time:intervalFinishes>
																<skos:broader rdf:resource="http://purl.org/weso/cloudindex/component/Assurance" />
															</ci-onto:KPIIndicator>
														</rdfindex:dataset>
														<rdfindex:weight rdf:datatype="http://www.w3.org/2001/XMLSchema#double">0.14</rdfindex:weight>
													</rdf:Description>
												</rdfindex:part-of>
												<rdfindex:part-of>
													<rdf:Description>
														<rdfindex:dataset>
															<ci-onto:KPIIndicator rdf:about="http://purl.org/weso/cloudindex/indicator/Recoverability">
																<rdfs:label xml:lang="en">Recoverability</rdfs:label>
																<rdfs:comment xml:lang="en">Recoverability is the degree to which a service is able to quickly resume a normal state of operation after an unplanned disruption.</rdfs:comment>
																<skos:definition xml:lang="en">Recoverability is the degree to which a service is able to quickly resume a normal state of operation after an unplanned disruption.</skos:definition>
																<ci-onto:defined-in rdf:resource="http://csmic.org/wp-content/uploads/2011/09/SMI-Overview-110913_v1F.pdf" />
																<ci-onto:defined-by rdf:resource="http://purl.org/weso/cloudindex/organization/CSMIC" />
																<ci-onto:weight rdf:datatype="http://www.w3.org/2001/XMLSchema#double">1.0</ci-onto:weight>
																<ci-onto:pref-value rdf:resource="http://purl.org/weso/cloudindex/ontology/High" />
																<skos:notation>Recoverability</skos:notation>
																<time:intervalStarts rdf:datatype="http://www.w3.org/2001/XMLSchema#int">2013</time:intervalStarts>
																<time:intervalFinishes rdf:datatype="http://www.w3.org/2001/XMLSchema#int">2013</time:intervalFinishes>
																<skos:broader rdf:resource="http://purl.org/weso/cloudindex/component/Assurance" />
															</ci-onto:KPIIndicator>
														</rdfindex:dataset>
														<rdfindex:weight rdf:datatype="http://www.w3.org/2001/XMLSchema#double">0.14</rdfindex:weight>
													</rdf:Description>
												</rdfindex:part-of>
												<rdfindex:part-of>
													<rdf:Description>
														<rdfindex:dataset>
															<ci-onto:KPIIndicator rdf:about="http://purl.org/weso/cloudindex/indicator/Reliability">
																<rdfs:label xml:lang="en">Reliability</rdfs:label>
																<rdfs:comment xml:lang="en">Reliability reflects measures of how a service operates without failure under
given conditions during a given time period.</rdfs:comment>
																<skos:definition xml:lang="en">Reliability reflects measures of how a service operates without failure under
given conditions during a given time period.</skos:definition>
																<ci-onto:defined-in rdf:resource="http://csmic.org/wp-content/uploads/2011/09/SMI-Overview-110913_v1F.pdf" />
																<ci-onto:defined-by rdf:resource="http://purl.org/weso/cloudindex/organization/CSMIC" />
																<ci-onto:weight rdf:datatype="http://www.w3.org/2001/XMLSchema#double">1.0</ci-onto:weight>
																<ci-onto:pref-value rdf:resource="http://purl.org/weso/cloudindex/ontology/High" />
																<skos:notation>Reliability</skos:notation>
																<time:intervalStarts rdf:datatype="http://www.w3.org/2001/XMLSchema#int">2013</time:intervalStarts>
																<time:intervalFinishes rdf:datatype="http://www.w3.org/2001/XMLSchema#int">2013</time:intervalFinishes>
																<skos:broader rdf:resource="http://purl.org/weso/cloudindex/component/Assurance" />
															</ci-onto:KPIIndicator>
														</rdfindex:dataset>
														<rdfindex:weight rdf:datatype="http://www.w3.org/2001/XMLSchema#double">0.14</rdfindex:weight>
													</rdf:Description>
												</rdfindex:part-of>
												<rdfindex:part-of>
													<rdf:Description>
														<rdfindex:dataset>
															<ci-onto:KPIIndicator rdf:about="http://purl.org/weso/cloudindex/indicator/Resiliency">
																<rdfs:label xml:lang="en">Resiliency</rdfs:label>
																<rdfs:comment xml:lang="en">The ability of a service to continue to operate properly in the event of a failure in
one or more of its components.</rdfs:comment>
																<skos:definition xml:lang="en">The ability of a service to continue to operate properly in the event of a failure in
one or more of its components.</skos:definition>
																<ci-onto:defined-in rdf:resource="http://csmic.org/wp-content/uploads/2011/09/SMI-Overview-110913_v1F.pdf" />
																<ci-onto:defined-by rdf:resource="http://purl.org/weso/cloudindex/organization/CSMIC" />
																<ci-onto:weight rdf:datatype="http://www.w3.org/2001/XMLSchema#double">1.0</ci-onto:weight>
																<ci-onto:pref-value rdf:resource="http://purl.org/weso/cloudindex/ontology/High" />
																<skos:notation>Resiliency</skos:notation>
																<time:intervalStarts rdf:datatype="http://www.w3.org/2001/XMLSchema#int">2013</time:intervalStarts>
																<time:intervalFinishes rdf:datatype="http://www.w3.org/2001/XMLSchema#int">2013</time:intervalFinishes>
																<skos:broader rdf:resource="http://purl.org/weso/cloudindex/component/Assurance" />
															</ci-onto:KPIIndicator>
														</rdfindex:dataset>
														<rdfindex:weight rdf:datatype="http://www.w3.org/2001/XMLSchema#double">0.14</rdfindex:weight>
													</rdf:Description>
												</rdfindex:part-of>
												<rdfindex:part-of>
													<rdf:Description>
														<rdfindex:dataset>
															<ci-onto:KPIIndicator rdf:about="http://purl.org/weso/cloudindex/indicator/Stability">
																<rdfs:label xml:lang="en">Stability</rdfs:label>
																<rdfs:comment xml:lang="en">The degree to which the service is resistant to change, deterioration, or displacement.</rdfs:comment>
																<skos:definition xml:lang="en">The degree to which the service is resistant to change, deterioration, or displacement.</skos:definition>
																<ci-onto:defined-in rdf:resource="http://csmic.org/wp-content/uploads/2011/09/SMI-Overview-110913_v1F.pdf" />
																<ci-onto:defined-by rdf:resource="http://purl.org/weso/cloudindex/organization/CSMIC" />
																<ci-onto:weight rdf:datatype="http://www.w3.org/2001/XMLSchema#double">1.0</ci-onto:weight>
																<ci-onto:pref-value rdf:resource="http://purl.org/weso/cloudindex/ontology/High" />
																<skos:notation>Stability</skos:notation>
																<time:intervalStarts rdf:datatype="http://www.w3.org/2001/XMLSchema#int">2013</time:intervalStarts>
																<time:intervalFinishes rdf:datatype="http://www.w3.org/2001/XMLSchema#int">2013</time:intervalFinishes>
																<skos:broader rdf:resource="http://purl.org/weso/cloudindex/component/Assurance" />
															</ci-onto:KPIIndicator>
														</rdfindex:dataset>
														<rdfindex:weight rdf:datatype="http://www.w3.org/2001/XMLSchema#double">0.14</rdfindex:weight>
													</rdf:Description>
												</rdfindex:part-of>
												<rdfindex:part-of>
													<rdf:Description>
														<rdfindex:dataset>
															<ci-onto:KPIIndicator rdf:about="http://purl.org/weso/cloudindex/indicator/Serviceability">
																<rdfs:label xml:lang="en">Serviceability</rdfs:label>
																<rdfs:comment xml:lang="en">The ease and efficiency of performing maintenance and correcting problems with the service.</rdfs:comment>
																<skos:definition xml:lang="en">The ease and efficiency of performing maintenance and correcting problems with the service.</skos:definition>
																<ci-onto:defined-in rdf:resource="http://csmic.org/wp-content/uploads/2011/09/SMI-Overview-110913_v1F.pdf" />
																<ci-onto:defined-by rdf:resource="http://purl.org/weso/cloudindex/organization/CSMIC" />
																<ci-onto:weight rdf:datatype="http://www.w3.org/2001/XMLSchema#double">1.0</ci-onto:weight>
																<ci-onto:pref-value rdf:resource="http://purl.org/weso/cloudindex/ontology/High" />
																<skos:notation>Serviceability</skos:notation>
																<time:intervalStarts rdf:datatype="http://www.w3.org/2001/XMLSchema#int">2013</time:intervalStarts>
																<time:intervalFinishes rdf:datatype="http://www.w3.org/2001/XMLSchema#int">2013</time:intervalFinishes>
																<skos:broader rdf:resource="http://purl.org/weso/cloudindex/component/Assurance" />
															</ci-onto:KPIIndicator>
														</rdfindex:dataset>
														<rdfindex:weight rdf:datatype="http://www.w3.org/2001/XMLSchema#double">0.14</rdfindex:weight>
													</rdf:Description>
												</rdfindex:part-of>
											</rdf:Description>
										</rdfindex:aggregates>
										<qb:structure rdf:resource="http://purl.org/weso/cloudindex/AssuranceDSD" />
										<skos:narrower rdf:resource="http://purl.org/weso/cloudindex/indicator/Availability" />
										<skos:narrower rdf:resource="http://purl.org/weso/cloudindex/indicator/Maintainability" />
										<skos:narrower rdf:resource="http://purl.org/weso/cloudindex/indicator/Recoverability" />
										<skos:narrower rdf:resource="http://purl.org/weso/cloudindex/indicator/Reliability" />
										<skos:narrower rdf:resource="http://purl.org/weso/cloudindex/indicator/Resiliency" />
										<skos:narrower rdf:resource="http://purl.org/weso/cloudindex/indicator/Stability" />
										<skos:narrower rdf:resource="http://purl.org/weso/cloudindex/indicator/Serviceability" />
									</rdfindex:Component>
								</rdfindex:dataset>
								<rdfindex:weight rdf:datatype="http://www.w3.org/2001/XMLSchema#double">0.14</rdfindex:weight>
							</rdf:Description>
						</rdfindex:part-of>
						<rdfindex:part-of>
							<rdf:Description>
								<rdfindex:dataset>
									<rdfindex:Component rdf:about="http://purl.org/weso/cloudindex/component/Financial">
										<rdfs:label xml:lang="en">Financial</rdfs:label>
										<rdfs:comment xml:lang="en">The amount of money spent on the service by the client.</rdfs:comment>
										<ci-onto:defined-in rdf:resource="http://csmic.org/wp-content/uploads/2011/09/SMI-Overview-110913_v1F.pdf" />
										<ci-onto:defined-by rdf:resource="http://purl.org/weso/cloudindex/organization/CSMIC" />
										<ci-onto:weight rdf:datatype="http://www.w3.org/2001/XMLSchema#double">1</ci-onto:weight>
										<rdfindex:aggregates>
											<rdf:Description>
												<rdfindex:aggregation-operator rdf:resource="http://purl.org/weso/rdfindex/ontology/OWA" />
												<rdfindex:part-of>
													<rdf:Description>
														<rdfindex:dataset>
															<ci-onto:KPIIndicator rdf:about="http://purl.org/weso/cloudindex/indicator/Acquisition">
																<rdfs:label xml:lang="en">Acquisition</rdfs:label>
																<rdfs:comment xml:lang="en">Any client costs to acquire the rights and ability to use a service and to move from an existing service to the new one.</rdfs:comment>
																<skos:definition xml:lang="en">Any client costs to acquire the rights and ability to use a service and to move
from an existing service to the new one.</skos:definition>
																<ci-onto:defined-in rdf:resource="http://csmic.org/wp-content/uploads/2011/09/SMI-Overview-110913_v1F.pdf" />
																<ci-onto:defined-by rdf:resource="http://purl.org/weso/cloudindex/organization/CSMIC" />
																<ci-onto:weight rdf:datatype="http://www.w3.org/2001/XMLSchema#double">1.0</ci-onto:weight>
																<ci-onto:pref-value rdf:resource="http://purl.org/weso/cloudindex/ontology/High" />
																<skos:notation>Acquisition</skos:notation>
																<time:intervalStarts rdf:datatype="http://www.w3.org/2001/XMLSchema#int">2013</time:intervalStarts>
																<time:intervalFinishes rdf:datatype="http://www.w3.org/2001/XMLSchema#int">2013</time:intervalFinishes>
																<skos:broader rdf:resource="http://purl.org/weso/cloudindex/component/Financial" />
															</ci-onto:KPIIndicator>
														</rdfindex:dataset>
														<rdfindex:weight rdf:datatype="http://www.w3.org/2001/XMLSchema#double">0.33</rdfindex:weight>
													</rdf:Description>
												</rdfindex:part-of>
												<rdfindex:part-of>
													<rdf:Description>
														<rdfindex:dataset>
															<ci-onto:KPIIndicator rdf:about="http://purl.org/weso/cloudindex/indicator/OngoingCost">
																<rdfs:label xml:lang="en">On-going Cost</rdfs:label>
																<rdfs:comment xml:lang="en">The client cost to operate a service. This includes both recurring flat costs (e.g.,
monthly access fees) and usage-based costs.</rdfs:comment>
																<skos:definition xml:lang="en">The client cost to operate a service. This includes both recurring flat costs (e.g.,
monthly access fees) and usage-based costs.</skos:definition>
																<ci-onto:defined-in rdf:resource="http://csmic.org/wp-content/uploads/2011/09/SMI-Overview-110913_v1F.pdf" />
																<ci-onto:defined-by rdf:resource="http://purl.org/weso/cloudindex/organization/CSMIC" />
																<ci-onto:weight rdf:datatype="http://www.w3.org/2001/XMLSchema#double">1.0</ci-onto:weight>
																<ci-onto:pref-value rdf:resource="http://purl.org/weso/cloudindex/ontology/High" />
																<skos:notation>OngoingCost</skos:notation>
																<time:intervalStarts rdf:datatype="http://www.w3.org/2001/XMLSchema#int">2013</time:intervalStarts>
																<time:intervalFinishes rdf:datatype="http://www.w3.org/2001/XMLSchema#int">2013</time:intervalFinishes>
																<skos:broader rdf:resource="http://purl.org/weso/cloudindex/component/Financial" />
															</ci-onto:KPIIndicator>
														</rdfindex:dataset>
														<rdfindex:weight rdf:datatype="http://www.w3.org/2001/XMLSchema#double">0.33</rdfindex:weight>
													</rdf:Description>
												</rdfindex:part-of>
												<rdfindex:part-of>
													<rdf:Description>
														<rdfindex:dataset>
															<ci-onto:KPIIndicator rdf:about="http://purl.org/weso/cloudindex/indicator/Profit">
																<rdfs:label xml:lang="en">Profit</rdfs:label>
																<rdfs:comment xml:lang="en">Arrangement between client and provider(s) under which costs or profits of a
service are shared by the involved parties, according to an agreed upon formula.</rdfs:comment>
																<skos:definition xml:lang="en">Arrangement between client and provider(s) under which costs or profits of a
service are shared by the involved parties, according to an agreed upon formula.</skos:definition>
																<ci-onto:defined-in rdf:resource="http://csmic.org/wp-content/uploads/2011/09/SMI-Overview-110913_v1F.pdf" />
																<ci-onto:defined-by rdf:resource="http://purl.org/weso/cloudindex/organization/CSMIC" />
																<ci-onto:weight rdf:datatype="http://www.w3.org/2001/XMLSchema#double">1.0</ci-onto:weight>
																<ci-onto:pref-value rdf:resource="http://purl.org/weso/cloudindex/ontology/High" />
																<skos:notation>Profit</skos:notation>
																<time:intervalStarts rdf:datatype="http://www.w3.org/2001/XMLSchema#int">2013</time:intervalStarts>
																<time:intervalFinishes rdf:datatype="http://www.w3.org/2001/XMLSchema#int">2013</time:intervalFinishes>
																<skos:broader rdf:resource="http://purl.org/weso/cloudindex/component/Financial" />
															</ci-onto:KPIIndicator>
														</rdfindex:dataset>
														<rdfindex:weight rdf:datatype="http://www.w3.org/2001/XMLSchema#double">0.33</rdfindex:weight>
													</rdf:Description>
												</rdfindex:part-of>
											</rdf:Description>
										</rdfindex:aggregates>
										<qb:structure rdf:resource="http://purl.org/weso/cloudindex/FinancialDSD" />
										<skos:narrower rdf:resource="http://purl.org/weso/cloudindex/indicator/Acquisition" />
										<skos:narrower rdf:resource="http://purl.org/weso/cloudindex/indicator/OngoingCost" />
										<skos:narrower rdf:resource="http://purl.org/weso/cloudindex/indicator/Profit" />
									</rdfindex:Component>
								</rdfindex:dataset>
								<rdfindex:weight rdf:datatype="http://www.w3.org/2001/XMLSchema#double">0.14</rdfindex:weight>
							</rdf:Description>
						</rdfindex:part-of>
						<rdfindex:part-of>
							<rdf:Description>
								<rdfindex:dataset>
									<rdfindex:Component rdf:about="http://purl.org/weso/cloudindex/component/Performance">
										<rdfs:label xml:lang="en">Performance</rdfs:label>
										<rdfs:comment xml:lang="en">This category covers the features and functions of the provided services.</rdfs:comment>
										<ci-onto:defined-in rdf:resource="http://csmic.org/wp-content/uploads/2011/09/SMI-Overview-110913_v1F.pdf" />
										<ci-onto:defined-by rdf:resource="http://purl.org/weso/cloudindex/organization/CSMIC" />
										<ci-onto:weight rdf:datatype="http://www.w3.org/2001/XMLSchema#double">1</ci-onto:weight>
										<rdfindex:aggregates>
											<rdf:Description>
												<rdfindex:aggregation-operator rdf:resource="http://purl.org/weso/rdfindex/ontology/OWA" />
												<rdfindex:part-of>
													<rdf:Description>
														<rdfindex:dataset>
															<ci-onto:KPIIndicator rdf:about="http://purl.org/weso/cloudindex/indicator/Accuracy">
																<rdfs:label xml:lang="en">Accuracy</rdfs:label>
																<rdfs:comment xml:lang="en">The extent to which a service adheres to its requirements.</rdfs:comment>
																<skos:definition xml:lang="en">The extent to which a service adheres to its requirements.</skos:definition>
																<ci-onto:defined-in rdf:resource="http://csmic.org/wp-content/uploads/2011/09/SMI-Overview-110913_v1F.pdf" />
																<ci-onto:defined-by rdf:resource="http://purl.org/weso/cloudindex/organization/CSMIC" />
																<ci-onto:weight rdf:datatype="http://www.w3.org/2001/XMLSchema#double">1.0</ci-onto:weight>
																<ci-onto:pref-value rdf:resource="http://purl.org/weso/cloudindex/ontology/High" />
																<skos:notation>Accuracy</skos:notation>
																<time:intervalStarts rdf:datatype="http://www.w3.org/2001/XMLSchema#int">2013</time:intervalStarts>
																<time:intervalFinishes rdf:datatype="http://www.w3.org/2001/XMLSchema#int">2013</time:intervalFinishes>
																<skos:broader rdf:resource="http://purl.org/weso/cloudindex/component/Performance" />
															</ci-onto:KPIIndicator>
														</rdfindex:dataset>
														<rdfindex:weight rdf:datatype="http://www.w3.org/2001/XMLSchema#double">0.2</rdfindex:weight>
													</rdf:Description>
												</rdfindex:part-of>
												<rdfindex:part-of>
													<rdf:Description>
														<rdfindex:dataset>
															<ci-onto:KPIIndicator rdf:about="http://purl.org/weso/cloudindex/indicator/Functionality">
																<rdfs:label xml:lang="en">Functionality</rdfs:label>
																<rdfs:comment xml:lang="en">The specific features provided by a service.</rdfs:comment>
																<skos:definition xml:lang="en">The specific features provided by a service.</skos:definition>
																<ci-onto:defined-in rdf:resource="http://csmic.org/wp-content/uploads/2011/09/SMI-Overview-110913_v1F.pdf" />
																<ci-onto:defined-by rdf:resource="http://purl.org/weso/cloudindex/organization/CSMIC" />
																<ci-onto:weight rdf:datatype="http://www.w3.org/2001/XMLSchema#double">1.0</ci-onto:weight>
																<ci-onto:pref-value rdf:resource="http://purl.org/weso/cloudindex/ontology/High" />
																<skos:notation>Functionality</skos:notation>
																<time:intervalStarts rdf:datatype="http://www.w3.org/2001/XMLSchema#int">2013</time:intervalStarts>
																<time:intervalFinishes rdf:datatype="http://www.w3.org/2001/XMLSchema#int">2013</time:intervalFinishes>
																<skos:broader rdf:resource="http://purl.org/weso/cloudindex/component/Performance" />
															</ci-onto:KPIIndicator>
														</rdfindex:dataset>
														<rdfindex:weight rdf:datatype="http://www.w3.org/2001/XMLSchema#double">0.2</rdfindex:weight>
													</rdf:Description>
												</rdfindex:part-of>
												<rdfindex:part-of>
													<rdf:Description>
														<rdfindex:dataset>
															<ci-onto:KPIIndicator rdf:about="http://purl.org/weso/cloudindex/indicator/Suitability">
																<rdfs:label xml:lang="en">Suitability</rdfs:label>
																<rdfs:comment xml:lang="en">How closely do the capabilities of the service match the needs of the client.</rdfs:comment>
																<skos:definition xml:lang="en">How closely do the capabilities of the service match the needs of the client.</skos:definition>
																<ci-onto:defined-in rdf:resource="http://csmic.org/wp-content/uploads/2011/09/SMI-Overview-110913_v1F.pdf" />
																<ci-onto:defined-by rdf:resource="http://purl.org/weso/cloudindex/organization/CSMIC" />
																<ci-onto:weight rdf:datatype="http://www.w3.org/2001/XMLSchema#double">1.0</ci-onto:weight>
																<ci-onto:pref-value rdf:resource="http://purl.org/weso/cloudindex/ontology/High" />
																<skos:notation>Suitability</skos:notation>
																<time:intervalStarts rdf:datatype="http://www.w3.org/2001/XMLSchema#int">2013</time:intervalStarts>
																<time:intervalFinishes rdf:datatype="http://www.w3.org/2001/XMLSchema#int">2013</time:intervalFinishes>
																<skos:broader rdf:resource="http://purl.org/weso/cloudindex/component/Performance" />
																<rdf:type rdf:resource="http://purl.org/weso/cloudindex/ontology/KPIIndicator" />
																<rdfs:label xml:lang="en">Suitability</rdfs:label>
																<rdfs:comment xml:lang="en">How closely do the capabilities of the service match the needs of the client.</rdfs:comment>
																<skos:definition xml:lang="en">How closely do the capabilities of the service match the needs of the client.</skos:definition>
																<ci-onto:defined-in rdf:resource="http://csmic.org/wp-content/uploads/2011/09/SMI-Overview-110913_v1F.pdf" />
																<ci-onto:defined-by rdf:resource="http://purl.org/weso/cloudindex/organization/CSMIC" />
																<ci-onto:weight rdf:datatype="http://www.w3.org/2001/XMLSchema#double">1.0</ci-onto:weight>
																<ci-onto:pref-value rdf:resource="http://purl.org/weso/cloudindex/ontology/High" />
																<skos:notation>Suitability</skos:notation>
																<time:intervalStarts rdf:datatype="http://www.w3.org/2001/XMLSchema#int">2013</time:intervalStarts>
																<time:intervalFinishes rdf:datatype="http://www.w3.org/2001/XMLSchema#int">2013</time:intervalFinishes>
																<skos:broader rdf:resource="http://purl.org/weso/cloudindex/component/Usability" />
															</ci-onto:KPIIndicator>
														</rdfindex:dataset>
														<rdfindex:weight rdf:datatype="http://www.w3.org/2001/XMLSchema#double">0.2</rdfindex:weight>
													</rdf:Description>
												</rdfindex:part-of>
												<rdfindex:part-of>
													<rdf:Description>
														<rdfindex:dataset>
															<ci-onto:KPIIndicator rdf:about="http://purl.org/weso/cloudindex/indicator/Interoperability">
																<rdfs:label xml:lang="en">Suitability</rdfs:label>
																<rdfs:comment xml:lang="en">The ability of a service to easily interact with other services (from the same service provider and from other service providers).</rdfs:comment>
																<skos:definition xml:lang="en">The ability of a service to easily interact with other services (from the same service provider and from other service providers).</skos:definition>
																<ci-onto:defined-in rdf:resource="http://csmic.org/wp-content/uploads/2011/09/SMI-Overview-110913_v1F.pdf" />
																<ci-onto:defined-by rdf:resource="http://purl.org/weso/cloudindex/organization/CSMIC" />
																<ci-onto:weight rdf:datatype="http://www.w3.org/2001/XMLSchema#double">1.0</ci-onto:weight>
																<ci-onto:pref-value rdf:resource="http://purl.org/weso/cloudindex/ontology/High" />
																<skos:notation>Interoperability</skos:notation>
																<time:intervalStarts rdf:datatype="http://www.w3.org/2001/XMLSchema#int">2013</time:intervalStarts>
																<time:intervalFinishes rdf:datatype="http://www.w3.org/2001/XMLSchema#int">2013</time:intervalFinishes>
																<skos:broader rdf:resource="http://purl.org/weso/cloudindex/component/Performance" />
															</ci-onto:KPIIndicator>
														</rdfindex:dataset>
														<rdfindex:weight rdf:datatype="http://www.w3.org/2001/XMLSchema#double">0.2</rdfindex:weight>
													</rdf:Description>
												</rdfindex:part-of>
												<rdfindex:part-of>
													<rdf:Description>
														<rdfindex:dataset>
															<ci-onto:KPIIndicator rdf:about="http://purl.org/weso/cloudindex/indicator/ServiceResponseTime">
																<rdfs:label xml:lang="en">Service Response Time</rdfs:label>
																<rdfs:comment xml:lang="en">An indicator of the time between when a service is requested and when the response is available.</rdfs:comment>
																<skos:definition xml:lang="en">An indicator of the time between when a service is requested and when the response is available.</skos:definition>
																<ci-onto:defined-in rdf:resource="http://csmic.org/wp-content/uploads/2011/09/SMI-Overview-110913_v1F.pdf" />
																<ci-onto:defined-by rdf:resource="http://purl.org/weso/cloudindex/organization/CSMIC" />
																<ci-onto:weight rdf:datatype="http://www.w3.org/2001/XMLSchema#double">1.0</ci-onto:weight>
																<ci-onto:pref-value rdf:resource="http://purl.org/weso/cloudindex/ontology/High" />
																<skos:notation>ServiceResponseTime</skos:notation>
																<time:intervalStarts rdf:datatype="http://www.w3.org/2001/XMLSchema#int">2013</time:intervalStarts>
																<time:intervalFinishes rdf:datatype="http://www.w3.org/2001/XMLSchema#int">2013</time:intervalFinishes>
																<skos:broader rdf:resource="http://purl.org/weso/cloudindex/component/Performance" />
															</ci-onto:KPIIndicator>
														</rdfindex:dataset>
														<rdfindex:weight rdf:datatype="http://www.w3.org/2001/XMLSchema#double">0.2</rdfindex:weight>
													</rdf:Description>
												</rdfindex:part-of>
											</rdf:Description>
										</rdfindex:aggregates>
										<qb:structure rdf:resource="http://purl.org/weso/cloudindex/PerformanceDSD" />
										<skos:narrower rdf:resource="http://purl.org/weso/cloudindex/indicator/Accuracy" />
										<skos:narrower rdf:resource="http://purl.org/weso/cloudindex/indicator/Functionality" />
										<skos:narrower rdf:resource="http://purl.org/weso/cloudindex/indicator/Suitability" />
										<skos:narrower rdf:resource="http://purl.org/weso/cloudindex/indicator/Interoperability" />
										<skos:narrower rdf:resource="http://purl.org/weso/cloudindex/indicator/ServiceResponseTime" />
									</rdfindex:Component>
								</rdfindex:dataset>
								<rdfindex:weight rdf:datatype="http://www.w3.org/2001/XMLSchema#double">0.14</rdfindex:weight>
							</rdf:Description>
						</rdfindex:part-of>
						<rdfindex:part-of>
							<rdf:Description>
								<rdfindex:dataset>
									<rdfindex:Component rdf:about="http://purl.org/weso/cloudindex/component/SecurityPrivacy">
										<rdfs:label xml:lang="en">Security and Privacy</rdfs:label>
										<rdfs:comment xml:lang="en">This category includes attributes that indicate the effectiveness of a service provider's controls on
access to services, service data, and the physical facilities from which services are provided.</rdfs:comment>
										<ci-onto:defined-in rdf:resource="http://csmic.org/wp-content/uploads/2011/09/SMI-Overview-110913_v1F.pdf" />
										<ci-onto:defined-by rdf:resource="http://purl.org/weso/cloudindex/organization/CSMIC" />
										<ci-onto:weight rdf:datatype="http://www.w3.org/2001/XMLSchema#double">1</ci-onto:weight>
										<rdfindex:aggregates>
											<rdf:Description>
												<rdfindex:aggregation-operator rdf:resource="http://purl.org/weso/rdfindex/ontology/OWA" />
												<rdfindex:part-of>
													<rdf:Description>
														<rdfindex:dataset>
															<ci-onto:KPIIndicator rdf:about="http://purl.org/weso/cloudindex/indicator/AccessControl">
																<rdfs:label xml:lang="en">Access Control</rdfs:label>
																<rdfs:comment xml:lang="en">Policies and processes in use by the service provider to ensure that only the provider and client personnel with appropriate status/reasons to make use of or modify data/work products may do so.</rdfs:comment>
																<skos:definition xml:lang="en">Policies and processes in use by the service provider to ensure that only the provider and client personnel with appropriate status/reasons to make use of or modify data/work products may do so.</skos:definition>
																<ci-onto:defined-in rdf:resource="http://csmic.org/wp-content/uploads/2011/09/SMI-Overview-110913_v1F.pdf" />
																<ci-onto:defined-by rdf:resource="http://purl.org/weso/cloudindex/organization/CSMIC" />
																<ci-onto:weight rdf:datatype="http://www.w3.org/2001/XMLSchema#double">1.0</ci-onto:weight>
																<ci-onto:pref-value rdf:resource="http://purl.org/weso/cloudindex/ontology/High" />
																<skos:notation>AccessControl</skos:notation>
																<time:intervalStarts rdf:datatype="http://www.w3.org/2001/XMLSchema#int">2013</time:intervalStarts>
																<time:intervalFinishes rdf:datatype="http://www.w3.org/2001/XMLSchema#int">2013</time:intervalFinishes>
																<skos:broader rdf:resource="http://purl.org/weso/cloudindex/component/SecurityPrivacy" />
															</ci-onto:KPIIndicator>
														</rdfindex:dataset>
														<rdfindex:weight rdf:datatype="http://www.w3.org/2001/XMLSchema#double">0.1</rdfindex:weight>
													</rdf:Description>
												</rdfindex:part-of>
												<rdfindex:part-of>
													<rdf:Description>
														<rdfindex:dataset>
															<ci-onto:KPIIndicator rdf:about="http://purl.org/weso/cloudindex/indicator/GeographicalConstraint">
																<rdfs:label xml:lang="en">Geographical Constraint</rdfs:label>
																<rdfs:comment xml:lang="en">The client's constraints on service location based on geography.</rdfs:comment>
																<skos:definition xml:lang="en">The client's constraints on service location based on geography.</skos:definition>
																<ci-onto:defined-in rdf:resource="http://csmic.org/wp-content/uploads/2011/09/SMI-Overview-110913_v1F.pdf" />
																<ci-onto:defined-by rdf:resource="http://purl.org/weso/cloudindex/organization/CSMIC" />
																<ci-onto:weight rdf:datatype="http://www.w3.org/2001/XMLSchema#double">1.0</ci-onto:weight>
																<ci-onto:pref-value rdf:resource="http://purl.org/weso/cloudindex/ontology/High" />
																<skos:notation>GeographicalConstraint</skos:notation>
																<time:intervalStarts rdf:datatype="http://www.w3.org/2001/XMLSchema#int">2013</time:intervalStarts>
																<time:intervalFinishes rdf:datatype="http://www.w3.org/2001/XMLSchema#int">2013</time:intervalFinishes>
																<skos:broader rdf:resource="http://purl.org/weso/cloudindex/component/SecurityPrivacy" />
															</ci-onto:KPIIndicator>
														</rdfindex:dataset>
														<rdfindex:weight rdf:datatype="http://www.w3.org/2001/XMLSchema#double">0.1</rdfindex:weight>
													</rdf:Description>
												</rdfindex:part-of>
												<rdfindex:part-of>
													<rdf:Description>
														<rdfindex:dataset>
															<ci-onto:KPIIndicator rdf:about="http://purl.org/weso/cloudindex/indicator/PoliticalConstraint">
																<rdfs:label xml:lang="en">Political Constraint</rdfs:label>
																<rdfs:comment xml:lang="en">The client's constraints on service location based on politics.</rdfs:comment>
																<skos:definition xml:lang="en">The client's constraints on service location based on geography.</skos:definition>
																<ci-onto:defined-in rdf:resource="http://csmic.org/wp-content/uploads/2011/09/SMI-Overview-110913_v1F.pdf" />
																<ci-onto:defined-by rdf:resource="http://purl.org/weso/cloudindex/organization/CSMIC" />
																<ci-onto:weight rdf:datatype="http://www.w3.org/2001/XMLSchema#double">1.0</ci-onto:weight>
																<ci-onto:pref-value rdf:resource="http://purl.org/weso/cloudindex/ontology/High" />
																<skos:notation>PoliticalConstraint</skos:notation>
																<time:intervalStarts rdf:datatype="http://www.w3.org/2001/XMLSchema#int">2013</time:intervalStarts>
																<time:intervalFinishes rdf:datatype="http://www.w3.org/2001/XMLSchema#int">2013</time:intervalFinishes>
																<skos:broader rdf:resource="http://purl.org/weso/cloudindex/component/SecurityPrivacy" />
															</ci-onto:KPIIndicator>
														</rdfindex:dataset>
														<rdfindex:weight rdf:datatype="http://www.w3.org/2001/XMLSchema#double">0.1</rdfindex:weight>
													</rdf:Description>
												</rdfindex:part-of>
												<rdfindex:part-of>
													<rdf:Description>
														<rdfindex:dataset>
															<ci-onto:KPIIndicator rdf:about="http://purl.org/weso/cloudindex/indicator/DataIntegrity">
																<rdfs:label xml:lang="en">Data Integrity</rdfs:label>
																<rdfs:comment xml:lang="en">Keeping the data that is created, used, and stored in its correct form so that clients may be confident that it is accurate and valid.</rdfs:comment>
																<skos:definition xml:lang="en">Keeping the data that is created, used, and stored in its correct form so that clients may be confident that it is accurate and valid.</skos:definition>
																<ci-onto:defined-in rdf:resource="http://csmic.org/wp-content/uploads/2011/09/SMI-Overview-110913_v1F.pdf" />
																<ci-onto:defined-by rdf:resource="http://purl.org/weso/cloudindex/organization/CSMIC" />
																<ci-onto:weight rdf:datatype="http://www.w3.org/2001/XMLSchema#double">1.0</ci-onto:weight>
																<ci-onto:pref-value rdf:resource="http://purl.org/weso/cloudindex/ontology/High" />
																<skos:notation>DataIntegrity</skos:notation>
																<time:intervalStarts rdf:datatype="http://www.w3.org/2001/XMLSchema#int">2013</time:intervalStarts>
																<time:intervalFinishes rdf:datatype="http://www.w3.org/2001/XMLSchema#int">2013</time:intervalFinishes>
																<skos:broader rdf:resource="http://purl.org/weso/cloudindex/component/SecurityPrivacy" />
															</ci-onto:KPIIndicator>
														</rdfindex:dataset>
														<rdfindex:weight rdf:datatype="http://www.w3.org/2001/XMLSchema#double">0.1</rdfindex:weight>
													</rdf:Description>
												</rdfindex:part-of>
												<rdfindex:part-of>
													<rdf:Description>
														<rdfindex:dataset>
															<ci-onto:KPIIndicator rdf:about="http://purl.org/weso/cloudindex/indicator/DataPrivacy">
																<rdfs:label xml:lang="en">Data Privacy</rdfs:label>
																<rdfs:comment xml:lang="en">Client restrictions on access and use of client data are enforced by the service provider. Any failures of these protections are promptly detected and reported to the client.</rdfs:comment>
																<skos:definition xml:lang="en">Client restrictions on access and use of client data are enforced by the service provider. Any failures of these protections are promptly detected and reported to the client.</skos:definition>
																<ci-onto:defined-in rdf:resource="http://csmic.org/wp-content/uploads/2011/09/SMI-Overview-110913_v1F.pdf" />
																<ci-onto:defined-by rdf:resource="http://purl.org/weso/cloudindex/organization/CSMIC" />
																<ci-onto:weight rdf:datatype="http://www.w3.org/2001/XMLSchema#double">1.0</ci-onto:weight>
																<ci-onto:pref-value rdf:resource="http://purl.org/weso/cloudindex/ontology/High" />
																<skos:notation>DataPrivacy</skos:notation>
																<time:intervalStarts rdf:datatype="http://www.w3.org/2001/XMLSchema#int">2013</time:intervalStarts>
																<time:intervalFinishes rdf:datatype="http://www.w3.org/2001/XMLSchema#int">2013</time:intervalFinishes>
																<skos:broader rdf:resource="http://purl.org/weso/cloudindex/component/SecurityPrivacy" />
															</ci-onto:KPIIndicator>
														</rdfindex:dataset>
														<rdfindex:weight rdf:datatype="http://www.w3.org/2001/XMLSchema#double">0.1</rdfindex:weight>
													</rdf:Description>
												</rdfindex:part-of>
												<rdfindex:part-of>
													<rdf:Description>
														<rdfindex:dataset rdf:resource="http://purl.org/weso/cloudindex/indicator/DataPrivacy" />
														<rdfindex:weight rdf:datatype="http://www.w3.org/2001/XMLSchema#double">0.1</rdfindex:weight>
													</rdf:Description>
												</rdfindex:part-of>
												<rdfindex:part-of>
													<rdf:Description>
														<rdfindex:dataset>
															<ci-onto:KPIIndicator rdf:about="http://purl.org/weso/cloudindex/indicator/DataLoss">
																<rdfs:label xml:lang="en">Data Loss</rdfs:label>
																<rdfs:comment xml:lang="en">Client restrictions on access and use of client data are enforced by the service provider. Any failures of these protections are promptly detected and reported to the client.</rdfs:comment>
																<skos:definition xml:lang="en">Client restrictions on access and use of client data are enforced by the service provider. Any failures of these protections are promptly detected and reported to the client.</skos:definition>
																<ci-onto:defined-in rdf:resource="http://csmic.org/wp-content/uploads/2011/09/SMI-Overview-110913_v1F.pdf" />
																<ci-onto:defined-by rdf:resource="http://purl.org/weso/cloudindex/organization/CSMIC" />
																<ci-onto:weight rdf:datatype="http://www.w3.org/2001/XMLSchema#double">1.0</ci-onto:weight>
																<ci-onto:pref-value rdf:resource="http://purl.org/weso/cloudindex/ontology/High" />
																<skos:notation>DataLoss</skos:notation>
																<time:intervalStarts rdf:datatype="http://www.w3.org/2001/XMLSchema#int">2013</time:intervalStarts>
																<time:intervalFinishes rdf:datatype="http://www.w3.org/2001/XMLSchema#int">2013</time:intervalFinishes>
																<skos:broader rdf:resource="http://purl.org/weso/cloudindex/component/SecurityPrivacy" />
															</ci-onto:KPIIndicator>
														</rdfindex:dataset>
														<rdfindex:weight rdf:datatype="http://www.w3.org/2001/XMLSchema#double">0.1</rdfindex:weight>
													</rdf:Description>
												</rdfindex:part-of>
												<rdfindex:part-of>
													<rdf:Description>
														<rdfindex:dataset>
															<ci-onto:KPIIndicator rdf:about="http://purl.org/weso/cloudindex/indicator/EnvironmentSecurity">
																<rdfs:label xml:lang="en">Physical &amp; Environmental Security</rdfs:label>
																<rdfs:comment xml:lang="en">Policies and processes in use by the service provider to protect the provider
facilities from unauthorized access, damage or interference.</rdfs:comment>
																<skos:definition xml:lang="en">Policies and processes in use by the service provider to protect the provider
facilities from unauthorized access, damage or interference.</skos:definition>
																<ci-onto:defined-in rdf:resource="http://csmic.org/wp-content/uploads/2011/09/SMI-Overview-110913_v1F.pdf" />
																<ci-onto:defined-by rdf:resource="http://purl.org/weso/cloudindex/organization/CSMIC" />
																<ci-onto:weight rdf:datatype="http://www.w3.org/2001/XMLSchema#double">1.0</ci-onto:weight>
																<ci-onto:pref-value rdf:resource="http://purl.org/weso/cloudindex/ontology/High" />
																<skos:notation>EnvironmentSecurity</skos:notation>
																<time:intervalStarts rdf:datatype="http://www.w3.org/2001/XMLSchema#int">2013</time:intervalStarts>
																<time:intervalFinishes rdf:datatype="http://www.w3.org/2001/XMLSchema#int">2013</time:intervalFinishes>
																<skos:broader rdf:resource="http://purl.org/weso/cloudindex/component/SecurityPrivacy" />
															</ci-onto:KPIIndicator>
														</rdfindex:dataset>
														<rdfindex:weight rdf:datatype="http://www.w3.org/2001/XMLSchema#double">0.1</rdfindex:weight>
													</rdf:Description>
												</rdfindex:part-of>
												<rdfindex:part-of>
													<rdf:Description>
														<rdfindex:dataset>
															<ci-onto:KPIIndicator rdf:about="http://purl.org/weso/cloudindex/indicator/ProactiveThreat">
																<rdfs:label xml:lang="en">Proactive Threat &amp;  Vulnerability Management</rdfs:label>
																<rdfs:comment xml:lang="en">Mechanisms in place to ensure that the service is protected against know
recurring threats as well as new evolving vulnerabilities.</rdfs:comment>
																<skos:definition xml:lang="en">Mechanisms in place to ensure that the service is protected against know
recurring threats as well as new evolving vulnerabilities.</skos:definition>
																<ci-onto:defined-in rdf:resource="http://csmic.org/wp-content/uploads/2011/09/SMI-Overview-110913_v1F.pdf" />
																<ci-onto:defined-by rdf:resource="http://purl.org/weso/cloudindex/organization/CSMIC" />
																<ci-onto:weight rdf:datatype="http://www.w3.org/2001/XMLSchema#double">1.0</ci-onto:weight>
																<ci-onto:pref-value rdf:resource="http://purl.org/weso/cloudindex/ontology/High" />
																<skos:notation>ProactiveThreat</skos:notation>
																<time:intervalStarts rdf:datatype="http://www.w3.org/2001/XMLSchema#int">2013</time:intervalStarts>
																<time:intervalFinishes rdf:datatype="http://www.w3.org/2001/XMLSchema#int">2013</time:intervalFinishes>
																<skos:broader rdf:resource="http://purl.org/weso/cloudindex/component/SecurityPrivacy" />
															</ci-onto:KPIIndicator>
														</rdfindex:dataset>
														<rdfindex:weight rdf:datatype="http://www.w3.org/2001/XMLSchema#double">0.1</rdfindex:weight>
													</rdf:Description>
												</rdfindex:part-of>
												<rdfindex:part-of>
													<rdf:Description>
														<rdfindex:dataset>
															<ci-onto:KPIIndicator rdf:about="http://purl.org/weso/cloudindex/indicator/Retention">
																<rdfs:label xml:lang="en">Retention/Disposition</rdfs:label>
																<rdfs:comment xml:lang="en">The service providers data retention and disposition processes meet the clients'
 requirements.</rdfs:comment>
																<skos:definition xml:lang="en">The service providers data retention and disposition processes meet the clients'
 requirements.</skos:definition>
																<ci-onto:defined-in rdf:resource="http://csmic.org/wp-content/uploads/2011/09/SMI-Overview-110913_v1F.pdf" />
																<ci-onto:defined-by rdf:resource="http://purl.org/weso/cloudindex/organization/CSMIC" />
																<ci-onto:weight rdf:datatype="http://www.w3.org/2001/XMLSchema#double">1.0</ci-onto:weight>
																<ci-onto:pref-value rdf:resource="http://purl.org/weso/cloudindex/ontology/High" />
																<skos:notation>Retention</skos:notation>
																<time:intervalStarts rdf:datatype="http://www.w3.org/2001/XMLSchema#int">2013</time:intervalStarts>
																<time:intervalFinishes rdf:datatype="http://www.w3.org/2001/XMLSchema#int">2013</time:intervalFinishes>
																<skos:broader rdf:resource="http://purl.org/weso/cloudindex/component/SecurityPrivacy" />
															</ci-onto:KPIIndicator>
														</rdfindex:dataset>
														<rdfindex:weight rdf:datatype="http://www.w3.org/2001/XMLSchema#double">0.1</rdfindex:weight>
													</rdf:Description>
												</rdfindex:part-of>
												<rdfindex:part-of>
													<rdf:Description>
														<rdfindex:dataset>
															<ci-onto:KPIIndicator rdf:about="http://purl.org/weso/cloudindex/indicator/Disposition">
																<rdfs:label xml:lang="en">Retention/Disposition</rdfs:label>
																<rdfs:comment xml:lang="en">The service providers data retention and disposition processes meet the clients'
 requirements.</rdfs:comment>
																<skos:definition xml:lang="en">The service providers data retention and disposition processes meet the clients'
 requirements.</skos:definition>
																<ci-onto:defined-in rdf:resource="http://csmic.org/wp-content/uploads/2011/09/SMI-Overview-110913_v1F.pdf" />
																<ci-onto:defined-by rdf:resource="http://purl.org/weso/cloudindex/organization/CSMIC" />
																<ci-onto:weight rdf:datatype="http://www.w3.org/2001/XMLSchema#double">1.0</ci-onto:weight>
																<ci-onto:pref-value rdf:resource="http://purl.org/weso/cloudindex/ontology/High" />
																<skos:notation>Disposition</skos:notation>
																<time:intervalStarts rdf:datatype="http://www.w3.org/2001/XMLSchema#int">2013</time:intervalStarts>
																<time:intervalFinishes rdf:datatype="http://www.w3.org/2001/XMLSchema#int">2013</time:intervalFinishes>
																<skos:broader rdf:resource="http://purl.org/weso/cloudindex/component/SecurityPrivacy" />
															</ci-onto:KPIIndicator>
														</rdfindex:dataset>
														<rdfindex:weight rdf:datatype="http://www.w3.org/2001/XMLSchema#double">0.1</rdfindex:weight>
													</rdf:Description>
												</rdfindex:part-of>
											</rdf:Description>
										</rdfindex:aggregates>
										<qb:structure rdf:resource="http://purl.org/weso/cloudindex/SecurityPrivacyDSD" />
										<skos:narrower rdf:resource="http://purl.org/weso/cloudindex/indicator/AccessControl" />
										<skos:narrower rdf:resource="http://purl.org/weso/cloudindex/indicator/GeographicalConstraint" />
										<skos:narrower rdf:resource="http://purl.org/weso/cloudindex/indicator/PoliticalConstraint" />
										<skos:narrower rdf:resource="http://purl.org/weso/cloudindex/indicator/DataIntegrity" />
										<skos:narrower rdf:resource="http://purl.org/weso/cloudindex/indicator/DataPrivacy" />
										<skos:narrower rdf:resource="http://purl.org/weso/cloudindex/indicator/DataLoss" />
										<skos:narrower rdf:resource="http://purl.org/weso/cloudindex/indicator/EnvironmentSecurity" />
										<skos:narrower rdf:resource="http://purl.org/weso/cloudindex/indicator/ProactiveThreat" />
										<skos:narrower rdf:resource="http://purl.org/weso/cloudindex/indicator/Retention" />
										<skos:narrower rdf:resource="http://purl.org/weso/cloudindex/indicator/Disposition" />
									</rdfindex:Component>
								</rdfindex:dataset>
								<rdfindex:weight rdf:datatype="http://www.w3.org/2001/XMLSchema#double">0.14</rdfindex:weight>
							</rdf:Description>
						</rdfindex:part-of>
						<rdfindex:part-of>
							<rdf:Description>
								<rdfindex:dataset>
									<rdfindex:Component rdf:about="http://purl.org/weso/cloudindex/component/Usability">
										<rdfs:label xml:lang="en">Usability</rdfs:label>
										<rdfs:comment xml:lang="en">The ease with which a service can be used.</rdfs:comment>
										<ci-onto:defined-in rdf:resource="http://csmic.org/wp-content/uploads/2011/09/SMI-Overview-110913_v1F.pdf" />
										<ci-onto:defined-by rdf:resource="http://purl.org/weso/cloudindex/organization/CSMIC" />
										<ci-onto:weight rdf:datatype="http://www.w3.org/2001/XMLSchema#double">1</ci-onto:weight>
										<rdfindex:aggregates>
											<rdf:Description>
												<rdfindex:aggregation-operator rdf:resource="http://purl.org/weso/rdfindex/ontology/OWA" />
												<rdfindex:part-of>
													<rdf:Description>
														<rdfindex:dataset>
															<ci-onto:KPIIndicator rdf:about="http://purl.org/weso/cloudindex/indicator/Accessibility">
																<rdfs:label xml:lang="en">Accessibility</rdfs:label>
																<rdfs:comment xml:lang="en">The degree to which a service is operable by users with disabilities.</rdfs:comment>
																<skos:definition xml:lang="en">The degree to which a service is operable by users with disabilities.</skos:definition>
																<ci-onto:defined-in rdf:resource="http://csmic.org/wp-content/uploads/2011/09/SMI-Overview-110913_v1F.pdf" />
																<ci-onto:defined-by rdf:resource="http://purl.org/weso/cloudindex/organization/CSMIC" />
																<ci-onto:weight rdf:datatype="http://www.w3.org/2001/XMLSchema#double">1.0</ci-onto:weight>
																<ci-onto:pref-value rdf:resource="http://purl.org/weso/cloudindex/ontology/High" />
																<skos:notation>Accessibility</skos:notation>
																<time:intervalStarts rdf:datatype="http://www.w3.org/2001/XMLSchema#int">2013</time:intervalStarts>
																<time:intervalFinishes rdf:datatype="http://www.w3.org/2001/XMLSchema#int">2013</time:intervalFinishes>
																<skos:broader rdf:resource="http://purl.org/weso/cloudindex/component/Usability" />
															</ci-onto:KPIIndicator>
														</rdfindex:dataset>
														<rdfindex:weight rdf:datatype="http://www.w3.org/2001/XMLSchema#double">0.125</rdfindex:weight>
													</rdf:Description>
												</rdfindex:part-of>
												<rdfindex:part-of>
													<rdf:Description>
														<rdfindex:dataset>
															<ci-onto:KPIIndicator rdf:about="http://purl.org/weso/cloudindex/indicator/ClientPersonnelRequirements">
																<rdfs:label xml:lang="en">Client Personnel Requirements</rdfs:label>
																<rdfs:comment xml:lang="en">The minimum number of personnel satisfying roles, skills, experience, education,
and certification required of the client to effectively utilize a service.</rdfs:comment>
																<skos:definition xml:lang="en">The minimum number of personnel satisfying roles, skills, experience, education,
and certification required of the client to effectively utilize a service.</skos:definition>
																<ci-onto:defined-in rdf:resource="http://csmic.org/wp-content/uploads/2011/09/SMI-Overview-110913_v1F.pdf" />
																<ci-onto:defined-by rdf:resource="http://purl.org/weso/cloudindex/organization/CSMIC" />
																<ci-onto:weight rdf:datatype="http://www.w3.org/2001/XMLSchema#double">1.0</ci-onto:weight>
																<ci-onto:pref-value rdf:resource="http://purl.org/weso/cloudindex/ontology/High" />
																<skos:notation>ClientPersonnelRequirements</skos:notation>
																<time:intervalStarts rdf:datatype="http://www.w3.org/2001/XMLSchema#int">2013</time:intervalStarts>
																<time:intervalFinishes rdf:datatype="http://www.w3.org/2001/XMLSchema#int">2013</time:intervalFinishes>
																<skos:broader rdf:resource="http://purl.org/weso/cloudindex/component/Usability" />
															</ci-onto:KPIIndicator>
														</rdfindex:dataset>
														<rdfindex:weight rdf:datatype="http://www.w3.org/2001/XMLSchema#double">0.125</rdfindex:weight>
													</rdf:Description>
												</rdfindex:part-of>
												<rdfindex:part-of>
													<rdf:Description>
														<rdfindex:dataset>
															<ci-onto:KPIIndicator rdf:about="http://purl.org/weso/cloudindex/indicator/Installability">
																<rdfs:label xml:lang="en">Client Personnel Requirements</rdfs:label>
																<rdfs:comment xml:lang="en">Installability characterizes the time and effort required to get a service ready for
delivery (where applicable).</rdfs:comment>
																<skos:definition xml:lang="en">Installability characterizes the time and effort required to get a service ready for
delivery (where applicable).</skos:definition>
																<ci-onto:defined-in rdf:resource="http://csmic.org/wp-content/uploads/2011/09/SMI-Overview-110913_v1F.pdf" />
																<ci-onto:defined-by rdf:resource="http://purl.org/weso/cloudindex/organization/CSMIC" />
																<ci-onto:weight rdf:datatype="http://www.w3.org/2001/XMLSchema#double">1.0</ci-onto:weight>
																<ci-onto:pref-value rdf:resource="http://purl.org/weso/cloudindex/ontology/High" />
																<skos:notation>Installability</skos:notation>
																<time:intervalStarts rdf:datatype="http://www.w3.org/2001/XMLSchema#int">2013</time:intervalStarts>
																<time:intervalFinishes rdf:datatype="http://www.w3.org/2001/XMLSchema#int">2013</time:intervalFinishes>
																<skos:broader rdf:resource="http://purl.org/weso/cloudindex/component/Usability" />
															</ci-onto:KPIIndicator>
														</rdfindex:dataset>
														<rdfindex:weight rdf:datatype="http://www.w3.org/2001/XMLSchema#double">0.125</rdfindex:weight>
													</rdf:Description>
												</rdfindex:part-of>
												<rdfindex:part-of>
													<rdf:Description>
														<rdfindex:dataset>
															<ci-onto:KPIIndicator rdf:about="http://purl.org/weso/cloudindex/indicator/Learnability">
																<rdfs:label xml:lang="en">Learnability</rdfs:label>
																<rdfs:comment xml:lang="en">The effort required of users to learn to use the service.</rdfs:comment>
																<skos:definition xml:lang="en">The effort required of users to learn to use the service.</skos:definition>
																<ci-onto:defined-in rdf:resource="http://csmic.org/wp-content/uploads/2011/09/SMI-Overview-110913_v1F.pdf" />
																<ci-onto:defined-by rdf:resource="http://purl.org/weso/cloudindex/organization/CSMIC" />
																<ci-onto:weight rdf:datatype="http://www.w3.org/2001/XMLSchema#double">1.0</ci-onto:weight>
																<ci-onto:pref-value rdf:resource="http://purl.org/weso/cloudindex/ontology/High" />
																<skos:notation>Learnability</skos:notation>
																<time:intervalStarts rdf:datatype="http://www.w3.org/2001/XMLSchema#int">2013</time:intervalStarts>
																<time:intervalFinishes rdf:datatype="http://www.w3.org/2001/XMLSchema#int">2013</time:intervalFinishes>
																<skos:broader rdf:resource="http://purl.org/weso/cloudindex/component/Usability" />
															</ci-onto:KPIIndicator>
														</rdfindex:dataset>
														<rdfindex:weight rdf:datatype="http://www.w3.org/2001/XMLSchema#double">0.125</rdfindex:weight>
													</rdf:Description>
												</rdfindex:part-of>
												<rdfindex:part-of>
													<rdf:Description>
														<rdfindex:dataset>
															<ci-onto:KPIIndicator rdf:about="http://purl.org/weso/cloudindex/indicator/Operability">
																<rdfs:label xml:lang="en">Operability</rdfs:label>
																<rdfs:comment xml:lang="en">The ability of a service to be easily operated by users.</rdfs:comment>
																<skos:definition xml:lang="en">The ability of a service to be easily operated by users.</skos:definition>
																<ci-onto:defined-in rdf:resource="http://csmic.org/wp-content/uploads/2011/09/SMI-Overview-110913_v1F.pdf" />
																<ci-onto:defined-by rdf:resource="http://purl.org/weso/cloudindex/organization/CSMIC" />
																<ci-onto:weight rdf:datatype="http://www.w3.org/2001/XMLSchema#double">1.0</ci-onto:weight>
																<ci-onto:pref-value rdf:resource="http://purl.org/weso/cloudindex/ontology/High" />
																<skos:notation>Operability</skos:notation>
																<time:intervalStarts rdf:datatype="http://www.w3.org/2001/XMLSchema#int">2013</time:intervalStarts>
																<time:intervalFinishes rdf:datatype="http://www.w3.org/2001/XMLSchema#int">2013</time:intervalFinishes>
																<skos:broader rdf:resource="http://purl.org/weso/cloudindex/component/Usability" />
															</ci-onto:KPIIndicator>
														</rdfindex:dataset>
														<rdfindex:weight rdf:datatype="http://www.w3.org/2001/XMLSchema#double">0.125</rdfindex:weight>
													</rdf:Description>
												</rdfindex:part-of>
												<rdfindex:part-of>
													<rdf:Description>
														<rdfindex:dataset rdf:resource="http://purl.org/weso/cloudindex/indicator/Suitability" />
														<rdfindex:weight rdf:datatype="http://www.w3.org/2001/XMLSchema#double">0.125</rdfindex:weight>
													</rdf:Description>
												</rdfindex:part-of>
												<rdfindex:part-of>
													<rdf:Description>
														<rdfindex:dataset>
															<ci-onto:KPIIndicator rdf:about="http://purl.org/weso/cloudindex/indicator/Transparency">
																<rdfs:label xml:lang="en">Transparency</rdfs:label>
																<rdfs:comment xml:lang="en">The extent to which users are able to determine when changes in a feature or component of the service occur and whether these changes impact usability.</rdfs:comment>
																<skos:definition xml:lang="en">The extent to which users are able to determine when changes in a feature or component of the service occur and whether these changes impact usability.</skos:definition>
																<ci-onto:defined-in rdf:resource="http://csmic.org/wp-content/uploads/2011/09/SMI-Overview-110913_v1F.pdf" />
																<ci-onto:defined-by rdf:resource="http://purl.org/weso/cloudindex/organization/CSMIC" />
																<ci-onto:weight rdf:datatype="http://www.w3.org/2001/XMLSchema#double">1.0</ci-onto:weight>
																<ci-onto:pref-value rdf:resource="http://purl.org/weso/cloudindex/ontology/High" />
																<skos:notation>Transparency</skos:notation>
																<time:intervalStarts rdf:datatype="http://www.w3.org/2001/XMLSchema#int">2013</time:intervalStarts>
																<time:intervalFinishes rdf:datatype="http://www.w3.org/2001/XMLSchema#int">2013</time:intervalFinishes>
																<skos:broader rdf:resource="http://purl.org/weso/cloudindex/component/Usability" />
															</ci-onto:KPIIndicator>
														</rdfindex:dataset>
														<rdfindex:weight rdf:datatype="http://www.w3.org/2001/XMLSchema#double">0.125</rdfindex:weight>
													</rdf:Description>
												</rdfindex:part-of>
												<rdfindex:part-of>
													<rdf:Description>
														<rdfindex:dataset>
															<ci-onto:KPIIndicator rdf:about="http://purl.org/weso/cloudindex/indicator/Understandability">
																<rdfs:label xml:lang="en">Understandability</rdfs:label>
																<rdfs:comment xml:lang="en">The ease with which users can understand the capabilities and operation of the service.</rdfs:comment>
																<skos:definition xml:lang="en">The ease with which users can understand the capabilities and operation of the service.</skos:definition>
																<ci-onto:defined-in rdf:resource="http://csmic.org/wp-content/uploads/2011/09/SMI-Overview-110913_v1F.pdf" />
																<ci-onto:defined-by rdf:resource="http://purl.org/weso/cloudindex/organization/CSMIC" />
																<ci-onto:weight rdf:datatype="http://www.w3.org/2001/XMLSchema#double">1.0</ci-onto:weight>
																<ci-onto:pref-value rdf:resource="http://purl.org/weso/cloudindex/ontology/High" />
																<skos:notation>Understandability</skos:notation>
																<time:intervalStarts rdf:datatype="http://www.w3.org/2001/XMLSchema#int">2013</time:intervalStarts>
																<time:intervalFinishes rdf:datatype="http://www.w3.org/2001/XMLSchema#int">2013</time:intervalFinishes>
																<skos:broader rdf:resource="http://purl.org/weso/cloudindex/component/Usability" />
															</ci-onto:KPIIndicator>
														</rdfindex:dataset>
														<rdfindex:weight rdf:datatype="http://www.w3.org/2001/XMLSchema#double">0.125</rdfindex:weight>
													</rdf:Description>
												</rdfindex:part-of>
											</rdf:Description>
										</rdfindex:aggregates>
										<qb:structure rdf:resource="http://purl.org/weso/cloudindex/UsabilityDSD" />
										<skos:narrower rdf:resource="http://purl.org/weso/cloudindex/indicator/Accessibility" />
										<skos:narrower rdf:resource="http://purl.org/weso/cloudindex/indicator/ClientPersonnelRequirements" />
										<skos:narrower rdf:resource="http://purl.org/weso/cloudindex/indicator/Installability" />
										<skos:narrower rdf:resource="http://purl.org/weso/cloudindex/indicator/Learnability" />
										<skos:narrower rdf:resource="http://purl.org/weso/cloudindex/indicator/Operability" />
										<skos:narrower rdf:resource="http://purl.org/weso/cloudindex/indicator/Suitability" />
										<skos:narrower rdf:resource="http://purl.org/weso/cloudindex/indicator/Transparency" />
										<skos:narrower rdf:resource="http://purl.org/weso/cloudindex/indicator/Understandability" />
									</rdfindex:Component>
								</rdfindex:dataset>
								<rdfindex:weight rdf:datatype="http://www.w3.org/2001/XMLSchema#double">0.14</rdfindex:weight>
							</rdf:Description>
						</rdfindex:part-of>
					</rdf:Description>
				</rdfindex:aggregates>
				<qb:structure rdf:resource="http://purl.org/weso/cloudindex/CloundIndexDSD" />
				<skos:narrower rdf:resource="http://purl.org/weso/cloudindex/component/Accountability" />
				<skos:narrower rdf:resource="http://purl.org/weso/cloudindex/component/Agility" />
				<skos:narrower rdf:resource="http://purl.org/weso/cloudindex/component/Assurance" />
				<skos:narrower rdf:resource="http://purl.org/weso/cloudindex/component/Financial" />
				<skos:narrower rdf:resource="http://purl.org/weso/cloudindex/component/Performance" />
				<skos:narrower rdf:resource="http://purl.org/weso/cloudindex/component/SecurityPrivacy" />
				<skos:narrower rdf:resource="http://purl.org/weso/cloudindex/component/Usability" />
			</rdfindex:Index>
		</rdfs:seeAlso>
		<rdfs:seeAlso>
			<void:Dataset rdf:about="http://purl.org/weso/cloudindex/component/ds">
				<rdfs:label xml:lang="en">SEERC| CloudIndex | Components</rdfs:label>
				<rdfs:comment xml:lang="en">Dataset of components that aggregates different indicators and are part of a subindex.</rdfs:comment>
				<dcterms:created rdf:datatype="http://www.w3.org/2001/XMLSchema#date">2012-20-05</dcterms:created>
				<dcterms:modified rdf:datatype="http://www.w3.org/2001/XMLSchema#date">2012-08-31</dcterms:modified>
				<dcterms:title xml:lang="en">Core CloudIndex ontology</dcterms:title>
				<dcterms:author rdf:resource="http://purl.org/weso/cloudindex/people/Chema" />
				<dcterms:author rdf:resource="http://purl.org/weso/rdfindex/organization/SEERC" />
				<dcterms:publisher rdf:resource="http://purl.org/weso/cloudindex/people/Chema" />
				<dcterms:contributor rdf:resource="http://purl.org/weso/rdfindex/organization/SEERC" />
				<dcterms:contributor rdf:resource="http://purl.org/weso/rdfindex/project/RELATE" />
				<dcterms:license rdf:resource="http://opendatacommons.org/licenses/by/1.0/" />
				<void:exampleResource rdf:resource="http://purl.org/weso/cloudindex/component/Accountability" />
				<void:uriRegexPattern>http://purl.org/weso/cloudindex/component/.+</void:uriRegexPattern>
				<void:vocabulary rdf:resource="http://www.w3.org/2000/01/rdf-schema#" />
				<void:vocabulary rdf:resource="http://www.w3.org/2004/02/skos/core#" />
				<foaf:homepage rdf:resource="http://purl.org/weso/cloudindex/" />
			</void:Dataset>
		</rdfs:seeAlso>
		<rdfs:seeAlso>
			<void:Dataset rdf:about="http://purl.org/weso/cloudindex/indicator/ds">
				<rdfs:label xml:lang="en">SEERC| CloudIndex | Indicators</rdfs:label>
				<rdfs:comment xml:lang="en">Indicators used to retrieve observations according to the different dimensions. They can also be taken as measures.</rdfs:comment>
				<dcterms:created rdf:datatype="http://www.w3.org/2001/XMLSchema#date">2013-05-20</dcterms:created>
				<dcterms:modified rdf:datatype="http://www.w3.org/2001/XMLSchema#date">2013-06-20-</dcterms:modified>
				<dcterms:title xml:lang="en">Indicators of Core CloudIndex ontology</dcterms:title>
				<dcterms:author rdf:resource="http://purl.org/weso/cloudindex/people/Chema" />
				<dcterms:author rdf:resource="http://purl.org/weso/rdfindex/organization/SEERC" />
				<dcterms:publisher rdf:resource="http://purl.org/weso/cloudindex/people/Chema" />
				<dcterms:contributor rdf:resource="http://purl.org/weso/rdfindex/organization/SEERC" />
				<dcterms:contributor rdf:resource="http://purl.org/weso/rdfindex/project/RELATE" />
				<dcterms:license rdf:resource="http://opendatacommons.org/licenses/by/1.0/" />
				<void:exampleResource rdf:resource="http://purl.org/weso/cloudindex/component/CommunicationsInfrastructure" />
				<void:uriRegexPattern>http://purl.org/weso/cloudindex/indicator/.+</void:uriRegexPattern>
				<void:vocabulary rdf:resource="http://www.w3.org/2000/01/rdf-schema#" />
				<void:vocabulary rdf:resource="http://www.w3.org/2004/02/skos/core#" />
				<foaf:homepage rdf:resource="http://purl.org/weso/cloudindex/" />
			</void:Dataset>
		</rdfs:seeAlso>
		<rdfs:seeAlso>
			<void:Dataset rdf:about="http://purl.org/weso/cloudindex/organization/ds">
				<rdfs:label xml:lang="en">SEERC | Cloud Index | Organizations</rdfs:label>
				<dcterms:created rdf:datatype="http://www.w3.org/2001/XMLSchema#date">2012-20-05</dcterms:created>
				<dcterms:modified rdf:datatype="http://www.w3.org/2001/XMLSchema#date">2012-08-31</dcterms:modified>
				<dcterms:title xml:lang="en">Organizations dataset involved in the development of Core CloudIndex ontology</dcterms:title>
				<dcterms:author rdf:resource="http://purl.org/weso/cloudindex/people/Chema" />
				<dcterms:author rdf:resource="http://purl.org/weso/rdfindex/organization/SEERC" />
				<dcterms:publisher rdf:resource="http://purl.org/weso/cloudindex/people/Chema" />
				<dcterms:contributor rdf:resource="http://purl.org/weso/rdfindex/organization/SEERC" />
				<dcterms:contributor rdf:resource="http://purl.org/weso/rdfindex/project/RELATE" />
				<dcterms:license rdf:resource="http://opendatacommons.org/licenses/by/1.0/" />
				<void:exampleResource rdf:resource="http://purl.org/weso/cloudindex/organization/CSMIC" />
				<void:uriRegexPattern>http://purl.org/weso/cloudindex/organization/.+</void:uriRegexPattern>
				<void:vocabulary rdf:resource="http://www.w3.org/2000/01/rdf-schema#" />
				<void:vocabulary rdf:resource="http://xmlns.com/foaf/0.1/" />
				<foaf:homepage rdf:resource="http://purl.org/weso/cloudindex/" />
			</void:Dataset>
		</rdfs:seeAlso>
		<dcterms:modified rdf:datatype="http://www.w3.org/2001/XMLSchema#date">2012-06-20</dcterms:modified>
		<dcterms:title xml:lang="en">The CloudIndex structure</dcterms:title>
		<dcterms:author rdf:resource="http://purl.org/weso/cloudindex/people/Chema" />
		<dcterms:author rdf:resource="http://purl.org/weso/rdfindex/organization/SEERC" />
		<dcterms:publisher rdf:resource="http://purl.org/weso/cloudindex/people/Chema" />
		<dcterms:contributor rdf:resource="http://purl.org/weso/rdfindex/organization/SEERC" />
		<dcterms:contributor rdf:resource="http://purl.org/weso/rdfindex/project/RELATE" />
		<dcterms:license rdf:resource="http://opendatacommons.org/licenses/by/1.0/" />
	</owl:Ontology>
	<owl:Class rdf:about="http://purl.org/weso/cloudindex/ontology/KPIIndicator">
		<rdf:type rdf:resource="http://www.w3.org/2000/01/rdf-schema#Class" />
		<rdfs:subClassOf rdf:resource="http://purl.org/weso/rdfindex/ontology/Indicator" />
		<rdfs:label xml:lang="en">KPI Indicator</rdfs:label>
		<rdfs:comment xml:lang="en">Key Performance Indicator.</rdfs:comment>
	</owl:Class>
	<rdf:Property rdf:about="http://purl.org/weso/cloudindex/ontology/ref-area">
		<rdf:type rdf:resource="http://purl.org/linked-data/cube#DimensionProperty" />
		<rdfs:label xml:lang="en">URI to an Area</rdfs:label>
		<rdfs:subPropertyOf rdf:resource="http://purl.org/linked-data/sdmx/2009/dimension#ref-area" />
		<rdfs:range rdf:resource="http://www.w3.org/2004/02/skos/core#Concept" />
		<qb:concept rdf:resource="http://purl.org/linked-data/sdmx/2009/concept#ref-area" />
	</rdf:Property>
	<rdf:Property rdf:about="http://purl.org/weso/cloudindex/ontology/ref-provider">
		<rdf:type rdf:resource="http://purl.org/linked-data/cube#DimensionProperty" />
		<rdfs:label xml:lang="en">URI to a provider</rdfs:label>
		<rdfs:subPropertyOf rdf:resource="http://purl.org/linked-data/sdmx/2009/dimension#ref-area" />
		<rdfs:range rdf:resource="http://www.w3.org/2004/02/skos/core#Concept" />
		<qb:concept rdf:resource="http://purl.org/linked-data/sdmx/2009/concept#ref-area" />
	</rdf:Property>
	<rdf:Property rdf:about="http://purl.org/weso/cloudindex/ontology/ref-year">
		<rdf:type rdf:resource="http://purl.org/linked-data/cube#DimensionProperty" />
		<rdfs:label xml:lang="en">Period and year</rdfs:label>
		<rdfs:subPropertyOf rdf:resource="http://purl.org/linked-data/sdmx/2009/dimension#ref-period" />
		<rdfs:range rdf:resource="http://www.w3.org/2006/time#Interval" />
		<qb:concept rdf:resource="http://purl.org/linked-data/sdmx/2009/concept#ref-period" />
	</rdf:Property>
	<rdf:Property rdf:about="http://purl.org/weso/cloudindex/ontology/ref-period">
		<rdf:type rdf:resource="http://purl.org/linked-data/cube#DimensionProperty" />
		<rdfs:label xml:lang="en">Period</rdfs:label>
		<rdfs:subPropertyOf rdf:resource="http://purl.org/linked-data/sdmx/2009/dimension#ref-period" />
		<rdfs:range rdf:resource="http://www.w3.org/2006/time#Interval" />
		<qb:concept rdf:resource="http://purl.org/linked-data/sdmx/2009/concept#ref-period" />
	</rdf:Property>
	<owl:ObjectProperty rdf:about="http://purl.org/weso/cloudindex/ontology/value">
		<rdf:type rdf:resource="http://purl.org/linked-data/cube#MeasureProperty" />
		<rdfs:label xml:lang="en">Observation's value</rdfs:label>
		<rdfs:comment xml:lang="en">Values should be accessed through a proxy class</rdfs:comment>
		<rdfs:subPropertyOf rdf:resource="http://purl.org/linked-data/sdmx/2009/measure#obsValue" />
	</owl:ObjectProperty>
	<owl:ObjectProperty rdf:about="http://purl.org/weso/cloudindex/ontology/timestamp">
		<rdf:type rdf:resource="http://www.w3.org/1999/02/22-rdf-syntax-ns#Property" />
		<rdfs:label xml:lang="en">Timestamp of an observation</rdfs:label>
		<rdfs:comment xml:lang="en">It is used to specify the precise moment in which the observation has been generated.</rdfs:comment>
	</owl:ObjectProperty>
	<owl:ObjectProperty rdf:about="http://purl.org/weso/cloudindex/ontology/pref-value">
		<rdf:type rdf:resource="http://www.w3.org/1999/02/22-rdf-syntax-ns#Property" />
		<rdfs:label xml:lang="en">Preferred  value</rdfs:label>
		<rdfs:domain rdf:resource="http://www.w3.org/2004/02/skos/core#Concept" />
		<rdfs:range rdf:resource="http://www.w3.org/2004/02/skos/core#Concept" />
		<rdfs:comment xml:lang="en">It is used to specify when a value is better.</rdfs:comment>
	</owl:ObjectProperty>
	<owl:ObjectProperty rdf:about="http://purl.org/weso/cloudindex/ontology/defined-by">
		<rdf:type rdf:resource="http://www.w3.org/1999/02/22-rdf-syntax-ns#Property" />
		<rdfs:subPropertyOf rdf:resource="http://purl.org/dc/terms/source" />
		<rdfs:label xml:lang="en">provider-link</rdfs:label>
		<rdfs:comment xml:lang="en">URI to the provider of a definition</rdfs:comment>
	</owl:ObjectProperty>
</rdf:RDF>
The underlying triples

<http://purl.org/weso/cloudindex/ontology/> <http://www.w3.org/1999/02/22-rdf-syntax-ns#type> <http://www.w3.org/2002/07/owl#Ontology>.
<http://purl.org/weso/cloudindex/ontology/> <http://www.w3.org/2002/07/owl#versionInfo> "0.1".
<http://purl.org/weso/cloudindex/ontology/> <http://www.w3.org/2000/01/rdf-schema#label> "Core Cloud Index structure and computation process"@en.
<http://purl.org/weso/cloudindex/ontology/> <http://www.w3.org/2000/01/rdf-schema#comment> "This is the first version of the The CloudIndex taxonomy for representing QoS indicators and modeling an index."@en.
<http://purl.org/weso/cloudindex/ontology/> <http://purl.org/dc/terms/created> "2012-05-20"^^<http://www.w3.org/2001/XMLSchema#date>.
<http://purl.org/weso/cloudindex/ontology/> <http://www.w3.org/2000/01/rdf-schema#seeAlso> <http://purl.org/weso/rdfindex/ontology/>.
<http://purl.org/weso/cloudindex/ontology/> <http://www.w3.org/2000/01/rdf-schema#seeAlso> <http://purl.org/weso/cloudindex/index>.
<http://purl.org/weso/cloudindex/ontology/> <http://www.w3.org/2000/01/rdf-schema#seeAlso> <http://purl.org/weso/cloudindex/component/ds>.
<http://purl.org/weso/cloudindex/ontology/> <http://www.w3.org/2000/01/rdf-schema#seeAlso> <http://purl.org/weso/cloudindex/indicator/ds>.
<http://purl.org/weso/cloudindex/ontology/> <http://www.w3.org/2000/01/rdf-schema#seeAlso> <http://purl.org/weso/cloudindex/organization/ds>.
<http://purl.org/weso/cloudindex/ontology/> <http://purl.org/dc/terms/modified> "2012-06-20"^^<http://www.w3.org/2001/XMLSchema#date>.
<http://purl.org/weso/cloudindex/ontology/> <http://purl.org/dc/terms/title> "The CloudIndex structure"@en.
<http://purl.org/weso/cloudindex/ontology/> <http://purl.org/dc/terms/author> <http://purl.org/weso/cloudindex/people/Chema>.
<http://purl.org/weso/cloudindex/ontology/> <http://purl.org/dc/terms/author> <http://purl.org/weso/rdfindex/organization/SEERC>.
<http://purl.org/weso/cloudindex/ontology/> <http://purl.org/dc/terms/publisher> <http://purl.org/weso/cloudindex/people/Chema>.
<http://purl.org/weso/cloudindex/ontology/> <http://purl.org/dc/terms/contributor> <http://purl.org/weso/rdfindex/organization/SEERC>.
<http://purl.org/weso/cloudindex/ontology/> <http://purl.org/dc/terms/contributor> <http://purl.org/weso/rdfindex/project/RELATE>.
<http://purl.org/weso/cloudindex/ontology/> <http://purl.org/dc/terms/license> <http://opendatacommons.org/licenses/by/1.0/>.
<http://purl.org/weso/cloudindex/ontology/KPIIndicator> <http://www.w3.org/1999/02/22-rdf-syntax-ns#type> <http://www.w3.org/2002/07/owl#Class>.
<http://purl.org/weso/cloudindex/ontology/KPIIndicator> <http://www.w3.org/1999/02/22-rdf-syntax-ns#type> <http://www.w3.org/2000/01/rdf-schema#Class>.
<http://purl.org/weso/cloudindex/ontology/KPIIndicator> <http://www.w3.org/2000/01/rdf-schema#subClassOf> <http://purl.org/weso/rdfindex/ontology/Indicator>.
<http://purl.org/weso/cloudindex/ontology/KPIIndicator> <http://www.w3.org/2000/01/rdf-schema#label> "KPI Indicator"@en.
<http://purl.org/weso/cloudindex/ontology/KPIIndicator> <http://www.w3.org/2000/01/rdf-schema#comment> "Key Performance Indicator."@en.
<http://purl.org/weso/cloudindex/ontology/ref-area> <http://www.w3.org/1999/02/22-rdf-syntax-ns#type> <http://www.w3.org/1999/02/22-rdf-syntax-ns#Property>.
<http://purl.org/weso/cloudindex/ontology/ref-area> <http://www.w3.org/1999/02/22-rdf-syntax-ns#type> <http://purl.org/linked-data/cube#DimensionProperty>.
<http://purl.org/weso/cloudindex/ontology/ref-area> <http://www.w3.org/2000/01/rdf-schema#label> "URI to an Area"@en.
<http://purl.org/weso/cloudindex/ontology/ref-area> <http://www.w3.org/2000/01/rdf-schema#subPropertyOf> <http://purl.org/linked-data/sdmx/2009/dimension#ref-area>.
<http://purl.org/weso/cloudindex/ontology/ref-area> <http://www.w3.org/2000/01/rdf-schema#range> <http://www.w3.org/2004/02/skos/core#Concept>.
<http://purl.org/weso/cloudindex/ontology/ref-area> <http://purl.org/linked-data/cube#concept> <http://purl.org/linked-data/sdmx/2009/concept#ref-area>.
<http://purl.org/weso/cloudindex/ontology/ref-provider> <http://www.w3.org/1999/02/22-rdf-syntax-ns#type> <http://www.w3.org/1999/02/22-rdf-syntax-ns#Property>.
<http://purl.org/weso/cloudindex/ontology/ref-provider> <http://www.w3.org/1999/02/22-rdf-syntax-ns#type> <http://purl.org/linked-data/cube#DimensionProperty>.
<http://purl.org/weso/cloudindex/ontology/ref-provider> <http://www.w3.org/2000/01/rdf-schema#label> "URI to a provider"@en.
<http://purl.org/weso/cloudindex/ontology/ref-provider> <http://www.w3.org/2000/01/rdf-schema#subPropertyOf> <http://purl.org/linked-data/sdmx/2009/dimension#ref-area>.
<http://purl.org/weso/cloudindex/ontology/ref-provider> <http://www.w3.org/2000/01/rdf-schema#range> <http://www.w3.org/2004/02/skos/core#Concept>.
<http://purl.org/weso/cloudindex/ontology/ref-provider> <http://purl.org/linked-data/cube#concept> <http://purl.org/linked-data/sdmx/2009/concept#ref-area>.
<http://purl.org/weso/cloudindex/ontology/ref-year> <http://www.w3.org/1999/02/22-rdf-syntax-ns#type> <http://www.w3.org/1999/02/22-rdf-syntax-ns#Property>.
<http://purl.org/weso/cloudindex/ontology/ref-year> <http://www.w3.org/1999/02/22-rdf-syntax-ns#type> <http://purl.org/linked-data/cube#DimensionProperty>.
<http://purl.org/weso/cloudindex/ontology/ref-year> <http://www.w3.org/2000/01/rdf-schema#label> "Period and year"@en.
<http://purl.org/weso/cloudindex/ontology/ref-year> <http://www.w3.org/2000/01/rdf-schema#subPropertyOf> <http://purl.org/linked-data/sdmx/2009/dimension#ref-period>.
<http://purl.org/weso/cloudindex/ontology/ref-year> <http://www.w3.org/2000/01/rdf-schema#range> <http://www.w3.org/2006/time#Interval>.
<http://purl.org/weso/cloudindex/ontology/ref-year> <http://purl.org/linked-data/cube#concept> <http://purl.org/linked-data/sdmx/2009/concept#ref-period>.
<http://purl.org/weso/cloudindex/ontology/ref-period> <http://www.w3.org/1999/02/22-rdf-syntax-ns#type> <http://www.w3.org/1999/02/22-rdf-syntax-ns#Property>.
<http://purl.org/weso/cloudindex/ontology/ref-period> <http://www.w3.org/1999/02/22-rdf-syntax-ns#type> <http://purl.org/linked-data/cube#DimensionProperty>.
<http://purl.org/weso/cloudindex/ontology/ref-period> <http://www.w3.org/2000/01/rdf-schema#label> "Period"@en.
<http://purl.org/weso/cloudindex/ontology/ref-period> <http://www.w3.org/2000/01/rdf-schema#subPropertyOf> <http://purl.org/linked-data/sdmx/2009/dimension#ref-period>.
<http://purl.org/weso/cloudindex/ontology/ref-period> <http://www.w3.org/2000/01/rdf-schema#range> <http://www.w3.org/2006/time#Interval>.
<http://purl.org/weso/cloudindex/ontology/ref-period> <http://purl.org/linked-data/cube#concept> <http://purl.org/linked-data/sdmx/2009/concept#ref-period>.
<http://purl.org/weso/cloudindex/ontology/value> <http://www.w3.org/1999/02/22-rdf-syntax-ns#type> <http://www.w3.org/2002/07/owl#ObjectProperty>.
<http://purl.org/weso/cloudindex/ontology/value> <http://www.w3.org/1999/02/22-rdf-syntax-ns#type> <http://purl.org/linked-data/cube#MeasureProperty>.
<http://purl.org/weso/cloudindex/ontology/value> <http://www.w3.org/2000/01/rdf-schema#label> "Observation's value"@en.
<http://purl.org/weso/cloudindex/ontology/value> <http://www.w3.org/2000/01/rdf-schema#comment> "Values should be accessed through a proxy class"@en.
<http://purl.org/weso/cloudindex/ontology/value> <http://www.w3.org/2000/01/rdf-schema#subPropertyOf> <http://purl.org/linked-data/sdmx/2009/measure#obsValue>.
<http://purl.org/weso/cloudindex/ontology/timestamp> <http://www.w3.org/1999/02/22-rdf-syntax-ns#type> <http://www.w3.org/2002/07/owl#ObjectProperty>.
<http://purl.org/weso/cloudindex/ontology/timestamp> <http://www.w3.org/1999/02/22-rdf-syntax-ns#type> <http://www.w3.org/1999/02/22-rdf-syntax-ns#Property>.
<http://purl.org/weso/cloudindex/ontology/timestamp> <http://www.w3.org/2000/01/rdf-schema#label> "Timestamp of an observation"@en.
<http://purl.org/weso/cloudindex/ontology/timestamp> <http://www.w3.org/2000/01/rdf-schema#comment> "It is used to specify the precise moment in which the observation has been generated."@en.
<http://purl.org/weso/cloudindex/ontology/pref-value> <http://www.w3.org/1999/02/22-rdf-syntax-ns#type> <http://www.w3.org/2002/07/owl#ObjectProperty>.
<http://purl.org/weso/cloudindex/ontology/pref-value> <http://www.w3.org/1999/02/22-rdf-syntax-ns#type> <http://www.w3.org/1999/02/22-rdf-syntax-ns#Property>.
<http://purl.org/weso/cloudindex/ontology/pref-value> <http://www.w3.org/2000/01/rdf-schema#label> "Preferred  value"@en.
<http://purl.org/weso/cloudindex/ontology/pref-value> <http://www.w3.org/2000/01/rdf-schema#domain> <http://www.w3.org/2004/02/skos/core#Concept>.
<http://purl.org/weso/cloudindex/ontology/pref-value> <http://www.w3.org/2000/01/rdf-schema#range> <http://www.w3.org/2004/02/skos/core#Concept>.
<http://purl.org/weso/cloudindex/ontology/pref-value> <http://www.w3.org/2000/01/rdf-schema#comment> "It is used to specify when a value is better."@en.
<http://purl.org/weso/cloudindex/ontology/defined-by> <http://www.w3.org/1999/02/22-rdf-syntax-ns#type> <http://www.w3.org/2002/07/owl#ObjectProperty>.
<http://purl.org/weso/cloudindex/ontology/defined-by> <http://www.w3.org/1999/02/22-rdf-syntax-ns#type> <http://www.w3.org/1999/02/22-rdf-syntax-ns#Property>.
<http://purl.org/weso/cloudindex/ontology/defined-by> <http://www.w3.org/2000/01/rdf-schema#subPropertyOf> <http://purl.org/dc/terms/source>.
<http://purl.org/weso/cloudindex/ontology/defined-by> <http://www.w3.org/2000/01/rdf-schema#label> "provider-link"@en.
<http://purl.org/weso/cloudindex/ontology/defined-by> <http://www.w3.org/2000/01/rdf-schema#comment> "URI to the provider of a definition"@en.
<http://purl.org/weso/cloudindex/index> <http://www.w3.org/1999/02/22-rdf-syntax-ns#type> <http://purl.org/weso/rdfindex/ontology/Index>.
<http://purl.org/weso/cloudindex/index> <http://www.w3.org/2000/01/rdf-schema#label> "The CloudIndex"@en.
<http://purl.org/weso/cloudindex/index> <http://www.w3.org/2000/01/rdf-schema#comment> "The index of components"@en.
<http://purl.org/weso/cloudindex/index> <http://purl.org/weso/cloudindex/ontology/defined-in> <http://csmic.org/wp-content/uploads/2011/09/SMI-Overview-110913_v1F.pdf>.
<http://purl.org/weso/cloudindex/index> <http://purl.org/weso/cloudindex/ontology/defined-by> <http://purl.org/weso/cloudindex/organization/CSMIC>.
_:bnode134673728 <http://purl.org/weso/rdfindex/ontology/aggregation-operator> <http://purl.org/weso/rdfindex/ontology/OWA>.
_:bnode653393792 <http://purl.org/weso/rdfindex/ontology/dataset> <http://purl.org/weso/cloudindex/component/Accountability>.
_:bnode653393792 <http://purl.org/weso/rdfindex/ontology/weight> "0.14"^^<http://www.w3.org/2001/XMLSchema#double>.
_:bnode134673728 <http://purl.org/weso/rdfindex/ontology/part-of> _:bnode653393792.
_:bnode1172113856 <http://purl.org/weso/rdfindex/ontology/dataset> <http://purl.org/weso/cloudindex/component/Agility>.
_:bnode1172113856 <http://purl.org/weso/rdfindex/ontology/weight> "0.14"^^<http://www.w3.org/2001/XMLSchema#double>.
_:bnode134673728 <http://purl.org/weso/rdfindex/ontology/part-of> _:bnode1172113856.
_:bnode1690833920 <http://purl.org/weso/rdfindex/ontology/dataset> <http://purl.org/weso/cloudindex/component/Assurance>.
_:bnode1690833920 <http://purl.org/weso/rdfindex/ontology/weight> "0.14"^^<http://www.w3.org/2001/XMLSchema#double>.
_:bnode134673728 <http://purl.org/weso/rdfindex/ontology/part-of> _:bnode1690833920.
_:bnode2085413312 <http://purl.org/weso/rdfindex/ontology/dataset> <http://purl.org/weso/cloudindex/component/Financial>.
_:bnode2085413312 <http://purl.org/weso/rdfindex/ontology/weight> "0.14"^^<http://www.w3.org/2001/XMLSchema#double>.
_:bnode134673728 <http://purl.org/weso/rdfindex/ontology/part-of> _:bnode2085413312.
_:bnode1566693248 <http://purl.org/weso/rdfindex/ontology/dataset> <http://purl.org/weso/cloudindex/component/Performance>.
_:bnode1566693248 <http://purl.org/weso/rdfindex/ontology/weight> "0.14"^^<http://www.w3.org/2001/XMLSchema#double>.
_:bnode134673728 <http://purl.org/weso/rdfindex/ontology/part-of> _:bnode1566693248.
_:bnode1047973184 <http://purl.org/weso/rdfindex/ontology/dataset> <http://purl.org/weso/cloudindex/component/SecurityPrivacy>.
_:bnode1047973184 <http://purl.org/weso/rdfindex/ontology/weight> "0.14"^^<http://www.w3.org/2001/XMLSchema#double>.
_:bnode134673728 <http://purl.org/weso/rdfindex/ontology/part-of> _:bnode1047973184.
_:bnode529253120 <http://purl.org/weso/rdfindex/ontology/dataset> <http://purl.org/weso/cloudindex/component/Usability>.
_:bnode529253120 <http://purl.org/weso/rdfindex/ontology/weight> "0.14"^^<http://www.w3.org/2001/XMLSchema#double>.
_:bnode134673728 <http://purl.org/weso/rdfindex/ontology/part-of> _:bnode529253120.
<http://purl.org/weso/cloudindex/index> <http://purl.org/weso/rdfindex/ontology/aggregates> _:bnode134673728.
<http://purl.org/weso/cloudindex/index> <http://purl.org/linked-data/cube#structure> <http://purl.org/weso/cloudindex/CloundIndexDSD>.
<http://purl.org/weso/cloudindex/index> <http://www.w3.org/2004/02/skos/core#narrower> <http://purl.org/weso/cloudindex/component/Accountability>.
<http://purl.org/weso/cloudindex/index> <http://www.w3.org/2004/02/skos/core#narrower> <http://purl.org/weso/cloudindex/component/Agility>.
<http://purl.org/weso/cloudindex/index> <http://www.w3.org/2004/02/skos/core#narrower> <http://purl.org/weso/cloudindex/component/Assurance>.
<http://purl.org/weso/cloudindex/index> <http://www.w3.org/2004/02/skos/core#narrower> <http://purl.org/weso/cloudindex/component/Financial>.
<http://purl.org/weso/cloudindex/index> <http://www.w3.org/2004/02/skos/core#narrower> <http://purl.org/weso/cloudindex/component/Performance>.
<http://purl.org/weso/cloudindex/index> <http://www.w3.org/2004/02/skos/core#narrower> <http://purl.org/weso/cloudindex/component/SecurityPrivacy>.
<http://purl.org/weso/cloudindex/index> <http://www.w3.org/2004/02/skos/core#narrower> <http://purl.org/weso/cloudindex/component/Usability>.
<http://purl.org/weso/cloudindex/component/ds> <http://www.w3.org/1999/02/22-rdf-syntax-ns#type> <http://rdfs.org/ns/void#Dataset>.
<http://purl.org/weso/cloudindex/component/ds> <http://www.w3.org/2000/01/rdf-schema#label> "SEERC| CloudIndex | Components"@en.
<http://purl.org/weso/cloudindex/component/ds> <http://www.w3.org/2000/01/rdf-schema#comment> "Dataset of components that aggregates different indicators and are part of a subindex."@en.
<http://purl.org/weso/cloudindex/component/ds> <http://purl.org/dc/terms/created> "2012-20-05"^^<http://www.w3.org/2001/XMLSchema#date>.
<http://purl.org/weso/cloudindex/component/ds> <http://purl.org/dc/terms/modified> "2012-08-31"^^<http://www.w3.org/2001/XMLSchema#date>.
<http://purl.org/weso/cloudindex/component/ds> <http://purl.org/dc/terms/title> "Core CloudIndex ontology"@en.
<http://purl.org/weso/cloudindex/component/ds> <http://purl.org/dc/terms/author> <http://purl.org/weso/cloudindex/people/Chema>.
<http://purl.org/weso/cloudindex/component/ds> <http://purl.org/dc/terms/author> <http://purl.org/weso/rdfindex/organization/SEERC>.
<http://purl.org/weso/cloudindex/component/ds> <http://purl.org/dc/terms/publisher> <http://purl.org/weso/cloudindex/people/Chema>.
<http://purl.org/weso/cloudindex/component/ds> <http://purl.org/dc/terms/contributor> <http://purl.org/weso/rdfindex/organization/SEERC>.
<http://purl.org/weso/cloudindex/component/ds> <http://purl.org/dc/terms/contributor> <http://purl.org/weso/rdfindex/project/RELATE>.
<http://purl.org/weso/cloudindex/component/ds> <http://purl.org/dc/terms/license> <http://opendatacommons.org/licenses/by/1.0/>.
<http://purl.org/weso/cloudindex/component/ds> <http://rdfs.org/ns/void#exampleResource> <http://purl.org/weso/cloudindex/component/Accountability>.
<http://purl.org/weso/cloudindex/component/ds> <http://rdfs.org/ns/void#uriRegexPattern> "http://purl.org/weso/cloudindex/component/.+".
<http://purl.org/weso/cloudindex/component/ds> <http://rdfs.org/ns/void#vocabulary> <http://www.w3.org/2000/01/rdf-schema#>.
<http://purl.org/weso/cloudindex/component/ds> <http://rdfs.org/ns/void#vocabulary> <http://www.w3.org/2004/02/skos/core#>.
<http://purl.org/weso/cloudindex/component/ds> <http://xmlns.com/foaf/0.1/homepage> <http://purl.org/weso/cloudindex/>.
<http://purl.org/weso/cloudindex/component/Accountability> <http://www.w3.org/1999/02/22-rdf-syntax-ns#type> <http://purl.org/weso/rdfindex/ontology/Component>.
<http://purl.org/weso/cloudindex/component/Accountability> <http://www.w3.org/2000/01/rdf-schema#label> "Accountability"@en.
<http://purl.org/weso/cloudindex/component/Accountability> <http://www.w3.org/2000/01/rdf-schema#comment> "This component is used to measure the properties related to the service provider\r\norganization. These properties may be independent of the service being provided."@en.
<http://purl.org/weso/cloudindex/component/Accountability> <http://purl.org/weso/cloudindex/ontology/defined-in> <http://csmic.org/wp-content/uploads/2011/09/SMI-Overview-110913_v1F.pdf>.
<http://purl.org/weso/cloudindex/component/Accountability> <http://purl.org/weso/cloudindex/ontology/defined-by> <http://purl.org/weso/cloudindex/organization/CSMIC>.
<http://purl.org/weso/cloudindex/component/Accountability> <http://purl.org/weso/rdfindex/ontology/weight> "1"^^<http://www.w3.org/2001/XMLSchema#double>.
_:bnode1026907072 <http://purl.org/weso/rdfindex/ontology/aggregation-operator> <http://purl.org/weso/rdfindex/ontology/OWA>.
_:bnode1545627136 <http://purl.org/weso/rdfindex/ontology/dataset> <http://purl.org/weso/cloudindex/indicator/Auditability>.
_:bnode1545627136 <http://purl.org/weso/rdfindex/ontology/weight> "0.06"^^<http://www.w3.org/2001/XMLSchema#double>.
_:bnode1026907072 <http://purl.org/weso/rdfindex/ontology/part-of> _:bnode1545627136.
_:bnode2064347200 <http://purl.org/weso/rdfindex/ontology/dataset> <http://purl.org/weso/cloudindex/indicator/Compliance>.
_:bnode2064347200 <http://purl.org/weso/rdfindex/ontology/weight> "0.06"^^<http://www.w3.org/2001/XMLSchema#double>.
_:bnode1026907072 <http://purl.org/weso/rdfindex/ontology/part-of> _:bnode2064347200.
_:bnode1711900032 <http://purl.org/weso/rdfindex/ontology/dataset> <http://purl.org/weso/cloudindex/indicator/ContractingExperience>.
_:bnode1711900032 <http://purl.org/weso/rdfindex/ontology/weight> "0.06"^^<http://www.w3.org/2001/XMLSchema#double>.
_:bnode1026907072 <http://purl.org/weso/rdfindex/ontology/part-of> _:bnode1711900032.
_:bnode1193179968 <http://purl.org/weso/rdfindex/ontology/dataset> <http://purl.org/weso/cloudindex/indicator/DataOwnership>.
_:bnode1193179968 <http://purl.org/weso/rdfindex/ontology/weight> "0.06"^^<http://www.w3.org/2001/XMLSchema#double>.
_:bnode1026907072 <http://purl.org/weso/rdfindex/ontology/part-of> _:bnode1193179968.
_:bnode674459904 <http://purl.org/weso/rdfindex/ontology/dataset> <http://purl.org/weso/cloudindex/indicator/EaseDoingBusiness>.
_:bnode674459904 <http://purl.org/weso/rdfindex/ontology/weight> "0.06"^^<http://www.w3.org/2001/XMLSchema#double>.
_:bnode1026907072 <http://purl.org/weso/rdfindex/ontology/part-of> _:bnode674459904.
_:bnode155739840 <http://purl.org/weso/rdfindex/ontology/dataset> <http://purl.org/weso/cloudindex/indicator/Governance>.
_:bnode155739840 <http://purl.org/weso/rdfindex/ontology/weight> "0.06"^^<http://www.w3.org/2001/XMLSchema#double>.
_:bnode1026907072 <http://purl.org/weso/rdfindex/ontology/part-of> _:bnode155739840.
_:bnode362980224 <http://purl.org/weso/rdfindex/ontology/dataset> <http://purl.org/weso/cloudindex/indicator/Ownership>.
_:bnode362980224 <http://purl.org/weso/rdfindex/ontology/weight> "0.06"^^<http://www.w3.org/2001/XMLSchema#double>.
_:bnode1026907072 <http://purl.org/weso/rdfindex/ontology/part-of> _:bnode362980224.
_:bnode881700288 <http://purl.org/weso/rdfindex/ontology/dataset> <http://purl.org/weso/cloudindex/indicator/ProviderStability>.
_:bnode881700288 <http://purl.org/weso/rdfindex/ontology/weight> "0.06"^^<http://www.w3.org/2001/XMLSchema#double>.
_:bnode1026907072 <http://purl.org/weso/rdfindex/ontology/part-of> _:bnode881700288.
_:bnode1400420352 <http://purl.org/weso/rdfindex/ontology/dataset> <http://purl.org/weso/cloudindex/indicator/ProviderCertifications>.
_:bnode1400420352 <http://purl.org/weso/rdfindex/ontology/weight> "0.06"^^<http://www.w3.org/2001/XMLSchema#double>.
_:bnode1026907072 <http://purl.org/weso/rdfindex/ontology/part-of> _:bnode1400420352.
_:bnode1919140416 <http://purl.org/weso/rdfindex/ontology/dataset> <http://purl.org/weso/cloudindex/indicator/ProviderSLAVerification>.
_:bnode1919140416 <http://purl.org/weso/rdfindex/ontology/weight> "0.06"^^<http://www.w3.org/2001/XMLSchema#double>.
_:bnode1026907072 <http://purl.org/weso/rdfindex/ontology/part-of> _:bnode1919140416.
_:bnode1857106816 <http://purl.org/weso/rdfindex/ontology/dataset> <http://purl.org/weso/cloudindex/indicator/ProviderEthics>.
_:bnode1857106816 <http://purl.org/weso/rdfindex/ontology/weight> "0.06"^^<http://www.w3.org/2001/XMLSchema#double>.
_:bnode1026907072 <http://purl.org/weso/rdfindex/ontology/part-of> _:bnode1857106816.
_:bnode1338386752 <http://purl.org/weso/rdfindex/ontology/dataset> <http://purl.org/weso/cloudindex/indicator/ProviderPersonnelRequirements>.
_:bnode1338386752 <http://purl.org/weso/rdfindex/ontology/weight> "0.06"^^<http://www.w3.org/2001/XMLSchema#double>.
_:bnode1026907072 <http://purl.org/weso/rdfindex/ontology/part-of> _:bnode1338386752.
_:bnode819666688 <http://purl.org/weso/rdfindex/ontology/dataset> <http://purl.org/weso/cloudindex/indicator/ProviderSupplyChain>.
_:bnode819666688 <http://purl.org/weso/rdfindex/ontology/weight> "0.06"^^<http://www.w3.org/2001/XMLSchema#double>.
_:bnode1026907072 <http://purl.org/weso/rdfindex/ontology/part-of> _:bnode819666688.
_:bnode300946624 <http://purl.org/weso/rdfindex/ontology/dataset> <http://purl.org/weso/cloudindex/indicator/ProviderSecurityCapabilities>.
_:bnode300946624 <http://purl.org/weso/rdfindex/ontology/weight> "0.06"^^<http://www.w3.org/2001/XMLSchema#double>.
_:bnode1026907072 <http://purl.org/weso/rdfindex/ontology/part-of> _:bnode300946624.
_:bnode217773440 <http://purl.org/weso/rdfindex/ontology/dataset> <http://purl.org/weso/cloudindex/indicator/Sustainability>.
_:bnode217773440 <http://purl.org/weso/rdfindex/ontology/weight> "0.06"^^<http://www.w3.org/2001/XMLSchema#double>.
_:bnode1026907072 <http://purl.org/weso/rdfindex/ontology/part-of> _:bnode217773440.
<http://purl.org/weso/cloudindex/component/Accountability> <http://purl.org/weso/rdfindex/ontology/aggregates> _:bnode1026907072.
<http://purl.org/weso/cloudindex/component/Accountability> <http://purl.org/linked-data/cube#structure> <http://purl.org/weso/cloudindex/AccountabilityDSD>.
<http://purl.org/weso/cloudindex/component/Accountability> <http://www.w3.org/2004/02/skos/core#narrower> <http://purl.org/weso/cloudindex/indicator/Auditability>.
<http://purl.org/weso/cloudindex/component/Accountability> <http://www.w3.org/2004/02/skos/core#narrower> <http://purl.org/weso/cloudindex/indicator/Compliance>.
<http://purl.org/weso/cloudindex/component/Accountability> <http://www.w3.org/2004/02/skos/core#narrower> <http://purl.org/weso/cloudindex/indicator/ContractingExperience>.
<http://purl.org/weso/cloudindex/component/Accountability> <http://www.w3.org/2004/02/skos/core#narrower> <http://purl.org/weso/cloudindex/indicator/DataOwnership>.
<http://purl.org/weso/cloudindex/component/Accountability> <http://www.w3.org/2004/02/skos/core#narrower> <http://purl.org/weso/cloudindex/indicator/EaseDoingBusiness>.
<http://purl.org/weso/cloudindex/component/Accountability> <http://www.w3.org/2004/02/skos/core#narrower> <http://purl.org/weso/cloudindex/indicator/Governance>.
<http://purl.org/weso/cloudindex/component/Accountability> <http://www.w3.org/2004/02/skos/core#narrower> <http://purl.org/weso/cloudindex/indicator/Ownership>.
<http://purl.org/weso/cloudindex/component/Accountability> <http://www.w3.org/2004/02/skos/core#narrower> <http://purl.org/weso/cloudindex/indicator/ProviderStability>.
<http://purl.org/weso/cloudindex/component/Accountability> <http://www.w3.org/2004/02/skos/core#narrower> <http://purl.org/weso/cloudindex/indicator/ProviderCertifications>.
<http://purl.org/weso/cloudindex/component/Accountability> <http://www.w3.org/2004/02/skos/core#narrower> <http://purl.org/weso/cloudindex/indicator/ProviderSLAVerification>.
<http://purl.org/weso/cloudindex/component/Accountability> <http://www.w3.org/2004/02/skos/core#narrower> <http://purl.org/weso/cloudindex/indicator/ProviderEthics>.
<http://purl.org/weso/cloudindex/component/Accountability> <http://www.w3.org/2004/02/skos/core#narrower> <http://purl.org/weso/cloudindex/indicator/ProviderPersonnelRequirements>.
<http://purl.org/weso/cloudindex/component/Accountability> <http://www.w3.org/2004/02/skos/core#narrower> <http://purl.org/weso/cloudindex/indicator/ProviderSupplyChain>.
<http://purl.org/weso/cloudindex/component/Accountability> <http://www.w3.org/2004/02/skos/core#narrower> <http://purl.org/weso/cloudindex/indicator/ProviderSecurityCapabilities>.
<http://purl.org/weso/cloudindex/component/Accountability> <http://www.w3.org/2004/02/skos/core#narrower> <http://purl.org/weso/cloudindex/indicator/Sustainability>.
<http://purl.org/weso/cloudindex/component/Agility> <http://www.w3.org/1999/02/22-rdf-syntax-ns#type> <http://purl.org/weso/rdfindex/ontology/Component>.
<http://purl.org/weso/cloudindex/component/Agility> <http://www.w3.org/2000/01/rdf-schema#label> "Agility"@en.
<http://purl.org/weso/cloudindex/component/Agility> <http://www.w3.org/2000/01/rdf-schema#comment> "Indicates the impact of a service upon a client's ability to change direction, strategy, or tactics quickly\r\nand with minimal disruption."@en.
<http://purl.org/weso/cloudindex/component/Agility> <http://purl.org/weso/cloudindex/ontology/defined-in> <http://csmic.org/wp-content/uploads/2011/09/SMI-Overview-110913_v1F.pdf>.
<http://purl.org/weso/cloudindex/component/Agility> <http://purl.org/weso/cloudindex/ontology/defined-by> <http://purl.org/weso/cloudindex/organization/CSMIC>.
<http://purl.org/weso/cloudindex/component/Agility> <http://purl.org/weso/cloudindex/ontology/weight> "1"^^<http://www.w3.org/2001/XMLSchema#double>.
_:bnode736493504 <http://purl.org/weso/rdfindex/ontology/aggregation-operator> <http://purl.org/weso/rdfindex/ontology/OWA>.
_:bnode1255213568 <http://purl.org/weso/rdfindex/ontology/dataset> <http://purl.org/weso/cloudindex/indicator/Adaptability>.
_:bnode1255213568 <http://purl.org/weso/rdfindex/ontology/weight> "0.14"^^<http://www.w3.org/2001/XMLSchema#double>.
_:bnode736493504 <http://purl.org/weso/rdfindex/ontology/part-of> _:bnode1255213568.
_:bnode1773933632 <http://purl.org/weso/rdfindex/ontology/dataset> <http://purl.org/weso/cloudindex/indicator/Capacity>.
_:bnode1773933632 <http://purl.org/weso/rdfindex/ontology/weight> "0.14"^^<http://www.w3.org/2001/XMLSchema#double>.
_:bnode736493504 <http://purl.org/weso/rdfindex/ontology/part-of> _:bnode1773933632.
_:bnode2002313600 <http://purl.org/weso/rdfindex/ontology/dataset> <http://purl.org/weso/cloudindex/indicator/Elasticity>.
_:bnode2002313600 <http://purl.org/weso/rdfindex/ontology/weight> "0.14"^^<http://www.w3.org/2001/XMLSchema#double>.
_:bnode736493504 <http://purl.org/weso/rdfindex/ontology/part-of> _:bnode2002313600.
_:bnode1483593536 <http://purl.org/weso/rdfindex/ontology/dataset> <http://purl.org/weso/cloudindex/indicator/Extensibility>.
_:bnode1483593536 <http://purl.org/weso/rdfindex/ontology/weight> "0.14"^^<http://www.w3.org/2001/XMLSchema#double>.
_:bnode736493504 <http://purl.org/weso/rdfindex/ontology/part-of> _:bnode1483593536.
_:bnode964873472 <http://purl.org/weso/rdfindex/ontology/dataset> <http://purl.org/weso/cloudindex/indicator/Flexibility>.
_:bnode964873472 <http://purl.org/weso/rdfindex/ontology/weight> "0.14"^^<http://www.w3.org/2001/XMLSchema#double>.
_:bnode736493504 <http://purl.org/weso/rdfindex/ontology/part-of> _:bnode964873472.
_:bnode446153408 <http://purl.org/weso/rdfindex/ontology/dataset> <http://purl.org/weso/cloudindex/indicator/Portability>.
_:bnode446153408 <http://purl.org/weso/rdfindex/ontology/weight> "0.14"^^<http://www.w3.org/2001/XMLSchema#double>.
_:bnode736493504 <http://purl.org/weso/rdfindex/ontology/part-of> _:bnode446153408.
_:bnode72566656 <http://purl.org/weso/rdfindex/ontology/dataset> <http://purl.org/weso/cloudindex/indicator/Scalability>.
_:bnode72566656 <http://purl.org/weso/rdfindex/ontology/weight> "0.14"^^<http://www.w3.org/2001/XMLSchema#double>.
_:bnode736493504 <http://purl.org/weso/rdfindex/ontology/part-of> _:bnode72566656.
<http://purl.org/weso/cloudindex/component/Agility> <http://purl.org/weso/rdfindex/ontology/aggregates> _:bnode736493504.
<http://purl.org/weso/cloudindex/component/Agility> <http://purl.org/linked-data/cube#structure> <http://purl.org/weso/cloudindex/AgilityDSD>.
<http://purl.org/weso/cloudindex/component/Agility> <http://www.w3.org/2004/02/skos/core#narrower> <http://purl.org/weso/cloudindex/indicator/Adaptability>.
<http://purl.org/weso/cloudindex/component/Agility> <http://www.w3.org/2004/02/skos/core#narrower> <http://purl.org/weso/cloudindex/indicator/Capacity>.
<http://purl.org/weso/cloudindex/component/Agility> <http://www.w3.org/2004/02/skos/core#narrower> <http://purl.org/weso/cloudindex/indicator/Elasticity>.
<http://purl.org/weso/cloudindex/component/Agility> <http://www.w3.org/2004/02/skos/core#narrower> <http://purl.org/weso/cloudindex/indicator/Extensibility>.
<http://purl.org/weso/cloudindex/component/Agility> <http://www.w3.org/2004/02/skos/core#narrower> <http://purl.org/weso/cloudindex/indicator/Flexibility>.
<http://purl.org/weso/cloudindex/component/Agility> <http://www.w3.org/2004/02/skos/core#narrower> <http://purl.org/weso/cloudindex/indicator/Portability>.
<http://purl.org/weso/cloudindex/component/Agility> <http://www.w3.org/2004/02/skos/core#narrower> <http://purl.org/weso/cloudindex/indicator/Scalability>.
<http://purl.org/weso/cloudindex/component/Assurance> <http://www.w3.org/1999/02/22-rdf-syntax-ns#type> <http://purl.org/weso/rdfindex/ontology/Component>.
<http://purl.org/weso/cloudindex/component/Assurance> <http://www.w3.org/2000/01/rdf-schema#label> "Assurance"@en.
<http://purl.org/weso/cloudindex/component/Assurance> <http://www.w3.org/2000/01/rdf-schema#comment> "This category includes key attributes that indicate how likely it is that the service will be available as\r\nspecified."@en.
<http://purl.org/weso/cloudindex/component/Assurance> <http://purl.org/weso/cloudindex/ontology/defined-in> <http://csmic.org/wp-content/uploads/2011/09/SMI-Overview-110913_v1F.pdf>.
<http://purl.org/weso/cloudindex/component/Assurance> <http://purl.org/weso/cloudindex/ontology/defined-by> <http://purl.org/weso/cloudindex/organization/CSMIC>.
<http://purl.org/weso/cloudindex/component/Assurance> <http://purl.org/weso/cloudindex/ontology/weight> "1"^^<http://www.w3.org/2001/XMLSchema#double>.
_:bnode591286720 <http://purl.org/weso/rdfindex/ontology/aggregation-operator> <http://purl.org/weso/rdfindex/ontology/OWA>.
_:bnode1110006784 <http://purl.org/weso/rdfindex/ontology/dataset> <http://purl.org/weso/cloudindex/indicator/Availability>.
_:bnode1110006784 <http://purl.org/weso/rdfindex/ontology/weight> "0.14"^^<http://www.w3.org/2001/XMLSchema#double>.
_:bnode591286720 <http://purl.org/weso/rdfindex/ontology/part-of> _:bnode1110006784.
_:bnode1628726848 <http://purl.org/weso/rdfindex/ontology/dataset> <http://purl.org/weso/cloudindex/indicator/Maintainability>.
_:bnode1628726848 <http://purl.org/weso/rdfindex/ontology/weight> "0.14"^^<http://www.w3.org/2001/XMLSchema#double>.
_:bnode591286720 <http://purl.org/weso/rdfindex/ontology/part-of> _:bnode1628726848.
_:bnode2147446912 <http://purl.org/weso/rdfindex/ontology/dataset> <http://purl.org/weso/cloudindex/indicator/Recoverability>.
_:bnode2147446912 <http://purl.org/weso/rdfindex/ontology/weight> "0.14"^^<http://www.w3.org/2001/XMLSchema#double>.
_:bnode591286720 <http://purl.org/weso/rdfindex/ontology/part-of> _:bnode2147446912.
_:bnode1628800320 <http://purl.org/weso/rdfindex/ontology/dataset> <http://purl.org/weso/cloudindex/indicator/Reliability>.
_:bnode1628800320 <http://purl.org/weso/rdfindex/ontology/weight> "0.14"^^<http://www.w3.org/2001/XMLSchema#double>.
_:bnode591286720 <http://purl.org/weso/rdfindex/ontology/part-of> _:bnode1628800320.
_:bnode1110080256 <http://purl.org/weso/rdfindex/ontology/dataset> <http://purl.org/weso/cloudindex/indicator/Resiliency>.
_:bnode1110080256 <http://purl.org/weso/rdfindex/ontology/weight> "0.14"^^<http://www.w3.org/2001/XMLSchema#double>.
_:bnode591286720 <http://purl.org/weso/rdfindex/ontology/part-of> _:bnode1110080256.
_:bnode591360192 <http://purl.org/weso/rdfindex/ontology/dataset> <http://purl.org/weso/cloudindex/indicator/Stability>.
_:bnode591360192 <http://purl.org/weso/rdfindex/ontology/weight> "0.14"^^<http://www.w3.org/2001/XMLSchema#double>.
_:bnode591286720 <http://purl.org/weso/rdfindex/ontology/part-of> _:bnode591360192.
_:bnode72640128 <http://purl.org/weso/rdfindex/ontology/dataset> <http://purl.org/weso/cloudindex/indicator/Serviceability>.
_:bnode72640128 <http://purl.org/weso/rdfindex/ontology/weight> "0.14"^^<http://www.w3.org/2001/XMLSchema#double>.
_:bnode591286720 <http://purl.org/weso/rdfindex/ontology/part-of> _:bnode72640128.
<http://purl.org/weso/cloudindex/component/Assurance> <http://purl.org/weso/rdfindex/ontology/aggregates> _:bnode591286720.
<http://purl.org/weso/cloudindex/component/Assurance> <http://purl.org/linked-data/cube#structure> <http://purl.org/weso/cloudindex/AssuranceDSD>.
<http://purl.org/weso/cloudindex/component/Assurance> <http://www.w3.org/2004/02/skos/core#narrower> <http://purl.org/weso/cloudindex/indicator/Availability>.
<http://purl.org/weso/cloudindex/component/Assurance> <http://www.w3.org/2004/02/skos/core#narrower> <http://purl.org/weso/cloudindex/indicator/Maintainability>.
<http://purl.org/weso/cloudindex/component/Assurance> <http://www.w3.org/2004/02/skos/core#narrower> <http://purl.org/weso/cloudindex/indicator/Recoverability>.
<http://purl.org/weso/cloudindex/component/Assurance> <http://www.w3.org/2004/02/skos/core#narrower> <http://purl.org/weso/cloudindex/indicator/Reliability>.
<http://purl.org/weso/cloudindex/component/Assurance> <http://www.w3.org/2004/02/skos/core#narrower> <http://purl.org/weso/cloudindex/indicator/Resiliency>.
<http://purl.org/weso/cloudindex/component/Assurance> <http://www.w3.org/2004/02/skos/core#narrower> <http://purl.org/weso/cloudindex/indicator/Stability>.
<http://purl.org/weso/cloudindex/component/Assurance> <http://www.w3.org/2004/02/skos/core#narrower> <http://purl.org/weso/cloudindex/indicator/Serviceability>.
<http://purl.org/weso/cloudindex/component/Financial> <http://www.w3.org/1999/02/22-rdf-syntax-ns#type> <http://purl.org/weso/rdfindex/ontology/Component>.
<http://purl.org/weso/cloudindex/component/Financial> <http://www.w3.org/2000/01/rdf-schema#label> "Financial"@en.
<http://purl.org/weso/cloudindex/component/Financial> <http://www.w3.org/2000/01/rdf-schema#comment> "The amount of money spent on the service by the client."@en.
<http://purl.org/weso/cloudindex/component/Financial> <http://purl.org/weso/cloudindex/ontology/defined-in> <http://csmic.org/wp-content/uploads/2011/09/SMI-Overview-110913_v1F.pdf>.
<http://purl.org/weso/cloudindex/component/Financial> <http://purl.org/weso/cloudindex/ontology/defined-by> <http://purl.org/weso/cloudindex/organization/CSMIC>.
<http://purl.org/weso/cloudindex/component/Financial> <http://purl.org/weso/cloudindex/ontology/weight> "1"^^<http://www.w3.org/2001/XMLSchema#double>.
_:bnode446079936 <http://purl.org/weso/rdfindex/ontology/aggregation-operator> <http://purl.org/weso/rdfindex/ontology/OWA>.
_:bnode964800000 <http://purl.org/weso/rdfindex/ontology/dataset> <http://purl.org/weso/cloudindex/indicator/Acquisition>.
_:bnode964800000 <http://purl.org/weso/rdfindex/ontology/weight> "0.33"^^<http://www.w3.org/2001/XMLSchema#double>.
_:bnode446079936 <http://purl.org/weso/rdfindex/ontology/part-of> _:bnode964800000.
_:bnode1483520064 <http://purl.org/weso/rdfindex/ontology/dataset> <http://purl.org/weso/cloudindex/indicator/OngoingCost>.
_:bnode1483520064 <http://purl.org/weso/rdfindex/ontology/weight> "0.33"^^<http://www.w3.org/2001/XMLSchema#double>.
_:bnode446079936 <http://purl.org/weso/rdfindex/ontology/part-of> _:bnode1483520064.
_:bnode2002240128 <http://purl.org/weso/rdfindex/ontology/dataset> <http://purl.org/weso/cloudindex/indicator/Profit>.
_:bnode2002240128 <http://purl.org/weso/rdfindex/ontology/weight> "0.33"^^<http://www.w3.org/2001/XMLSchema#double>.
_:bnode446079936 <http://purl.org/weso/rdfindex/ontology/part-of> _:bnode2002240128.
<http://purl.org/weso/cloudindex/component/Financial> <http://purl.org/weso/rdfindex/ontology/aggregates> _:bnode446079936.
<http://purl.org/weso/cloudindex/component/Financial> <http://purl.org/linked-data/cube#structure> <http://purl.org/weso/cloudindex/FinancialDSD>.
<http://purl.org/weso/cloudindex/component/Financial> <http://www.w3.org/2004/02/skos/core#narrower> <http://purl.org/weso/cloudindex/indicator/Acquisition>.
<http://purl.org/weso/cloudindex/component/Financial> <http://www.w3.org/2004/02/skos/core#narrower> <http://purl.org/weso/cloudindex/indicator/OngoingCost>.
<http://purl.org/weso/cloudindex/component/Financial> <http://www.w3.org/2004/02/skos/core#narrower> <http://purl.org/weso/cloudindex/indicator/Profit>.
<http://purl.org/weso/cloudindex/component/Performance> <http://www.w3.org/1999/02/22-rdf-syntax-ns#type> <http://purl.org/weso/rdfindex/ontology/Component>.
<http://purl.org/weso/cloudindex/component/Performance> <http://www.w3.org/2000/01/rdf-schema#label> "Performance"@en.
<http://purl.org/weso/cloudindex/component/Performance> <http://www.w3.org/2000/01/rdf-schema#comment> "This category covers the features and functions of the provided services."@en.
<http://purl.org/weso/cloudindex/component/Performance> <http://purl.org/weso/cloudindex/ontology/defined-in> <http://csmic.org/wp-content/uploads/2011/09/SMI-Overview-110913_v1F.pdf>.
<http://purl.org/weso/cloudindex/component/Performance> <http://purl.org/weso/cloudindex/ontology/defined-by> <http://purl.org/weso/cloudindex/organization/CSMIC>.
<http://purl.org/weso/cloudindex/component/Performance> <http://purl.org/weso/cloudindex/ontology/weight> "1"^^<http://www.w3.org/2001/XMLSchema#double>.
_:bnode1774007104 <http://purl.org/weso/rdfindex/ontology/aggregation-operator> <http://purl.org/weso/rdfindex/ontology/OWA>.
_:bnode1255287040 <http://purl.org/weso/rdfindex/ontology/dataset> <http://purl.org/weso/cloudindex/indicator/Accuracy>.
_:bnode1255287040 <http://purl.org/weso/rdfindex/ontology/weight> "0.2"^^<http://www.w3.org/2001/XMLSchema#double>.
_:bnode1774007104 <http://purl.org/weso/rdfindex/ontology/part-of> _:bnode1255287040.
_:bnode736566976 <http://purl.org/weso/rdfindex/ontology/dataset> <http://purl.org/weso/cloudindex/indicator/Functionality>.
_:bnode736566976 <http://purl.org/weso/rdfindex/ontology/weight> "0.2"^^<http://www.w3.org/2001/XMLSchema#double>.
_:bnode1774007104 <http://purl.org/weso/rdfindex/ontology/part-of> _:bnode736566976.
_:bnode217846912 <http://purl.org/weso/rdfindex/ontology/dataset> <http://purl.org/weso/cloudindex/indicator/Suitability>.
_:bnode217846912 <http://purl.org/weso/rdfindex/ontology/weight> "0.2"^^<http://www.w3.org/2001/XMLSchema#double>.
_:bnode1774007104 <http://purl.org/weso/rdfindex/ontology/part-of> _:bnode217846912.
_:bnode300873152 <http://purl.org/weso/rdfindex/ontology/dataset> <http://purl.org/weso/cloudindex/indicator/Interoperability>.
_:bnode300873152 <http://purl.org/weso/rdfindex/ontology/weight> "0.2"^^<http://www.w3.org/2001/XMLSchema#double>.
_:bnode1774007104 <http://purl.org/weso/rdfindex/ontology/part-of> _:bnode300873152.
_:bnode819593216 <http://purl.org/weso/rdfindex/ontology/dataset> <http://purl.org/weso/cloudindex/indicator/ServiceResponseTime>.
_:bnode819593216 <http://purl.org/weso/rdfindex/ontology/weight> "0.2"^^<http://www.w3.org/2001/XMLSchema#double>.
_:bnode1774007104 <http://purl.org/weso/rdfindex/ontology/part-of> _:bnode819593216.
<http://purl.org/weso/cloudindex/component/Performance> <http://purl.org/weso/rdfindex/ontology/aggregates> _:bnode1774007104.
<http://purl.org/weso/cloudindex/component/Performance> <http://purl.org/linked-data/cube#structure> <http://purl.org/weso/cloudindex/PerformanceDSD>.
<http://purl.org/weso/cloudindex/component/Performance> <http://www.w3.org/2004/02/skos/core#narrower> <http://purl.org/weso/cloudindex/indicator/Accuracy>.
<http://purl.org/weso/cloudindex/component/Performance> <http://www.w3.org/2004/02/skos/core#narrower> <http://purl.org/weso/cloudindex/indicator/Functionality>.
<http://purl.org/weso/cloudindex/component/Performance> <http://www.w3.org/2004/02/skos/core#narrower> <http://purl.org/weso/cloudindex/indicator/Suitability>.
<http://purl.org/weso/cloudindex/component/Performance> <http://www.w3.org/2004/02/skos/core#narrower> <http://purl.org/weso/cloudindex/indicator/Interoperability>.
<http://purl.org/weso/cloudindex/component/Performance> <http://www.w3.org/2004/02/skos/core#narrower> <http://purl.org/weso/cloudindex/indicator/ServiceResponseTime>.
<http://purl.org/weso/cloudindex/component/SecurityPrivacy> <http://www.w3.org/1999/02/22-rdf-syntax-ns#type> <http://purl.org/weso/rdfindex/ontology/Component>.
<http://purl.org/weso/cloudindex/component/SecurityPrivacy> <http://www.w3.org/2000/01/rdf-schema#label> "Security and Privacy"@en.
<http://purl.org/weso/cloudindex/component/SecurityPrivacy> <http://www.w3.org/2000/01/rdf-schema#comment> "This category includes attributes that indicate the effectiveness of a service provider's controls on\r\naccess to services, service data, and the physical facilities from which services are provided."@en.
<http://purl.org/weso/cloudindex/component/SecurityPrivacy> <http://purl.org/weso/cloudindex/ontology/defined-in> <http://csmic.org/wp-content/uploads/2011/09/SMI-Overview-110913_v1F.pdf>.
<http://purl.org/weso/cloudindex/component/SecurityPrivacy> <http://purl.org/weso/cloudindex/ontology/defined-by> <http://purl.org/weso/cloudindex/organization/CSMIC>.
<http://purl.org/weso/cloudindex/component/SecurityPrivacy> <http://purl.org/weso/cloudindex/ontology/weight> "1"^^<http://www.w3.org/2001/XMLSchema#double>.
_:bnode1365351936 <http://purl.org/weso/rdfindex/ontology/aggregation-operator> <http://purl.org/weso/rdfindex/ontology/OWA>.
_:bnode1884072000 <http://purl.org/weso/rdfindex/ontology/dataset> <http://purl.org/weso/cloudindex/indicator/AccessControl>.
_:bnode1884072000 <http://purl.org/weso/rdfindex/ontology/weight> "0.1"^^<http://www.w3.org/2001/XMLSchema#double>.
_:bnode1365351936 <http://purl.org/weso/rdfindex/ontology/part-of> _:bnode1884072000.
_:bnode1892175232 <http://purl.org/weso/rdfindex/ontology/dataset> <http://purl.org/weso/cloudindex/indicator/GeographicalConstraint>.
_:bnode1892175232 <http://purl.org/weso/rdfindex/ontology/weight> "0.1"^^<http://www.w3.org/2001/XMLSchema#double>.
_:bnode1365351936 <http://purl.org/weso/rdfindex/ontology/part-of> _:bnode1892175232.
_:bnode1373455168 <http://purl.org/weso/rdfindex/ontology/dataset> <http://purl.org/weso/cloudindex/indicator/PoliticalConstraint>.
_:bnode1373455168 <http://purl.org/weso/rdfindex/ontology/weight> "0.1"^^<http://www.w3.org/2001/XMLSchema#double>.
_:bnode1365351936 <http://purl.org/weso/rdfindex/ontology/part-of> _:bnode1373455168.
_:bnode854735104 <http://purl.org/weso/rdfindex/ontology/dataset> <http://purl.org/weso/cloudindex/indicator/DataIntegrity>.
_:bnode854735104 <http://purl.org/weso/rdfindex/ontology/weight> "0.1"^^<http://www.w3.org/2001/XMLSchema#double>.
_:bnode1365351936 <http://purl.org/weso/rdfindex/ontology/part-of> _:bnode854735104.
_:bnode336015040 <http://purl.org/weso/rdfindex/ontology/dataset> <http://purl.org/weso/cloudindex/indicator/DataPrivacy>.
_:bnode336015040 <http://purl.org/weso/rdfindex/ontology/weight> "0.1"^^<http://www.w3.org/2001/XMLSchema#double>.
_:bnode1365351936 <http://purl.org/weso/rdfindex/ontology/part-of> _:bnode336015040.
_:bnode182705024 <http://purl.org/weso/rdfindex/ontology/dataset> <http://purl.org/weso/cloudindex/indicator/DataPrivacy>.
_:bnode182705024 <http://purl.org/weso/rdfindex/ontology/weight> "0.1"^^<http://www.w3.org/2001/XMLSchema#double>.
_:bnode1365351936 <http://purl.org/weso/rdfindex/ontology/part-of> _:bnode182705024.
_:bnode701425088 <http://purl.org/weso/rdfindex/ontology/dataset> <http://purl.org/weso/cloudindex/indicator/DataLoss>.
_:bnode701425088 <http://purl.org/weso/rdfindex/ontology/weight> "0.1"^^<http://www.w3.org/2001/XMLSchema#double>.
_:bnode1365351936 <http://purl.org/weso/rdfindex/ontology/part-of> _:bnode701425088.
_:bnode1220145152 <http://purl.org/weso/rdfindex/ontology/dataset> <http://purl.org/weso/cloudindex/indicator/EnvironmentSecurity>.
_:bnode1220145152 <http://purl.org/weso/rdfindex/ontology/weight> "0.1"^^<http://www.w3.org/2001/XMLSchema#double>.
_:bnode1365351936 <http://purl.org/weso/rdfindex/ontology/part-of> _:bnode1220145152.
_:bnode1738865216 <http://purl.org/weso/rdfindex/ontology/dataset> <http://purl.org/weso/cloudindex/indicator/ProactiveThreat>.
_:bnode1738865216 <http://purl.org/weso/rdfindex/ontology/weight> "0.1"^^<http://www.w3.org/2001/XMLSchema#double>.
_:bnode1365351936 <http://purl.org/weso/rdfindex/ontology/part-of> _:bnode1738865216.
_:bnode2037382016 <http://purl.org/weso/rdfindex/ontology/dataset> <http://purl.org/weso/cloudindex/indicator/Retention>.
_:bnode2037382016 <http://purl.org/weso/rdfindex/ontology/weight> "0.1"^^<http://www.w3.org/2001/XMLSchema#double>.
_:bnode1365351936 <http://purl.org/weso/rdfindex/ontology/part-of> _:bnode2037382016.
_:bnode1518661952 <http://purl.org/weso/rdfindex/ontology/dataset> <http://purl.org/weso/cloudindex/indicator/Disposition>.
_:bnode1518661952 <http://purl.org/weso/rdfindex/ontology/weight> "0.1"^^<http://www.w3.org/2001/XMLSchema#double>.
_:bnode1365351936 <http://purl.org/weso/rdfindex/ontology/part-of> _:bnode1518661952.
<http://purl.org/weso/cloudindex/component/SecurityPrivacy> <http://purl.org/weso/rdfindex/ontology/aggregates> _:bnode1365351936.
<http://purl.org/weso/cloudindex/component/SecurityPrivacy> <http://purl.org/linked-data/cube#structure> <http://purl.org/weso/cloudindex/SecurityPrivacyDSD>.
<http://purl.org/weso/cloudindex/component/SecurityPrivacy> <http://www.w3.org/2004/02/skos/core#narrower> <http://purl.org/weso/cloudindex/indicator/AccessControl>.
<http://purl.org/weso/cloudindex/component/SecurityPrivacy> <http://www.w3.org/2004/02/skos/core#narrower> <http://purl.org/weso/cloudindex/indicator/GeographicalConstraint>.
<http://purl.org/weso/cloudindex/component/SecurityPrivacy> <http://www.w3.org/2004/02/skos/core#narrower> <http://purl.org/weso/cloudindex/indicator/PoliticalConstraint>.
<http://purl.org/weso/cloudindex/component/SecurityPrivacy> <http://www.w3.org/2004/02/skos/core#narrower> <http://purl.org/weso/cloudindex/indicator/DataIntegrity>.
<http://purl.org/weso/cloudindex/component/SecurityPrivacy> <http://www.w3.org/2004/02/skos/core#narrower> <http://purl.org/weso/cloudindex/indicator/DataPrivacy>.
<http://purl.org/weso/cloudindex/component/SecurityPrivacy> <http://www.w3.org/2004/02/skos/core#narrower> <http://purl.org/weso/cloudindex/indicator/DataLoss>.
<http://purl.org/weso/cloudindex/component/SecurityPrivacy> <http://www.w3.org/2004/02/skos/core#narrower> <http://purl.org/weso/cloudindex/indicator/EnvironmentSecurity>.
<http://purl.org/weso/cloudindex/component/SecurityPrivacy> <http://www.w3.org/2004/02/skos/core#narrower> <http://purl.org/weso/cloudindex/indicator/ProactiveThreat>.
<http://purl.org/weso/cloudindex/component/SecurityPrivacy> <http://www.w3.org/2004/02/skos/core#narrower> <http://purl.org/weso/cloudindex/indicator/Retention>.
<http://purl.org/weso/cloudindex/component/SecurityPrivacy> <http://www.w3.org/2004/02/skos/core#narrower> <http://purl.org/weso/cloudindex/indicator/Disposition>.
<http://purl.org/weso/cloudindex/component/Usability> <http://www.w3.org/1999/02/22-rdf-syntax-ns#type> <http://purl.org/weso/rdfindex/ontology/Component>.
<http://purl.org/weso/cloudindex/component/Usability> <http://www.w3.org/2000/01/rdf-schema#label> "Usability"@en.
<http://purl.org/weso/cloudindex/component/Usability> <http://www.w3.org/2000/01/rdf-schema#comment> "The ease with which a service can be used."@en.
<http://purl.org/weso/cloudindex/component/Usability> <http://purl.org/weso/cloudindex/ontology/defined-in> <http://csmic.org/wp-content/uploads/2011/09/SMI-Overview-110913_v1F.pdf>.
<http://purl.org/weso/cloudindex/component/Usability> <http://purl.org/weso/cloudindex/ontology/defined-by> <http://purl.org/weso/cloudindex/organization/CSMIC>.
<http://purl.org/weso/cloudindex/component/Usability> <http://purl.org/weso/cloudindex/ontology/weight> "1"^^<http://www.w3.org/2001/XMLSchema#double>.
_:bnode999941888 <http://purl.org/weso/rdfindex/ontology/aggregation-operator> <http://purl.org/weso/rdfindex/ontology/OWA>.
_:bnode481221824 <http://purl.org/weso/rdfindex/ontology/dataset> <http://purl.org/weso/cloudindex/indicator/Accessibility>.
_:bnode481221824 <http://purl.org/weso/rdfindex/ontology/weight> "0.125"^^<http://www.w3.org/2001/XMLSchema#double>.
_:bnode999941888 <http://purl.org/weso/rdfindex/ontology/part-of> _:bnode481221824.
_:bnode37498240 <http://purl.org/weso/rdfindex/ontology/dataset> <http://purl.org/weso/cloudindex/indicator/ClientPersonnelRequirements>.
_:bnode37498240 <http://purl.org/weso/rdfindex/ontology/weight> "0.125"^^<http://www.w3.org/2001/XMLSchema#double>.
_:bnode999941888 <http://purl.org/weso/rdfindex/ontology/part-of> _:bnode37498240.
_:bnode556218304 <http://purl.org/weso/rdfindex/ontology/dataset> <http://purl.org/weso/cloudindex/indicator/Installability>.
_:bnode556218304 <http://purl.org/weso/rdfindex/ontology/weight> "0.125"^^<http://www.w3.org/2001/XMLSchema#double>.
_:bnode999941888 <http://purl.org/weso/rdfindex/ontology/part-of> _:bnode556218304.
_:bnode1074938368 <http://purl.org/weso/rdfindex/ontology/dataset> <http://purl.org/weso/cloudindex/indicator/Learnability>.
_:bnode1074938368 <http://purl.org/weso/rdfindex/ontology/weight> "0.125"^^<http://www.w3.org/2001/XMLSchema#double>.
_:bnode999941888 <http://purl.org/weso/rdfindex/ontology/part-of> _:bnode1074938368.
_:bnode1593658432 <http://purl.org/weso/rdfindex/ontology/dataset> <http://purl.org/weso/cloudindex/indicator/Operability>.
_:bnode1593658432 <http://purl.org/weso/rdfindex/ontology/weight> "0.125"^^<http://www.w3.org/2001/XMLSchema#double>.
_:bnode999941888 <http://purl.org/weso/rdfindex/ontology/part-of> _:bnode1593658432.
_:bnode2112378496 <http://purl.org/weso/rdfindex/ontology/dataset> <http://purl.org/weso/cloudindex/indicator/Suitability>.
_:bnode2112378496 <http://purl.org/weso/rdfindex/ontology/weight> "0.125"^^<http://www.w3.org/2001/XMLSchema#double>.
_:bnode999941888 <http://purl.org/weso/rdfindex/ontology/part-of> _:bnode2112378496.
_:bnode1663868736 <http://purl.org/weso/rdfindex/ontology/dataset> <http://purl.org/weso/cloudindex/indicator/Transparency>.
_:bnode1663868736 <http://purl.org/weso/rdfindex/ontology/weight> "0.125"^^<http://www.w3.org/2001/XMLSchema#double>.
_:bnode999941888 <http://purl.org/weso/rdfindex/ontology/part-of> _:bnode1663868736.
_:bnode1145148672 <http://purl.org/weso/rdfindex/ontology/dataset> <http://purl.org/weso/cloudindex/indicator/Understandability>.
_:bnode1145148672 <http://purl.org/weso/rdfindex/ontology/weight> "0.125"^^<http://www.w3.org/2001/XMLSchema#double>.
_:bnode999941888 <http://purl.org/weso/rdfindex/ontology/part-of> _:bnode1145148672.
<http://purl.org/weso/cloudindex/component/Usability> <http://purl.org/weso/rdfindex/ontology/aggregates> _:bnode999941888.
<http://purl.org/weso/cloudindex/component/Usability> <http://purl.org/linked-data/cube#structure> <http://purl.org/weso/cloudindex/UsabilityDSD>.
<http://purl.org/weso/cloudindex/component/Usability> <http://www.w3.org/2004/02/skos/core#narrower> <http://purl.org/weso/cloudindex/indicator/Accessibility>.
<http://purl.org/weso/cloudindex/component/Usability> <http://www.w3.org/2004/02/skos/core#narrower> <http://purl.org/weso/cloudindex/indicator/ClientPersonnelRequirements>.
<http://purl.org/weso/cloudindex/component/Usability> <http://www.w3.org/2004/02/skos/core#narrower> <http://purl.org/weso/cloudindex/indicator/Installability>.
<http://purl.org/weso/cloudindex/component/Usability> <http://www.w3.org/2004/02/skos/core#narrower> <http://purl.org/weso/cloudindex/indicator/Learnability>.
<http://purl.org/weso/cloudindex/component/Usability> <http://www.w3.org/2004/02/skos/core#narrower> <http://purl.org/weso/cloudindex/indicator/Operability>.
<http://purl.org/weso/cloudindex/component/Usability> <http://www.w3.org/2004/02/skos/core#narrower> <http://purl.org/weso/cloudindex/indicator/Suitability>.
<http://purl.org/weso/cloudindex/component/Usability> <http://www.w3.org/2004/02/skos/core#narrower> <http://purl.org/weso/cloudindex/indicator/Transparency>.
<http://purl.org/weso/cloudindex/component/Usability> <http://www.w3.org/2004/02/skos/core#narrower> <http://purl.org/weso/cloudindex/indicator/Understandability>.
<http://purl.org/weso/cloudindex/indicator/ds> <http://www.w3.org/1999/02/22-rdf-syntax-ns#type> <http://rdfs.org/ns/void#Dataset>.
<http://purl.org/weso/cloudindex/indicator/ds> <http://www.w3.org/2000/01/rdf-schema#label> "SEERC| CloudIndex | Indicators"@en.
<http://purl.org/weso/cloudindex/indicator/ds> <http://www.w3.org/2000/01/rdf-schema#comment> "Indicators used to retrieve observations according to the different dimensions. They can also be taken as measures."@en.
<http://purl.org/weso/cloudindex/indicator/ds> <http://purl.org/dc/terms/created> "2013-05-20"^^<http://www.w3.org/2001/XMLSchema#date>.
<http://purl.org/weso/cloudindex/indicator/ds> <http://purl.org/dc/terms/modified> "2013-06-20-"^^<http://www.w3.org/2001/XMLSchema#date>.
<http://purl.org/weso/cloudindex/indicator/ds> <http://purl.org/dc/terms/title> "Indicators of Core CloudIndex ontology"@en.
<http://purl.org/weso/cloudindex/indicator/ds> <http://purl.org/dc/terms/author> <http://purl.org/weso/cloudindex/people/Chema>.
<http://purl.org/weso/cloudindex/indicator/ds> <http://purl.org/dc/terms/author> <http://purl.org/weso/rdfindex/organization/SEERC>.
<http://purl.org/weso/cloudindex/indicator/ds> <http://purl.org/dc/terms/publisher> <http://purl.org/weso/cloudindex/people/Chema>.
<http://purl.org/weso/cloudindex/indicator/ds> <http://purl.org/dc/terms/contributor> <http://purl.org/weso/rdfindex/organization/SEERC>.
<http://purl.org/weso/cloudindex/indicator/ds> <http://purl.org/dc/terms/contributor> <http://purl.org/weso/rdfindex/project/RELATE>.
<http://purl.org/weso/cloudindex/indicator/ds> <http://purl.org/dc/terms/license> <http://opendatacommons.org/licenses/by/1.0/>.
<http://purl.org/weso/cloudindex/indicator/ds> <http://rdfs.org/ns/void#exampleResource> <http://purl.org/weso/cloudindex/component/CommunicationsInfrastructure>.
<http://purl.org/weso/cloudindex/indicator/ds> <http://rdfs.org/ns/void#uriRegexPattern> "http://purl.org/weso/cloudindex/indicator/.+".
<http://purl.org/weso/cloudindex/indicator/ds> <http://rdfs.org/ns/void#vocabulary> <http://www.w3.org/2000/01/rdf-schema#>.
<http://purl.org/weso/cloudindex/indicator/ds> <http://rdfs.org/ns/void#vocabulary> <http://www.w3.org/2004/02/skos/core#>.
<http://purl.org/weso/cloudindex/indicator/ds> <http://xmlns.com/foaf/0.1/homepage> <http://purl.org/weso/cloudindex/>.
<http://purl.org/weso/cloudindex/indicator/Auditability> <http://www.w3.org/1999/02/22-rdf-syntax-ns#type> <http://purl.org/weso/cloudindex/ontology/KPIIndicator>.
<http://purl.org/weso/cloudindex/indicator/Auditability> <http://www.w3.org/2000/01/rdf-schema#label> "Auditability"@en.
<http://purl.org/weso/cloudindex/indicator/Auditability> <http://www.w3.org/2000/01/rdf-schema#comment> "The ability of a client to verify that the service provider is adhering to the standards, processes, and policies that they follow."@en.
<http://purl.org/weso/cloudindex/indicator/Auditability> <http://www.w3.org/2004/02/skos/core#definition> "The ability of a client to verify that the service provider is adhering to the standards, processes, and policies that they follow."@en.
<http://purl.org/weso/cloudindex/indicator/Auditability> <http://purl.org/weso/cloudindex/ontology/defined-in> <http://csmic.org/wp-content/uploads/2011/09/SMI-Overview-110913_v1F.pdf>.
<http://purl.org/weso/cloudindex/indicator/Auditability> <http://purl.org/weso/cloudindex/ontology/defined-by> <http://purl.org/weso/cloudindex/organization/CSMIC>.
<http://purl.org/weso/cloudindex/indicator/Auditability> <http://purl.org/weso/cloudindex/ontology/weight> "1.0"^^<http://www.w3.org/2001/XMLSchema#double>.
<http://purl.org/weso/cloudindex/indicator/Auditability> <http://purl.org/weso/cloudindex/ontology/pref-value> <http://purl.org/weso/cloudindex/ontology/High>.
<http://purl.org/weso/cloudindex/indicator/Auditability> <http://www.w3.org/2004/02/skos/core#notation> "Auditability".
<http://purl.org/weso/cloudindex/indicator/Auditability> <http://www.w3.org/2006/time#intervalStarts> "2013"^^<http://www.w3.org/2001/XMLSchema#int>.
<http://purl.org/weso/cloudindex/indicator/Auditability> <http://www.w3.org/2006/time#intervalFinishes> "2013"^^<http://www.w3.org/2001/XMLSchema#int>.
<http://purl.org/weso/cloudindex/indicator/Auditability> <http://www.w3.org/2004/02/skos/core#broader> <http://purl.org/weso/cloudindex/component/Accountability>.
<http://purl.org/weso/cloudindex/indicator/Compliance> <http://www.w3.org/1999/02/22-rdf-syntax-ns#type> <http://purl.org/weso/cloudindex/ontology/KPIIndicator>.
<http://purl.org/weso/cloudindex/indicator/Compliance> <http://www.w3.org/2000/01/rdf-schema#label> "Compliance"@en.
<http://purl.org/weso/cloudindex/indicator/Compliance> <http://www.w3.org/2000/01/rdf-schema#comment> "Standards, processes, and policies committed to by the service provider are followed."@en.
<http://purl.org/weso/cloudindex/indicator/Compliance> <http://www.w3.org/2004/02/skos/core#definition> "Standards, processes, and policies committed to by the service provider are followed."@en.
<http://purl.org/weso/cloudindex/indicator/Compliance> <http://purl.org/weso/cloudindex/ontology/defined-in> <http://csmic.org/wp-content/uploads/2011/09/SMI-Overview-110913_v1F.pdf>.
<http://purl.org/weso/cloudindex/indicator/Compliance> <http://purl.org/weso/cloudindex/ontology/defined-by> <http://purl.org/weso/cloudindex/organization/CSMIC>.
<http://purl.org/weso/cloudindex/indicator/Compliance> <http://purl.org/weso/cloudindex/ontology/weight> "1.0"^^<http://www.w3.org/2001/XMLSchema#double>.
<http://purl.org/weso/cloudindex/indicator/Compliance> <http://purl.org/weso/cloudindex/ontology/pref-value> <http://purl.org/weso/cloudindex/ontology/High>.
<http://purl.org/weso/cloudindex/indicator/Compliance> <http://www.w3.org/2004/02/skos/core#notation> "Compliance".
<http://purl.org/weso/cloudindex/indicator/Compliance> <http://www.w3.org/2006/time#intervalStarts> "2013"^^<http://www.w3.org/2001/XMLSchema#int>.
<http://purl.org/weso/cloudindex/indicator/Compliance> <http://www.w3.org/2006/time#intervalFinishes> "2013"^^<http://www.w3.org/2001/XMLSchema#int>.
<http://purl.org/weso/cloudindex/indicator/Compliance> <http://www.w3.org/2004/02/skos/core#broader> <http://purl.org/weso/cloudindex/component/Accountability>.
<http://purl.org/weso/cloudindex/indicator/ContractingExperience> <http://www.w3.org/1999/02/22-rdf-syntax-ns#type> <http://purl.org/weso/cloudindex/ontology/KPIIndicator>.
<http://purl.org/weso/cloudindex/indicator/ContractingExperience> <http://www.w3.org/2000/01/rdf-schema#label> "Contracting Experience"@en.
<http://purl.org/weso/cloudindex/indicator/ContractingExperience> <http://www.w3.org/2000/01/rdf-schema#comment> "Indicators of client effort and satisfaction with the process of entering into the agreements required to use a service."@en.
<http://purl.org/weso/cloudindex/indicator/ContractingExperience> <http://www.w3.org/2004/02/skos/core#definition> "Indicators of client effort and satisfaction with the process of entering into the agreements required to use a service."@en.
<http://purl.org/weso/cloudindex/indicator/ContractingExperience> <http://purl.org/weso/cloudindex/ontology/defined-in> <http://csmic.org/wp-content/uploads/2011/09/SMI-Overview-110913_v1F.pdf>.
<http://purl.org/weso/cloudindex/indicator/ContractingExperience> <http://purl.org/weso/cloudindex/ontology/defined-by> <http://purl.org/weso/cloudindex/organization/CSMIC>.
<http://purl.org/weso/cloudindex/indicator/ContractingExperience> <http://purl.org/weso/cloudindex/ontology/weight> "1.0"^^<http://www.w3.org/2001/XMLSchema#double>.
<http://purl.org/weso/cloudindex/indicator/ContractingExperience> <http://purl.org/weso/cloudindex/ontology/pref-value> <http://purl.org/weso/cloudindex/ontology/High>.
<http://purl.org/weso/cloudindex/indicator/ContractingExperience> <http://www.w3.org/2004/02/skos/core#notation> "ContractingExperience".
<http://purl.org/weso/cloudindex/indicator/ContractingExperience> <http://www.w3.org/2006/time#intervalStarts> "2013"^^<http://www.w3.org/2001/XMLSchema#int>.
<http://purl.org/weso/cloudindex/indicator/ContractingExperience> <http://www.w3.org/2006/time#intervalFinishes> "2013"^^<http://www.w3.org/2001/XMLSchema#int>.
<http://purl.org/weso/cloudindex/indicator/ContractingExperience> <http://www.w3.org/2004/02/skos/core#broader> <http://purl.org/weso/cloudindex/component/Accountability>.
<http://purl.org/weso/cloudindex/indicator/DataOwnership> <http://www.w3.org/1999/02/22-rdf-syntax-ns#type> <http://purl.org/weso/cloudindex/ontology/KPIIndicator>.
<http://purl.org/weso/cloudindex/indicator/DataOwnership> <http://www.w3.org/2000/01/rdf-schema#label> "Data Ownership"@en.
<http://purl.org/weso/cloudindex/indicator/DataOwnership> <http://www.w3.org/2000/01/rdf-schema#comment> "The Level of rights a client has over client data associated with a service."@en.
<http://purl.org/weso/cloudindex/indicator/DataOwnership> <http://www.w3.org/2004/02/skos/core#definition> "The Level of rights a client has over client data associated with a service."@en.
<http://purl.org/weso/cloudindex/indicator/DataOwnership> <http://purl.org/weso/cloudindex/ontology/defined-in> <http://csmic.org/wp-content/uploads/2011/09/SMI-Overview-110913_v1F.pdf>.
<http://purl.org/weso/cloudindex/indicator/DataOwnership> <http://purl.org/weso/cloudindex/ontology/defined-by> <http://purl.org/weso/cloudindex/organization/CSMIC>.
<http://purl.org/weso/cloudindex/indicator/DataOwnership> <http://purl.org/weso/cloudindex/ontology/weight> "1.0"^^<http://www.w3.org/2001/XMLSchema#double>.
<http://purl.org/weso/cloudindex/indicator/DataOwnership> <http://purl.org/weso/cloudindex/ontology/pref-value> <http://purl.org/weso/cloudindex/ontology/High>.
<http://purl.org/weso/cloudindex/indicator/DataOwnership> <http://www.w3.org/2004/02/skos/core#notation> "DataOwnership".
<http://purl.org/weso/cloudindex/indicator/DataOwnership> <http://www.w3.org/2006/time#intervalStarts> "2013"^^<http://www.w3.org/2001/XMLSchema#int>.
<http://purl.org/weso/cloudindex/indicator/DataOwnership> <http://www.w3.org/2006/time#intervalFinishes> "2013"^^<http://www.w3.org/2001/XMLSchema#int>.
<http://purl.org/weso/cloudindex/indicator/DataOwnership> <http://www.w3.org/2004/02/skos/core#broader> <http://purl.org/weso/cloudindex/component/Accountability>.
<http://purl.org/weso/cloudindex/indicator/EaseDoingBusiness> <http://www.w3.org/1999/02/22-rdf-syntax-ns#type> <http://purl.org/weso/cloudindex/ontology/KPIIndicator>.
<http://purl.org/weso/cloudindex/indicator/EaseDoingBusiness> <http://www.w3.org/2000/01/rdf-schema#label> "Ease of Doing Business"@en.
<http://purl.org/weso/cloudindex/indicator/EaseDoingBusiness> <http://www.w3.org/2000/01/rdf-schema#comment> "Client satisfaction with the ability to do business with a service provider."@en.
<http://purl.org/weso/cloudindex/indicator/EaseDoingBusiness> <http://www.w3.org/2004/02/skos/core#definition> "Client satisfaction with the ability to do business with a service provider."@en.
<http://purl.org/weso/cloudindex/indicator/EaseDoingBusiness> <http://purl.org/weso/cloudindex/ontology/defined-in> <http://csmic.org/wp-content/uploads/2011/09/SMI-Overview-110913_v1F.pdf>.
<http://purl.org/weso/cloudindex/indicator/EaseDoingBusiness> <http://purl.org/weso/cloudindex/ontology/defined-by> <http://purl.org/weso/cloudindex/organization/CSMIC>.
<http://purl.org/weso/cloudindex/indicator/EaseDoingBusiness> <http://purl.org/weso/cloudindex/ontology/weight> "1.0"^^<http://www.w3.org/2001/XMLSchema#double>.
<http://purl.org/weso/cloudindex/indicator/EaseDoingBusiness> <http://purl.org/weso/cloudindex/ontology/pref-value> <http://purl.org/weso/cloudindex/ontology/High>.
<http://purl.org/weso/cloudindex/indicator/EaseDoingBusiness> <http://www.w3.org/2004/02/skos/core#notation> "EaseDoingBusiness".
<http://purl.org/weso/cloudindex/indicator/EaseDoingBusiness> <http://www.w3.org/2006/time#intervalStarts> "2013"^^<http://www.w3.org/2001/XMLSchema#int>.
<http://purl.org/weso/cloudindex/indicator/EaseDoingBusiness> <http://www.w3.org/2006/time#intervalFinishes> "2013"^^<http://www.w3.org/2001/XMLSchema#int>.
<http://purl.org/weso/cloudindex/indicator/EaseDoingBusiness> <http://www.w3.org/2004/02/skos/core#broader> <http://purl.org/weso/cloudindex/component/Accountability>.
<http://purl.org/weso/cloudindex/indicator/Governance> <http://www.w3.org/1999/02/22-rdf-syntax-ns#type> <http://purl.org/weso/cloudindex/ontology/KPIIndicator>.
<http://purl.org/weso/cloudindex/indicator/Governance> <http://www.w3.org/2000/01/rdf-schema#label> "Ease of Doing Business"@en.
<http://purl.org/weso/cloudindex/indicator/Governance> <http://www.w3.org/2000/01/rdf-schema#comment> "The processes used by the service provider to manage client expectations, issues and service performance."@en.
<http://purl.org/weso/cloudindex/indicator/Governance> <http://www.w3.org/2004/02/skos/core#definition> "The processes used by the service provider to manage client expectations, issues and service performance."@en.
<http://purl.org/weso/cloudindex/indicator/Governance> <http://purl.org/weso/cloudindex/ontology/defined-in> <http://csmic.org/wp-content/uploads/2011/09/SMI-Overview-110913_v1F.pdf>.
<http://purl.org/weso/cloudindex/indicator/Governance> <http://purl.org/weso/cloudindex/ontology/defined-by> <http://purl.org/weso/cloudindex/organization/CSMIC>.
<http://purl.org/weso/cloudindex/indicator/Governance> <http://purl.org/weso/cloudindex/ontology/weight> "1.0"^^<http://www.w3.org/2001/XMLSchema#double>.
<http://purl.org/weso/cloudindex/indicator/Governance> <http://purl.org/weso/cloudindex/ontology/pref-value> <http://purl.org/weso/cloudindex/ontology/High>.
<http://purl.org/weso/cloudindex/indicator/Governance> <http://www.w3.org/2004/02/skos/core#notation> "Governance".
<http://purl.org/weso/cloudindex/indicator/Governance> <http://www.w3.org/2006/time#intervalStarts> "2013"^^<http://www.w3.org/2001/XMLSchema#int>.
<http://purl.org/weso/cloudindex/indicator/Governance> <http://www.w3.org/2006/time#intervalFinishes> "2013"^^<http://www.w3.org/2001/XMLSchema#int>.
<http://purl.org/weso/cloudindex/indicator/Governance> <http://www.w3.org/2004/02/skos/core#broader> <http://purl.org/weso/cloudindex/component/Accountability>.
<http://purl.org/weso/cloudindex/indicator/Ownership> <http://www.w3.org/1999/02/22-rdf-syntax-ns#type> <http://purl.org/weso/cloudindex/ontology/KPIIndicator>.
<http://purl.org/weso/cloudindex/indicator/Ownership> <http://www.w3.org/2000/01/rdf-schema#label> "Ownership"@en.
<http://purl.org/weso/cloudindex/indicator/Ownership> <http://www.w3.org/2000/01/rdf-schema#comment> "The level of rights a client has over software licenses, intellectual property and data associated with a service."@en.
<http://purl.org/weso/cloudindex/indicator/Ownership> <http://www.w3.org/2004/02/skos/core#definition> "The level of rights a client has over software licenses, intellectual property and data associated with a service."@en.
<http://purl.org/weso/cloudindex/indicator/Ownership> <http://purl.org/weso/cloudindex/ontology/defined-in> <http://csmic.org/wp-content/uploads/2011/09/SMI-Overview-110913_v1F.pdf>.
<http://purl.org/weso/cloudindex/indicator/Ownership> <http://purl.org/weso/cloudindex/ontology/defined-by> <http://purl.org/weso/cloudindex/organization/CSMIC>.
<http://purl.org/weso/cloudindex/indicator/Ownership> <http://purl.org/weso/cloudindex/ontology/weight> "1.0"^^<http://www.w3.org/2001/XMLSchema#double>.
<http://purl.org/weso/cloudindex/indicator/Ownership> <http://purl.org/weso/cloudindex/ontology/pref-value> <http://purl.org/weso/cloudindex/ontology/High>.
<http://purl.org/weso/cloudindex/indicator/Ownership> <http://www.w3.org/2004/02/skos/core#notation> "Ownership".
<http://purl.org/weso/cloudindex/indicator/Ownership> <http://www.w3.org/2006/time#intervalStarts> "2013"^^<http://www.w3.org/2001/XMLSchema#int>.
<http://purl.org/weso/cloudindex/indicator/Ownership> <http://www.w3.org/2006/time#intervalFinishes> "2013"^^<http://www.w3.org/2001/XMLSchema#int>.
<http://purl.org/weso/cloudindex/indicator/Ownership> <http://www.w3.org/2004/02/skos/core#broader> <http://purl.org/weso/cloudindex/component/Accountability>.
<http://purl.org/weso/cloudindex/indicator/ProviderStability> <http://www.w3.org/1999/02/22-rdf-syntax-ns#type> <http://purl.org/weso/cloudindex/ontology/KPIIndicator>.
<http://purl.org/weso/cloudindex/indicator/ProviderStability> <http://www.w3.org/2000/01/rdf-schema#label> "Provider business stability"@en.
<http://purl.org/weso/cloudindex/indicator/ProviderStability> <http://www.w3.org/2000/01/rdf-schema#comment> "The likelihood that the service provider will continue to exist throughout the contracted term."@en.
<http://purl.org/weso/cloudindex/indicator/ProviderStability> <http://www.w3.org/2004/02/skos/core#definition> "The likelihood that the service provider will continue to exist throughout the contracted term."@en.
<http://purl.org/weso/cloudindex/indicator/ProviderStability> <http://purl.org/weso/cloudindex/ontology/defined-in> <http://csmic.org/wp-content/uploads/2011/09/SMI-Overview-110913_v1F.pdf>.
<http://purl.org/weso/cloudindex/indicator/ProviderStability> <http://purl.org/weso/cloudindex/ontology/defined-by> <http://purl.org/weso/cloudindex/organization/CSMIC>.
<http://purl.org/weso/cloudindex/indicator/ProviderStability> <http://purl.org/weso/cloudindex/ontology/weight> "1.0"^^<http://www.w3.org/2001/XMLSchema#double>.
<http://purl.org/weso/cloudindex/indicator/ProviderStability> <http://purl.org/weso/cloudindex/ontology/pref-value> <http://purl.org/weso/cloudindex/ontology/High>.
<http://purl.org/weso/cloudindex/indicator/ProviderStability> <http://www.w3.org/2004/02/skos/core#notation> "ProviderStability".
<http://purl.org/weso/cloudindex/indicator/ProviderStability> <http://www.w3.org/2006/time#intervalStarts> "2013"^^<http://www.w3.org/2001/XMLSchema#int>.
<http://purl.org/weso/cloudindex/indicator/ProviderStability> <http://www.w3.org/2006/time#intervalFinishes> "2013"^^<http://www.w3.org/2001/XMLSchema#int>.
<http://purl.org/weso/cloudindex/indicator/ProviderStability> <http://www.w3.org/2004/02/skos/core#broader> <http://purl.org/weso/cloudindex/component/Accountability>.
<http://purl.org/weso/cloudindex/indicator/ProviderCertifications> <http://www.w3.org/1999/02/22-rdf-syntax-ns#type> <http://purl.org/weso/cloudindex/ontology/KPIIndicator>.
<http://purl.org/weso/cloudindex/indicator/ProviderCertifications> <http://www.w3.org/2000/01/rdf-schema#label> "Provider Certifications"@en.
<http://purl.org/weso/cloudindex/indicator/ProviderCertifications> <http://www.w3.org/2000/01/rdf-schema#comment> "The service provider maintains current certifications for standards relevant to their clients' requirements."@en.
<http://purl.org/weso/cloudindex/indicator/ProviderCertifications> <http://www.w3.org/2004/02/skos/core#definition> "The service provider maintains current certifications for standards relevant to their clients' requirements."@en.
<http://purl.org/weso/cloudindex/indicator/ProviderCertifications> <http://purl.org/weso/cloudindex/ontology/defined-in> <http://csmic.org/wp-content/uploads/2011/09/SMI-Overview-110913_v1F.pdf>.
<http://purl.org/weso/cloudindex/indicator/ProviderCertifications> <http://purl.org/weso/cloudindex/ontology/defined-by> <http://purl.org/weso/cloudindex/organization/CSMIC>.
<http://purl.org/weso/cloudindex/indicator/ProviderCertifications> <http://purl.org/weso/cloudindex/ontology/weight> "1.0"^^<http://www.w3.org/2001/XMLSchema#double>.
<http://purl.org/weso/cloudindex/indicator/ProviderCertifications> <http://purl.org/weso/cloudindex/ontology/pref-value> <http://purl.org/weso/cloudindex/ontology/High>.
<http://purl.org/weso/cloudindex/indicator/ProviderCertifications> <http://www.w3.org/2004/02/skos/core#notation> "ProviderCertifications".
<http://purl.org/weso/cloudindex/indicator/ProviderCertifications> <http://www.w3.org/2006/time#intervalStarts> "2013"^^<http://www.w3.org/2001/XMLSchema#int>.
<http://purl.org/weso/cloudindex/indicator/ProviderCertifications> <http://www.w3.org/2006/time#intervalFinishes> "2013"^^<http://www.w3.org/2001/XMLSchema#int>.
<http://purl.org/weso/cloudindex/indicator/ProviderCertifications> <http://www.w3.org/2004/02/skos/core#broader> <http://purl.org/weso/cloudindex/component/Accountability>.
<http://purl.org/weso/cloudindex/indicator/ProviderSLAVerification> <http://www.w3.org/1999/02/22-rdf-syntax-ns#type> <http://purl.org/weso/cloudindex/ontology/KPIIndicator>.
<http://purl.org/weso/cloudindex/indicator/ProviderSLAVerification> <http://www.w3.org/2000/01/rdf-schema#label> "Provider Contract/SLA Verification"@en.
<http://purl.org/weso/cloudindex/indicator/ProviderSLAVerification> <http://www.w3.org/2000/01/rdf-schema#comment> "The service provider makes available to clients SLAs adequate to manage the service and mitigate risks of service failure."@en.
<http://purl.org/weso/cloudindex/indicator/ProviderSLAVerification> <http://www.w3.org/2004/02/skos/core#definition> "The service provider makes available to clients SLAs adequate to manage the service and mitigate risks of service failure."@en.
<http://purl.org/weso/cloudindex/indicator/ProviderSLAVerification> <http://purl.org/weso/cloudindex/ontology/defined-in> <http://csmic.org/wp-content/uploads/2011/09/SMI-Overview-110913_v1F.pdf>.
<http://purl.org/weso/cloudindex/indicator/ProviderSLAVerification> <http://purl.org/weso/cloudindex/ontology/defined-by> <http://purl.org/weso/cloudindex/organization/CSMIC>.
<http://purl.org/weso/cloudindex/indicator/ProviderSLAVerification> <http://purl.org/weso/cloudindex/ontology/weight> "1.0"^^<http://www.w3.org/2001/XMLSchema#double>.
<http://purl.org/weso/cloudindex/indicator/ProviderSLAVerification> <http://purl.org/weso/cloudindex/ontology/pref-value> <http://purl.org/weso/cloudindex/ontology/High>.
<http://purl.org/weso/cloudindex/indicator/ProviderSLAVerification> <http://www.w3.org/2004/02/skos/core#notation> "ProviderSLAVerification".
<http://purl.org/weso/cloudindex/indicator/ProviderSLAVerification> <http://www.w3.org/2006/time#intervalStarts> "2013"^^<http://www.w3.org/2001/XMLSchema#int>.
<http://purl.org/weso/cloudindex/indicator/ProviderSLAVerification> <http://www.w3.org/2006/time#intervalFinishes> "2013"^^<http://www.w3.org/2001/XMLSchema#int>.
<http://purl.org/weso/cloudindex/indicator/ProviderSLAVerification> <http://www.w3.org/2004/02/skos/core#broader> <http://purl.org/weso/cloudindex/component/Accountability>.
<http://purl.org/weso/cloudindex/indicator/ProviderEthics> <http://www.w3.org/1999/02/22-rdf-syntax-ns#type> <http://purl.org/weso/cloudindex/ontology/KPIIndicator>.
<http://purl.org/weso/cloudindex/indicator/ProviderEthics> <http://www.w3.org/2000/01/rdf-schema#label> "Provider Ethicality"@en.
<http://purl.org/weso/cloudindex/indicator/ProviderEthics> <http://www.w3.org/2000/01/rdf-schema#comment> "Ethicality refers to the manner in which the service provider conducts business; it includes business practices and ethics outside the scope of regulatory compliance. Ethicality includes fair practices with suppliers, customers, and employees."@en.
<http://purl.org/weso/cloudindex/indicator/ProviderEthics> <http://www.w3.org/2004/02/skos/core#definition> "Ethicality refers to the manner in which the service provider conducts business; it includes business practices and ethics outside the scope of regulatory compliance. Ethicality includes fair practices with suppliers, customers, and employees."@en.
<http://purl.org/weso/cloudindex/indicator/ProviderEthics> <http://purl.org/weso/cloudindex/ontology/defined-in> <http://csmic.org/wp-content/uploads/2011/09/SMI-Overview-110913_v1F.pdf>.
<http://purl.org/weso/cloudindex/indicator/ProviderEthics> <http://purl.org/weso/cloudindex/ontology/defined-by> <http://purl.org/weso/cloudindex/organization/CSMIC>.
<http://purl.org/weso/cloudindex/indicator/ProviderEthics> <http://purl.org/weso/cloudindex/ontology/weight> "1.0"^^<http://www.w3.org/2001/XMLSchema#double>.
<http://purl.org/weso/cloudindex/indicator/ProviderEthics> <http://purl.org/weso/cloudindex/ontology/pref-value> <http://purl.org/weso/cloudindex/ontology/High>.
<http://purl.org/weso/cloudindex/indicator/ProviderEthics> <http://www.w3.org/2004/02/skos/core#notation> "ProviderEthics".
<http://purl.org/weso/cloudindex/indicator/ProviderEthics> <http://www.w3.org/2006/time#intervalStarts> "2013"^^<http://www.w3.org/2001/XMLSchema#int>.
<http://purl.org/weso/cloudindex/indicator/ProviderEthics> <http://www.w3.org/2006/time#intervalFinishes> "2013"^^<http://www.w3.org/2001/XMLSchema#int>.
<http://purl.org/weso/cloudindex/indicator/ProviderEthics> <http://www.w3.org/2004/02/skos/core#broader> <http://purl.org/weso/cloudindex/component/Accountability>.
<http://purl.org/weso/cloudindex/indicator/ProviderPersonnelRequirements> <http://www.w3.org/1999/02/22-rdf-syntax-ns#type> <http://purl.org/weso/cloudindex/ontology/KPIIndicator>.
<http://purl.org/weso/cloudindex/indicator/ProviderPersonnelRequirements> <http://www.w3.org/2000/01/rdf-schema#label> "Provider Personnel Requirements"@en.
<http://purl.org/weso/cloudindex/indicator/ProviderPersonnelRequirements> <http://www.w3.org/2000/01/rdf-schema#comment> "The extent to which service provider personnel have the skills, experience, education, and certifications required to effectively deliver a service."@en.
<http://purl.org/weso/cloudindex/indicator/ProviderPersonnelRequirements> <http://www.w3.org/2004/02/skos/core#definition> "The extent to which service provider personnel have the skills, experience, education, and certifications required to effectively deliver a service."@en.
<http://purl.org/weso/cloudindex/indicator/ProviderPersonnelRequirements> <http://purl.org/weso/cloudindex/ontology/defined-in> <http://csmic.org/wp-content/uploads/2011/09/SMI-Overview-110913_v1F.pdf>.
<http://purl.org/weso/cloudindex/indicator/ProviderPersonnelRequirements> <http://purl.org/weso/cloudindex/ontology/defined-by> <http://purl.org/weso/cloudindex/organization/CSMIC>.
<http://purl.org/weso/cloudindex/indicator/ProviderPersonnelRequirements> <http://purl.org/weso/cloudindex/ontology/weight> "1.0"^^<http://www.w3.org/2001/XMLSchema#double>.
<http://purl.org/weso/cloudindex/indicator/ProviderPersonnelRequirements> <http://purl.org/weso/cloudindex/ontology/pref-value> <http://purl.org/weso/cloudindex/ontology/High>.
<http://purl.org/weso/cloudindex/indicator/ProviderPersonnelRequirements> <http://www.w3.org/2004/02/skos/core#notation> "ProviderPersonnelRequirements".
<http://purl.org/weso/cloudindex/indicator/ProviderPersonnelRequirements> <http://www.w3.org/2006/time#intervalStarts> "2013"^^<http://www.w3.org/2001/XMLSchema#int>.
<http://purl.org/weso/cloudindex/indicator/ProviderPersonnelRequirements> <http://www.w3.org/2006/time#intervalFinishes> "2013"^^<http://www.w3.org/2001/XMLSchema#int>.
<http://purl.org/weso/cloudindex/indicator/ProviderPersonnelRequirements> <http://www.w3.org/2004/02/skos/core#broader> <http://purl.org/weso/cloudindex/component/Accountability>.
<http://purl.org/weso/cloudindex/indicator/ProviderSupplyChain> <http://www.w3.org/1999/02/22-rdf-syntax-ns#type> <http://purl.org/weso/cloudindex/ontology/KPIIndicator>.
<http://purl.org/weso/cloudindex/indicator/ProviderSupplyChain> <http://www.w3.org/2000/01/rdf-schema#label> "Provider Supply Chain"@en.
<http://purl.org/weso/cloudindex/indicator/ProviderSupplyChain> <http://www.w3.org/2000/01/rdf-schema#comment> "The service provider ensures that any SLAs that must be supported by its suppliers are supported."@en.
<http://purl.org/weso/cloudindex/indicator/ProviderSupplyChain> <http://www.w3.org/2004/02/skos/core#definition> "The service provider ensures that any SLAs that must be supported by its suppliers are supported."@en.
<http://purl.org/weso/cloudindex/indicator/ProviderSupplyChain> <http://purl.org/weso/cloudindex/ontology/defined-in> <http://csmic.org/wp-content/uploads/2011/09/SMI-Overview-110913_v1F.pdf>.
<http://purl.org/weso/cloudindex/indicator/ProviderSupplyChain> <http://purl.org/weso/cloudindex/ontology/defined-by> <http://purl.org/weso/cloudindex/organization/CSMIC>.
<http://purl.org/weso/cloudindex/indicator/ProviderSupplyChain> <http://purl.org/weso/cloudindex/ontology/weight> "1.0"^^<http://www.w3.org/2001/XMLSchema#double>.
<http://purl.org/weso/cloudindex/indicator/ProviderSupplyChain> <http://purl.org/weso/cloudindex/ontology/pref-value> <http://purl.org/weso/cloudindex/ontology/High>.
<http://purl.org/weso/cloudindex/indicator/ProviderSupplyChain> <http://www.w3.org/2004/02/skos/core#notation> "ProviderSupplyChain".
<http://purl.org/weso/cloudindex/indicator/ProviderSupplyChain> <http://www.w3.org/2006/time#intervalStarts> "2013"^^<http://www.w3.org/2001/XMLSchema#int>.
<http://purl.org/weso/cloudindex/indicator/ProviderSupplyChain> <http://www.w3.org/2006/time#intervalFinishes> "2013"^^<http://www.w3.org/2001/XMLSchema#int>.
<http://purl.org/weso/cloudindex/indicator/ProviderSupplyChain> <http://www.w3.org/2004/02/skos/core#broader> <http://purl.org/weso/cloudindex/component/Accountability>.
<http://purl.org/weso/cloudindex/indicator/ProviderSecurityCapabilities> <http://www.w3.org/1999/02/22-rdf-syntax-ns#type> <http://purl.org/weso/cloudindex/ontology/KPIIndicator>.
<http://purl.org/weso/cloudindex/indicator/ProviderSecurityCapabilities> <http://www.w3.org/2000/01/rdf-schema#label> "Security Capabilities"@en.
<http://purl.org/weso/cloudindex/indicator/ProviderSecurityCapabilities> <http://www.w3.org/2000/01/rdf-schema#comment> "The capabilities of service providers to ensure application, data, and infrastructure securiy based on the security requirements of the client."@en.
<http://purl.org/weso/cloudindex/indicator/ProviderSecurityCapabilities> <http://www.w3.org/2004/02/skos/core#definition> "The capabilities of service providers to ensure application, data, and infrastructure securiy based on the security requirements of the client."@en.
<http://purl.org/weso/cloudindex/indicator/ProviderSecurityCapabilities> <http://purl.org/weso/cloudindex/ontology/defined-in> <http://csmic.org/wp-content/uploads/2011/09/SMI-Overview-110913_v1F.pdf>.
<http://purl.org/weso/cloudindex/indicator/ProviderSecurityCapabilities> <http://purl.org/weso/cloudindex/ontology/defined-by> <http://purl.org/weso/cloudindex/organization/CSMIC>.
<http://purl.org/weso/cloudindex/indicator/ProviderSecurityCapabilities> <http://purl.org/weso/cloudindex/ontology/weight> "1.0"^^<http://www.w3.org/2001/XMLSchema#double>.
<http://purl.org/weso/cloudindex/indicator/ProviderSecurityCapabilities> <http://purl.org/weso/cloudindex/ontology/pref-value> <http://purl.org/weso/cloudindex/ontology/High>.
<http://purl.org/weso/cloudindex/indicator/ProviderSecurityCapabilities> <http://www.w3.org/2004/02/skos/core#notation> "ProviderSecurityCapabilities".
<http://purl.org/weso/cloudindex/indicator/ProviderSecurityCapabilities> <http://www.w3.org/2006/time#intervalStarts> "2013"^^<http://www.w3.org/2001/XMLSchema#int>.
<http://purl.org/weso/cloudindex/indicator/ProviderSecurityCapabilities> <http://www.w3.org/2006/time#intervalFinishes> "2013"^^<http://www.w3.org/2001/XMLSchema#int>.
<http://purl.org/weso/cloudindex/indicator/ProviderSecurityCapabilities> <http://www.w3.org/2004/02/skos/core#broader> <http://purl.org/weso/cloudindex/component/Accountability>.
<http://purl.org/weso/cloudindex/indicator/Sustainability> <http://www.w3.org/1999/02/22-rdf-syntax-ns#type> <http://purl.org/weso/cloudindex/ontology/KPIIndicator>.
<http://purl.org/weso/cloudindex/indicator/Sustainability> <http://www.w3.org/2000/01/rdf-schema#label> "Sustainability"@en.
<http://purl.org/weso/cloudindex/indicator/Sustainability> <http://www.w3.org/2000/01/rdf-schema#comment> "The impact on the economy, society and the environment of the service provider."@en.
<http://purl.org/weso/cloudindex/indicator/Sustainability> <http://www.w3.org/2004/02/skos/core#definition> "The impact on the economy, society and the environment of the service provider."@en.
<http://purl.org/weso/cloudindex/indicator/Sustainability> <http://purl.org/weso/cloudindex/ontology/defined-in> <http://csmic.org/wp-content/uploads/2011/09/SMI-Overview-110913_v1F.pdf>.
<http://purl.org/weso/cloudindex/indicator/Sustainability> <http://purl.org/weso/cloudindex/ontology/defined-by> <http://purl.org/weso/cloudindex/organization/CSMIC>.
<http://purl.org/weso/cloudindex/indicator/Sustainability> <http://purl.org/weso/cloudindex/ontology/weight> "1.0"^^<http://www.w3.org/2001/XMLSchema#double>.
<http://purl.org/weso/cloudindex/indicator/Sustainability> <http://purl.org/weso/cloudindex/ontology/pref-value> <http://purl.org/weso/cloudindex/ontology/High>.
<http://purl.org/weso/cloudindex/indicator/Sustainability> <http://www.w3.org/2004/02/skos/core#notation> "Sustainability".
<http://purl.org/weso/cloudindex/indicator/Sustainability> <http://www.w3.org/2006/time#intervalStarts> "2013"^^<http://www.w3.org/2001/XMLSchema#int>.
<http://purl.org/weso/cloudindex/indicator/Sustainability> <http://www.w3.org/2006/time#intervalFinishes> "2013"^^<http://www.w3.org/2001/XMLSchema#int>.
<http://purl.org/weso/cloudindex/indicator/Sustainability> <http://www.w3.org/2004/02/skos/core#broader> <http://purl.org/weso/cloudindex/component/Accountability>.
<http://purl.org/weso/cloudindex/indicator/Adaptability> <http://www.w3.org/1999/02/22-rdf-syntax-ns#type> <http://purl.org/weso/cloudindex/ontology/KPIIndicator>.
<http://purl.org/weso/cloudindex/indicator/Adaptability> <http://www.w3.org/2000/01/rdf-schema#label> "Adaptability"@en.
<http://purl.org/weso/cloudindex/indicator/Adaptability> <http://www.w3.org/2000/01/rdf-schema#comment> "The ability of the service provider to adjust to changes in client requirements."@en.
<http://purl.org/weso/cloudindex/indicator/Adaptability> <http://www.w3.org/2004/02/skos/core#definition> "The ability of the service provider to adjust to changes in client requirements."@en.
<http://purl.org/weso/cloudindex/indicator/Adaptability> <http://purl.org/weso/cloudindex/ontology/defined-in> <http://csmic.org/wp-content/uploads/2011/09/SMI-Overview-110913_v1F.pdf>.
<http://purl.org/weso/cloudindex/indicator/Adaptability> <http://purl.org/weso/cloudindex/ontology/defined-by> <http://purl.org/weso/cloudindex/organization/CSMIC>.
<http://purl.org/weso/cloudindex/indicator/Adaptability> <http://purl.org/weso/cloudindex/ontology/weight> "1.0"^^<http://www.w3.org/2001/XMLSchema#double>.
<http://purl.org/weso/cloudindex/indicator/Adaptability> <http://purl.org/weso/cloudindex/ontology/pref-value> <http://purl.org/weso/cloudindex/ontology/High>.
<http://purl.org/weso/cloudindex/indicator/Adaptability> <http://www.w3.org/2004/02/skos/core#notation> "Adaptability".
<http://purl.org/weso/cloudindex/indicator/Adaptability> <http://www.w3.org/2006/time#intervalStarts> "2013"^^<http://www.w3.org/2001/XMLSchema#int>.
<http://purl.org/weso/cloudindex/indicator/Adaptability> <http://www.w3.org/2006/time#intervalFinishes> "2013"^^<http://www.w3.org/2001/XMLSchema#int>.
<http://purl.org/weso/cloudindex/indicator/Adaptability> <http://www.w3.org/2004/02/skos/core#broader> <http://purl.org/weso/cloudindex/component/Agility>.
<http://purl.org/weso/cloudindex/indicator/Capacity> <http://www.w3.org/1999/02/22-rdf-syntax-ns#type> <http://purl.org/weso/cloudindex/ontology/KPIIndicator>.
<http://purl.org/weso/cloudindex/indicator/Capacity> <http://www.w3.org/2000/01/rdf-schema#label> "Capacity"@en.
<http://purl.org/weso/cloudindex/indicator/Capacity> <http://www.w3.org/2000/01/rdf-schema#comment> "The maximum amount of a service that a service provider can deliver while meeting agreed SLAs."@en.
<http://purl.org/weso/cloudindex/indicator/Capacity> <http://www.w3.org/2004/02/skos/core#definition> "The maximum amount of a service that a service provider can deliver while meeting agreed SLAs."@en.
<http://purl.org/weso/cloudindex/indicator/Capacity> <http://purl.org/weso/cloudindex/ontology/defined-in> <http://csmic.org/wp-content/uploads/2011/09/SMI-Overview-110913_v1F.pdf>.
<http://purl.org/weso/cloudindex/indicator/Capacity> <http://purl.org/weso/cloudindex/ontology/defined-by> <http://purl.org/weso/cloudindex/organization/CSMIC>.
<http://purl.org/weso/cloudindex/indicator/Capacity> <http://purl.org/weso/cloudindex/ontology/weight> "1.0"^^<http://www.w3.org/2001/XMLSchema#double>.
<http://purl.org/weso/cloudindex/indicator/Capacity> <http://purl.org/weso/cloudindex/ontology/pref-value> <http://purl.org/weso/cloudindex/ontology/High>.
<http://purl.org/weso/cloudindex/indicator/Capacity> <http://www.w3.org/2004/02/skos/core#notation> "Capacity".
<http://purl.org/weso/cloudindex/indicator/Capacity> <http://www.w3.org/2006/time#intervalStarts> "2013"^^<http://www.w3.org/2001/XMLSchema#int>.
<http://purl.org/weso/cloudindex/indicator/Capacity> <http://www.w3.org/2006/time#intervalFinishes> "2013"^^<http://www.w3.org/2001/XMLSchema#int>.
<http://purl.org/weso/cloudindex/indicator/Capacity> <http://www.w3.org/2004/02/skos/core#broader> <http://purl.org/weso/cloudindex/component/Agility>.
<http://purl.org/weso/cloudindex/indicator/Elasticity> <http://www.w3.org/1999/02/22-rdf-syntax-ns#type> <http://purl.org/weso/cloudindex/ontology/KPIIndicator>.
<http://purl.org/weso/cloudindex/indicator/Elasticity> <http://www.w3.org/2000/01/rdf-schema#label> "Elasticity"@en.
<http://purl.org/weso/cloudindex/indicator/Elasticity> <http://www.w3.org/2000/01/rdf-schema#comment> "The ability of a service to adjust its resource consumption to meet demand."@en.
<http://purl.org/weso/cloudindex/indicator/Elasticity> <http://www.w3.org/2004/02/skos/core#definition> "The ability of a service to adjust its resource consumption to meet demand."@en.
<http://purl.org/weso/cloudindex/indicator/Elasticity> <http://purl.org/weso/cloudindex/ontology/defined-in> <http://csmic.org/wp-content/uploads/2011/09/SMI-Overview-110913_v1F.pdf>.
<http://purl.org/weso/cloudindex/indicator/Elasticity> <http://purl.org/weso/cloudindex/ontology/defined-by> <http://purl.org/weso/cloudindex/organization/CSMIC>.
<http://purl.org/weso/cloudindex/indicator/Elasticity> <http://purl.org/weso/cloudindex/ontology/weight> "1.0"^^<http://www.w3.org/2001/XMLSchema#double>.
<http://purl.org/weso/cloudindex/indicator/Elasticity> <http://purl.org/weso/cloudindex/ontology/pref-value> <http://purl.org/weso/cloudindex/ontology/High>.
<http://purl.org/weso/cloudindex/indicator/Elasticity> <http://www.w3.org/2004/02/skos/core#notation> "Elasticity".
<http://purl.org/weso/cloudindex/indicator/Elasticity> <http://www.w3.org/2006/time#intervalStarts> "2013"^^<http://www.w3.org/2001/XMLSchema#int>.
<http://purl.org/weso/cloudindex/indicator/Elasticity> <http://www.w3.org/2006/time#intervalFinishes> "2013"^^<http://www.w3.org/2001/XMLSchema#int>.
<http://purl.org/weso/cloudindex/indicator/Elasticity> <http://www.w3.org/2004/02/skos/core#broader> <http://purl.org/weso/cloudindex/component/Agility>.
<http://purl.org/weso/cloudindex/indicator/Extensibility> <http://www.w3.org/1999/02/22-rdf-syntax-ns#type> <http://purl.org/weso/cloudindex/ontology/KPIIndicator>.
<http://purl.org/weso/cloudindex/indicator/Extensibility> <http://www.w3.org/2000/01/rdf-schema#label> "Extensibility"@en.
<http://purl.org/weso/cloudindex/indicator/Extensibility> <http://www.w3.org/2000/01/rdf-schema#comment> "The ability to add new features or services to existing services."@en.
<http://purl.org/weso/cloudindex/indicator/Extensibility> <http://www.w3.org/2004/02/skos/core#definition> "The ability to add new features or services to existing services."@en.
<http://purl.org/weso/cloudindex/indicator/Extensibility> <http://purl.org/weso/cloudindex/ontology/defined-in> <http://csmic.org/wp-content/uploads/2011/09/SMI-Overview-110913_v1F.pdf>.
<http://purl.org/weso/cloudindex/indicator/Extensibility> <http://purl.org/weso/cloudindex/ontology/defined-by> <http://purl.org/weso/cloudindex/organization/CSMIC>.
<http://purl.org/weso/cloudindex/indicator/Extensibility> <http://purl.org/weso/cloudindex/ontology/weight> "1.0"^^<http://www.w3.org/2001/XMLSchema#double>.
<http://purl.org/weso/cloudindex/indicator/Extensibility> <http://purl.org/weso/cloudindex/ontology/pref-value> <http://purl.org/weso/cloudindex/ontology/High>.
<http://purl.org/weso/cloudindex/indicator/Extensibility> <http://www.w3.org/2004/02/skos/core#notation> "Extensibility".
<http://purl.org/weso/cloudindex/indicator/Extensibility> <http://www.w3.org/2006/time#intervalStarts> "2013"^^<http://www.w3.org/2001/XMLSchema#int>.
<http://purl.org/weso/cloudindex/indicator/Extensibility> <http://www.w3.org/2006/time#intervalFinishes> "2013"^^<http://www.w3.org/2001/XMLSchema#int>.
<http://purl.org/weso/cloudindex/indicator/Extensibility> <http://www.w3.org/2004/02/skos/core#broader> <http://purl.org/weso/cloudindex/component/Agility>.
<http://purl.org/weso/cloudindex/indicator/Flexibility> <http://www.w3.org/1999/02/22-rdf-syntax-ns#type> <http://purl.org/weso/cloudindex/ontology/KPIIndicator>.
<http://purl.org/weso/cloudindex/indicator/Flexibility> <http://www.w3.org/2000/01/rdf-schema#label> "Flexibility"@en.
<http://purl.org/weso/cloudindex/indicator/Flexibility> <http://www.w3.org/2000/01/rdf-schema#comment> "The ability to add or remove predefined features from a service."@en.
<http://purl.org/weso/cloudindex/indicator/Flexibility> <http://www.w3.org/2004/02/skos/core#definition> "The ability to add or remove predefined features from a service."@en.
<http://purl.org/weso/cloudindex/indicator/Flexibility> <http://purl.org/weso/cloudindex/ontology/defined-in> <http://csmic.org/wp-content/uploads/2011/09/SMI-Overview-110913_v1F.pdf>.
<http://purl.org/weso/cloudindex/indicator/Flexibility> <http://purl.org/weso/cloudindex/ontology/defined-by> <http://purl.org/weso/cloudindex/organization/CSMIC>.
<http://purl.org/weso/cloudindex/indicator/Flexibility> <http://purl.org/weso/cloudindex/ontology/weight> "1.0"^^<http://www.w3.org/2001/XMLSchema#double>.
<http://purl.org/weso/cloudindex/indicator/Flexibility> <http://purl.org/weso/cloudindex/ontology/pref-value> <http://purl.org/weso/cloudindex/ontology/High>.
<http://purl.org/weso/cloudindex/indicator/Flexibility> <http://www.w3.org/2004/02/skos/core#notation> "Flexibility".
<http://purl.org/weso/cloudindex/indicator/Flexibility> <http://www.w3.org/2006/time#intervalStarts> "2013"^^<http://www.w3.org/2001/XMLSchema#int>.
<http://purl.org/weso/cloudindex/indicator/Flexibility> <http://www.w3.org/2006/time#intervalFinishes> "2013"^^<http://www.w3.org/2001/XMLSchema#int>.
<http://purl.org/weso/cloudindex/indicator/Flexibility> <http://www.w3.org/2004/02/skos/core#broader> <http://purl.org/weso/cloudindex/component/Agility>.
<http://purl.org/weso/cloudindex/indicator/Portability> <http://www.w3.org/1999/02/22-rdf-syntax-ns#type> <http://purl.org/weso/cloudindex/ontology/KPIIndicator>.
<http://purl.org/weso/cloudindex/indicator/Portability> <http://www.w3.org/2000/01/rdf-schema#label> "Portability"@en.
<http://purl.org/weso/cloudindex/indicator/Portability> <http://www.w3.org/2000/01/rdf-schema#comment> "The ability of a client to easily move a service from one service provider to another with minimal disruption."@en.
<http://purl.org/weso/cloudindex/indicator/Portability> <http://www.w3.org/2004/02/skos/core#definition> "The ability of a client to easily move a service from one service provider to another with minimal disruption."@en.
<http://purl.org/weso/cloudindex/indicator/Portability> <http://purl.org/weso/cloudindex/ontology/defined-in> <http://csmic.org/wp-content/uploads/2011/09/SMI-Overview-110913_v1F.pdf>.
<http://purl.org/weso/cloudindex/indicator/Portability> <http://purl.org/weso/cloudindex/ontology/defined-by> <http://purl.org/weso/cloudindex/organization/CSMIC>.
<http://purl.org/weso/cloudindex/indicator/Portability> <http://purl.org/weso/cloudindex/ontology/weight> "1.0"^^<http://www.w3.org/2001/XMLSchema#double>.
<http://purl.org/weso/cloudindex/indicator/Portability> <http://purl.org/weso/cloudindex/ontology/pref-value> <http://purl.org/weso/cloudindex/ontology/High>.
<http://purl.org/weso/cloudindex/indicator/Portability> <http://www.w3.org/2004/02/skos/core#notation> "Portability".
<http://purl.org/weso/cloudindex/indicator/Portability> <http://www.w3.org/2006/time#intervalStarts> "2013"^^<http://www.w3.org/2001/XMLSchema#int>.
<http://purl.org/weso/cloudindex/indicator/Portability> <http://www.w3.org/2006/time#intervalFinishes> "2013"^^<http://www.w3.org/2001/XMLSchema#int>.
<http://purl.org/weso/cloudindex/indicator/Portability> <http://www.w3.org/2004/02/skos/core#broader> <http://purl.org/weso/cloudindex/component/Agility>.
<http://purl.org/weso/cloudindex/indicator/Scalability> <http://www.w3.org/1999/02/22-rdf-syntax-ns#type> <http://purl.org/weso/cloudindex/ontology/KPIIndicator>.
<http://purl.org/weso/cloudindex/indicator/Scalability> <http://www.w3.org/2000/01/rdf-schema#label> "Scalability"@en.
<http://purl.org/weso/cloudindex/indicator/Scalability> <http://www.w3.org/2000/01/rdf-schema#comment> "The ability of a service provider to increase or decrease the amount of service available to meet client requirements."@en.
<http://purl.org/weso/cloudindex/indicator/Scalability> <http://www.w3.org/2004/02/skos/core#definition> "The ability of a service provider to increase or decrease the amount of service available to meet client requirements."@en.
<http://purl.org/weso/cloudindex/indicator/Scalability> <http://purl.org/weso/cloudindex/ontology/defined-in> <http://csmic.org/wp-content/uploads/2011/09/SMI-Overview-110913_v1F.pdf>.
<http://purl.org/weso/cloudindex/indicator/Scalability> <http://purl.org/weso/cloudindex/ontology/defined-by> <http://purl.org/weso/cloudindex/organization/CSMIC>.
<http://purl.org/weso/cloudindex/indicator/Scalability> <http://purl.org/weso/cloudindex/ontology/weight> "1.0"^^<http://www.w3.org/2001/XMLSchema#double>.
<http://purl.org/weso/cloudindex/indicator/Scalability> <http://purl.org/weso/cloudindex/ontology/pref-value> <http://purl.org/weso/cloudindex/ontology/High>.
<http://purl.org/weso/cloudindex/indicator/Scalability> <http://www.w3.org/2004/02/skos/core#notation> "Scalability".
<http://purl.org/weso/cloudindex/indicator/Scalability> <http://www.w3.org/2006/time#intervalStarts> "2013"^^<http://www.w3.org/2001/XMLSchema#int>.
<http://purl.org/weso/cloudindex/indicator/Scalability> <http://www.w3.org/2006/time#intervalFinishes> "2013"^^<http://www.w3.org/2001/XMLSchema#int>.
<http://purl.org/weso/cloudindex/indicator/Scalability> <http://www.w3.org/2004/02/skos/core#broader> <http://purl.org/weso/cloudindex/component/Agility>.
<http://purl.org/weso/cloudindex/indicator/Availability> <http://www.w3.org/1999/02/22-rdf-syntax-ns#type> <http://purl.org/weso/cloudindex/ontology/KPIIndicator>.
<http://purl.org/weso/cloudindex/indicator/Availability> <http://www.w3.org/2000/01/rdf-schema#label> "Availability"@en.
<http://purl.org/weso/cloudindex/indicator/Availability> <http://www.w3.org/2000/01/rdf-schema#comment> "The amount of time that a client can make use of a service."@en.
<http://purl.org/weso/cloudindex/indicator/Availability> <http://www.w3.org/2004/02/skos/core#definition> "The amount of time that a client can make use of a service."@en.
<http://purl.org/weso/cloudindex/indicator/Availability> <http://purl.org/weso/cloudindex/ontology/defined-in> <http://csmic.org/wp-content/uploads/2011/09/SMI-Overview-110913_v1F.pdf>.
<http://purl.org/weso/cloudindex/indicator/Availability> <http://purl.org/weso/cloudindex/ontology/defined-by> <http://purl.org/weso/cloudindex/organization/CSMIC>.
<http://purl.org/weso/cloudindex/indicator/Availability> <http://purl.org/weso/cloudindex/ontology/weight> "1.0"^^<http://www.w3.org/2001/XMLSchema#double>.
<http://purl.org/weso/cloudindex/indicator/Availability> <http://purl.org/weso/cloudindex/ontology/pref-value> <http://purl.org/weso/cloudindex/ontology/High>.
<http://purl.org/weso/cloudindex/indicator/Availability> <http://www.w3.org/2004/02/skos/core#notation> "Availability".
<http://purl.org/weso/cloudindex/indicator/Availability> <http://www.w3.org/2006/time#intervalStarts> "2013"^^<http://www.w3.org/2001/XMLSchema#int>.
<http://purl.org/weso/cloudindex/indicator/Availability> <http://www.w3.org/2006/time#intervalFinishes> "2013"^^<http://www.w3.org/2001/XMLSchema#int>.
<http://purl.org/weso/cloudindex/indicator/Availability> <http://www.w3.org/2004/02/skos/core#broader> <http://purl.org/weso/cloudindex/component/Assurance>.
<http://purl.org/weso/cloudindex/indicator/Maintainability> <http://www.w3.org/1999/02/22-rdf-syntax-ns#type> <http://purl.org/weso/cloudindex/ontology/KPIIndicator>.
<http://purl.org/weso/cloudindex/indicator/Maintainability> <http://www.w3.org/2000/01/rdf-schema#label> "Maintainability"@en.
<http://purl.org/weso/cloudindex/indicator/Maintainability> <http://www.w3.org/2000/01/rdf-schema#comment> "Maintainability refers to the ability for the service provider to make modifications to the service to keep the service in a condition of good repair."@en.
<http://purl.org/weso/cloudindex/indicator/Maintainability> <http://www.w3.org/2004/02/skos/core#definition> "Maintainability refers to the ability for the service provider to make modifications to the service to keep the service in a condition of good repair."@en.
<http://purl.org/weso/cloudindex/indicator/Maintainability> <http://purl.org/weso/cloudindex/ontology/defined-in> <http://csmic.org/wp-content/uploads/2011/09/SMI-Overview-110913_v1F.pdf>.
<http://purl.org/weso/cloudindex/indicator/Maintainability> <http://purl.org/weso/cloudindex/ontology/defined-by> <http://purl.org/weso/cloudindex/organization/CSMIC>.
<http://purl.org/weso/cloudindex/indicator/Maintainability> <http://purl.org/weso/cloudindex/ontology/weight> "1.0"^^<http://www.w3.org/2001/XMLSchema#double>.
<http://purl.org/weso/cloudindex/indicator/Maintainability> <http://purl.org/weso/cloudindex/ontology/pref-value> <http://purl.org/weso/cloudindex/ontology/High>.
<http://purl.org/weso/cloudindex/indicator/Maintainability> <http://www.w3.org/2004/02/skos/core#notation> "Maintainability".
<http://purl.org/weso/cloudindex/indicator/Maintainability> <http://www.w3.org/2006/time#intervalStarts> "2013"^^<http://www.w3.org/2001/XMLSchema#int>.
<http://purl.org/weso/cloudindex/indicator/Maintainability> <http://www.w3.org/2006/time#intervalFinishes> "2013"^^<http://www.w3.org/2001/XMLSchema#int>.
<http://purl.org/weso/cloudindex/indicator/Maintainability> <http://www.w3.org/2004/02/skos/core#broader> <http://purl.org/weso/cloudindex/component/Assurance>.
<http://purl.org/weso/cloudindex/indicator/Recoverability> <http://www.w3.org/1999/02/22-rdf-syntax-ns#type> <http://purl.org/weso/cloudindex/ontology/KPIIndicator>.
<http://purl.org/weso/cloudindex/indicator/Recoverability> <http://www.w3.org/2000/01/rdf-schema#label> "Recoverability"@en.
<http://purl.org/weso/cloudindex/indicator/Recoverability> <http://www.w3.org/2000/01/rdf-schema#comment> "Recoverability is the degree to which a service is able to quickly resume a normal state of operation after an unplanned disruption."@en.
<http://purl.org/weso/cloudindex/indicator/Recoverability> <http://www.w3.org/2004/02/skos/core#definition> "Recoverability is the degree to which a service is able to quickly resume a normal state of operation after an unplanned disruption."@en.
<http://purl.org/weso/cloudindex/indicator/Recoverability> <http://purl.org/weso/cloudindex/ontology/defined-in> <http://csmic.org/wp-content/uploads/2011/09/SMI-Overview-110913_v1F.pdf>.
<http://purl.org/weso/cloudindex/indicator/Recoverability> <http://purl.org/weso/cloudindex/ontology/defined-by> <http://purl.org/weso/cloudindex/organization/CSMIC>.
<http://purl.org/weso/cloudindex/indicator/Recoverability> <http://purl.org/weso/cloudindex/ontology/weight> "1.0"^^<http://www.w3.org/2001/XMLSchema#double>.
<http://purl.org/weso/cloudindex/indicator/Recoverability> <http://purl.org/weso/cloudindex/ontology/pref-value> <http://purl.org/weso/cloudindex/ontology/High>.
<http://purl.org/weso/cloudindex/indicator/Recoverability> <http://www.w3.org/2004/02/skos/core#notation> "Recoverability".
<http://purl.org/weso/cloudindex/indicator/Recoverability> <http://www.w3.org/2006/time#intervalStarts> "2013"^^<http://www.w3.org/2001/XMLSchema#int>.
<http://purl.org/weso/cloudindex/indicator/Recoverability> <http://www.w3.org/2006/time#intervalFinishes> "2013"^^<http://www.w3.org/2001/XMLSchema#int>.
<http://purl.org/weso/cloudindex/indicator/Recoverability> <http://www.w3.org/2004/02/skos/core#broader> <http://purl.org/weso/cloudindex/component/Assurance>.
<http://purl.org/weso/cloudindex/indicator/Reliability> <http://www.w3.org/1999/02/22-rdf-syntax-ns#type> <http://purl.org/weso/cloudindex/ontology/KPIIndicator>.
<http://purl.org/weso/cloudindex/indicator/Reliability> <http://www.w3.org/2000/01/rdf-schema#label> "Reliability"@en.
<http://purl.org/weso/cloudindex/indicator/Reliability> <http://www.w3.org/2000/01/rdf-schema#comment> "Reliability reflects measures of how a service operates without failure under\r\ngiven conditions during a given time period."@en.
<http://purl.org/weso/cloudindex/indicator/Reliability> <http://www.w3.org/2004/02/skos/core#definition> "Reliability reflects measures of how a service operates without failure under\r\ngiven conditions during a given time period."@en.
<http://purl.org/weso/cloudindex/indicator/Reliability> <http://purl.org/weso/cloudindex/ontology/defined-in> <http://csmic.org/wp-content/uploads/2011/09/SMI-Overview-110913_v1F.pdf>.
<http://purl.org/weso/cloudindex/indicator/Reliability> <http://purl.org/weso/cloudindex/ontology/defined-by> <http://purl.org/weso/cloudindex/organization/CSMIC>.
<http://purl.org/weso/cloudindex/indicator/Reliability> <http://purl.org/weso/cloudindex/ontology/weight> "1.0"^^<http://www.w3.org/2001/XMLSchema#double>.
<http://purl.org/weso/cloudindex/indicator/Reliability> <http://purl.org/weso/cloudindex/ontology/pref-value> <http://purl.org/weso/cloudindex/ontology/High>.
<http://purl.org/weso/cloudindex/indicator/Reliability> <http://www.w3.org/2004/02/skos/core#notation> "Reliability".
<http://purl.org/weso/cloudindex/indicator/Reliability> <http://www.w3.org/2006/time#intervalStarts> "2013"^^<http://www.w3.org/2001/XMLSchema#int>.
<http://purl.org/weso/cloudindex/indicator/Reliability> <http://www.w3.org/2006/time#intervalFinishes> "2013"^^<http://www.w3.org/2001/XMLSchema#int>.
<http://purl.org/weso/cloudindex/indicator/Reliability> <http://www.w3.org/2004/02/skos/core#broader> <http://purl.org/weso/cloudindex/component/Assurance>.
<http://purl.org/weso/cloudindex/indicator/Resiliency> <http://www.w3.org/1999/02/22-rdf-syntax-ns#type> <http://purl.org/weso/cloudindex/ontology/KPIIndicator>.
<http://purl.org/weso/cloudindex/indicator/Resiliency> <http://www.w3.org/2000/01/rdf-schema#label> "Resiliency"@en.
<http://purl.org/weso/cloudindex/indicator/Resiliency> <http://www.w3.org/2000/01/rdf-schema#comment> "The ability of a service to continue to operate properly in the event of a failure in\r\none or more of its components."@en.
<http://purl.org/weso/cloudindex/indicator/Resiliency> <http://www.w3.org/2004/02/skos/core#definition> "The ability of a service to continue to operate properly in the event of a failure in\r\none or more of its components."@en.
<http://purl.org/weso/cloudindex/indicator/Resiliency> <http://purl.org/weso/cloudindex/ontology/defined-in> <http://csmic.org/wp-content/uploads/2011/09/SMI-Overview-110913_v1F.pdf>.
<http://purl.org/weso/cloudindex/indicator/Resiliency> <http://purl.org/weso/cloudindex/ontology/defined-by> <http://purl.org/weso/cloudindex/organization/CSMIC>.
<http://purl.org/weso/cloudindex/indicator/Resiliency> <http://purl.org/weso/cloudindex/ontology/weight> "1.0"^^<http://www.w3.org/2001/XMLSchema#double>.
<http://purl.org/weso/cloudindex/indicator/Resiliency> <http://purl.org/weso/cloudindex/ontology/pref-value> <http://purl.org/weso/cloudindex/ontology/High>.
<http://purl.org/weso/cloudindex/indicator/Resiliency> <http://www.w3.org/2004/02/skos/core#notation> "Resiliency".
<http://purl.org/weso/cloudindex/indicator/Resiliency> <http://www.w3.org/2006/time#intervalStarts> "2013"^^<http://www.w3.org/2001/XMLSchema#int>.
<http://purl.org/weso/cloudindex/indicator/Resiliency> <http://www.w3.org/2006/time#intervalFinishes> "2013"^^<http://www.w3.org/2001/XMLSchema#int>.
<http://purl.org/weso/cloudindex/indicator/Resiliency> <http://www.w3.org/2004/02/skos/core#broader> <http://purl.org/weso/cloudindex/component/Assurance>.
<http://purl.org/weso/cloudindex/indicator/Stability> <http://www.w3.org/1999/02/22-rdf-syntax-ns#type> <http://purl.org/weso/cloudindex/ontology/KPIIndicator>.
<http://purl.org/weso/cloudindex/indicator/Stability> <http://www.w3.org/2000/01/rdf-schema#label> "Stability"@en.
<http://purl.org/weso/cloudindex/indicator/Stability> <http://www.w3.org/2000/01/rdf-schema#comment> "The degree to which the service is resistant to change, deterioration, or displacement."@en.
<http://purl.org/weso/cloudindex/indicator/Stability> <http://www.w3.org/2004/02/skos/core#definition> "The degree to which the service is resistant to change, deterioration, or displacement."@en.
<http://purl.org/weso/cloudindex/indicator/Stability> <http://purl.org/weso/cloudindex/ontology/defined-in> <http://csmic.org/wp-content/uploads/2011/09/SMI-Overview-110913_v1F.pdf>.
<http://purl.org/weso/cloudindex/indicator/Stability> <http://purl.org/weso/cloudindex/ontology/defined-by> <http://purl.org/weso/cloudindex/organization/CSMIC>.
<http://purl.org/weso/cloudindex/indicator/Stability> <http://purl.org/weso/cloudindex/ontology/weight> "1.0"^^<http://www.w3.org/2001/XMLSchema#double>.
<http://purl.org/weso/cloudindex/indicator/Stability> <http://purl.org/weso/cloudindex/ontology/pref-value> <http://purl.org/weso/cloudindex/ontology/High>.
<http://purl.org/weso/cloudindex/indicator/Stability> <http://www.w3.org/2004/02/skos/core#notation> "Stability".
<http://purl.org/weso/cloudindex/indicator/Stability> <http://www.w3.org/2006/time#intervalStarts> "2013"^^<http://www.w3.org/2001/XMLSchema#int>.
<http://purl.org/weso/cloudindex/indicator/Stability> <http://www.w3.org/2006/time#intervalFinishes> "2013"^^<http://www.w3.org/2001/XMLSchema#int>.
<http://purl.org/weso/cloudindex/indicator/Stability> <http://www.w3.org/2004/02/skos/core#broader> <http://purl.org/weso/cloudindex/component/Assurance>.
<http://purl.org/weso/cloudindex/indicator/Serviceability> <http://www.w3.org/1999/02/22-rdf-syntax-ns#type> <http://purl.org/weso/cloudindex/ontology/KPIIndicator>.
<http://purl.org/weso/cloudindex/indicator/Serviceability> <http://www.w3.org/2000/01/rdf-schema#label> "Serviceability"@en.
<http://purl.org/weso/cloudindex/indicator/Serviceability> <http://www.w3.org/2000/01/rdf-schema#comment> "The ease and efficiency of performing maintenance and correcting problems with the service."@en.
<http://purl.org/weso/cloudindex/indicator/Serviceability> <http://www.w3.org/2004/02/skos/core#definition> "The ease and efficiency of performing maintenance and correcting problems with the service."@en.
<http://purl.org/weso/cloudindex/indicator/Serviceability> <http://purl.org/weso/cloudindex/ontology/defined-in> <http://csmic.org/wp-content/uploads/2011/09/SMI-Overview-110913_v1F.pdf>.
<http://purl.org/weso/cloudindex/indicator/Serviceability> <http://purl.org/weso/cloudindex/ontology/defined-by> <http://purl.org/weso/cloudindex/organization/CSMIC>.
<http://purl.org/weso/cloudindex/indicator/Serviceability> <http://purl.org/weso/cloudindex/ontology/weight> "1.0"^^<http://www.w3.org/2001/XMLSchema#double>.
<http://purl.org/weso/cloudindex/indicator/Serviceability> <http://purl.org/weso/cloudindex/ontology/pref-value> <http://purl.org/weso/cloudindex/ontology/High>.
<http://purl.org/weso/cloudindex/indicator/Serviceability> <http://www.w3.org/2004/02/skos/core#notation> "Serviceability".
<http://purl.org/weso/cloudindex/indicator/Serviceability> <http://www.w3.org/2006/time#intervalStarts> "2013"^^<http://www.w3.org/2001/XMLSchema#int>.
<http://purl.org/weso/cloudindex/indicator/Serviceability> <http://www.w3.org/2006/time#intervalFinishes> "2013"^^<http://www.w3.org/2001/XMLSchema#int>.
<http://purl.org/weso/cloudindex/indicator/Serviceability> <http://www.w3.org/2004/02/skos/core#broader> <http://purl.org/weso/cloudindex/component/Assurance>.
<http://purl.org/weso/cloudindex/indicator/Acquisition> <http://www.w3.org/1999/02/22-rdf-syntax-ns#type> <http://purl.org/weso/cloudindex/ontology/KPIIndicator>.
<http://purl.org/weso/cloudindex/indicator/Acquisition> <http://www.w3.org/2000/01/rdf-schema#label> "Acquisition"@en.
<http://purl.org/weso/cloudindex/indicator/Acquisition> <http://www.w3.org/2000/01/rdf-schema#comment> "Any client costs to acquire the rights and ability to use a service and to move from an existing service to the new one."@en.
<http://purl.org/weso/cloudindex/indicator/Acquisition> <http://www.w3.org/2004/02/skos/core#definition> "Any client costs to acquire the rights and ability to use a service and to move\r\nfrom an existing service to the new one."@en.
<http://purl.org/weso/cloudindex/indicator/Acquisition> <http://purl.org/weso/cloudindex/ontology/defined-in> <http://csmic.org/wp-content/uploads/2011/09/SMI-Overview-110913_v1F.pdf>.
<http://purl.org/weso/cloudindex/indicator/Acquisition> <http://purl.org/weso/cloudindex/ontology/defined-by> <http://purl.org/weso/cloudindex/organization/CSMIC>.
<http://purl.org/weso/cloudindex/indicator/Acquisition> <http://purl.org/weso/cloudindex/ontology/weight> "1.0"^^<http://www.w3.org/2001/XMLSchema#double>.
<http://purl.org/weso/cloudindex/indicator/Acquisition> <http://purl.org/weso/cloudindex/ontology/pref-value> <http://purl.org/weso/cloudindex/ontology/High>.
<http://purl.org/weso/cloudindex/indicator/Acquisition> <http://www.w3.org/2004/02/skos/core#notation> "Acquisition".
<http://purl.org/weso/cloudindex/indicator/Acquisition> <http://www.w3.org/2006/time#intervalStarts> "2013"^^<http://www.w3.org/2001/XMLSchema#int>.
<http://purl.org/weso/cloudindex/indicator/Acquisition> <http://www.w3.org/2006/time#intervalFinishes> "2013"^^<http://www.w3.org/2001/XMLSchema#int>.
<http://purl.org/weso/cloudindex/indicator/Acquisition> <http://www.w3.org/2004/02/skos/core#broader> <http://purl.org/weso/cloudindex/component/Financial>.
<http://purl.org/weso/cloudindex/indicator/OngoingCost> <http://www.w3.org/1999/02/22-rdf-syntax-ns#type> <http://purl.org/weso/cloudindex/ontology/KPIIndicator>.
<http://purl.org/weso/cloudindex/indicator/OngoingCost> <http://www.w3.org/2000/01/rdf-schema#label> "On-going Cost"@en.
<http://purl.org/weso/cloudindex/indicator/OngoingCost> <http://www.w3.org/2000/01/rdf-schema#comment> "The client cost to operate a service. This includes both recurring flat costs (e.g.,\r\nmonthly access fees) and usage-based costs."@en.
<http://purl.org/weso/cloudindex/indicator/OngoingCost> <http://www.w3.org/2004/02/skos/core#definition> "The client cost to operate a service. This includes both recurring flat costs (e.g.,\r\nmonthly access fees) and usage-based costs."@en.
<http://purl.org/weso/cloudindex/indicator/OngoingCost> <http://purl.org/weso/cloudindex/ontology/defined-in> <http://csmic.org/wp-content/uploads/2011/09/SMI-Overview-110913_v1F.pdf>.
<http://purl.org/weso/cloudindex/indicator/OngoingCost> <http://purl.org/weso/cloudindex/ontology/defined-by> <http://purl.org/weso/cloudindex/organization/CSMIC>.
<http://purl.org/weso/cloudindex/indicator/OngoingCost> <http://purl.org/weso/cloudindex/ontology/weight> "1.0"^^<http://www.w3.org/2001/XMLSchema#double>.
<http://purl.org/weso/cloudindex/indicator/OngoingCost> <http://purl.org/weso/cloudindex/ontology/pref-value> <http://purl.org/weso/cloudindex/ontology/High>.
<http://purl.org/weso/cloudindex/indicator/OngoingCost> <http://www.w3.org/2004/02/skos/core#notation> "OngoingCost".
<http://purl.org/weso/cloudindex/indicator/OngoingCost> <http://www.w3.org/2006/time#intervalStarts> "2013"^^<http://www.w3.org/2001/XMLSchema#int>.
<http://purl.org/weso/cloudindex/indicator/OngoingCost> <http://www.w3.org/2006/time#intervalFinishes> "2013"^^<http://www.w3.org/2001/XMLSchema#int>.
<http://purl.org/weso/cloudindex/indicator/OngoingCost> <http://www.w3.org/2004/02/skos/core#broader> <http://purl.org/weso/cloudindex/component/Financial>.
<http://purl.org/weso/cloudindex/indicator/Profit> <http://www.w3.org/1999/02/22-rdf-syntax-ns#type> <http://purl.org/weso/cloudindex/ontology/KPIIndicator>.
<http://purl.org/weso/cloudindex/indicator/Profit> <http://www.w3.org/2000/01/rdf-schema#label> "Profit"@en.
<http://purl.org/weso/cloudindex/indicator/Profit> <http://www.w3.org/2000/01/rdf-schema#comment> "Arrangement between client and provider(s) under which costs or profits of a\r\nservice are shared by the involved parties, according to an agreed upon formula."@en.
<http://purl.org/weso/cloudindex/indicator/Profit> <http://www.w3.org/2004/02/skos/core#definition> "Arrangement between client and provider(s) under which costs or profits of a\r\nservice are shared by the involved parties, according to an agreed upon formula."@en.
<http://purl.org/weso/cloudindex/indicator/Profit> <http://purl.org/weso/cloudindex/ontology/defined-in> <http://csmic.org/wp-content/uploads/2011/09/SMI-Overview-110913_v1F.pdf>.
<http://purl.org/weso/cloudindex/indicator/Profit> <http://purl.org/weso/cloudindex/ontology/defined-by> <http://purl.org/weso/cloudindex/organization/CSMIC>.
<http://purl.org/weso/cloudindex/indicator/Profit> <http://purl.org/weso/cloudindex/ontology/weight> "1.0"^^<http://www.w3.org/2001/XMLSchema#double>.
<http://purl.org/weso/cloudindex/indicator/Profit> <http://purl.org/weso/cloudindex/ontology/pref-value> <http://purl.org/weso/cloudindex/ontology/High>.
<http://purl.org/weso/cloudindex/indicator/Profit> <http://www.w3.org/2004/02/skos/core#notation> "Profit".
<http://purl.org/weso/cloudindex/indicator/Profit> <http://www.w3.org/2006/time#intervalStarts> "2013"^^<http://www.w3.org/2001/XMLSchema#int>.
<http://purl.org/weso/cloudindex/indicator/Profit> <http://www.w3.org/2006/time#intervalFinishes> "2013"^^<http://www.w3.org/2001/XMLSchema#int>.
<http://purl.org/weso/cloudindex/indicator/Profit> <http://www.w3.org/2004/02/skos/core#broader> <http://purl.org/weso/cloudindex/component/Financial>.
<http://purl.org/weso/cloudindex/indicator/Accuracy> <http://www.w3.org/1999/02/22-rdf-syntax-ns#type> <http://purl.org/weso/cloudindex/ontology/KPIIndicator>.
<http://purl.org/weso/cloudindex/indicator/Accuracy> <http://www.w3.org/2000/01/rdf-schema#label> "Accuracy"@en.
<http://purl.org/weso/cloudindex/indicator/Accuracy> <http://www.w3.org/2000/01/rdf-schema#comment> "The extent to which a service adheres to its requirements."@en.
<http://purl.org/weso/cloudindex/indicator/Accuracy> <http://www.w3.org/2004/02/skos/core#definition> "The extent to which a service adheres to its requirements."@en.
<http://purl.org/weso/cloudindex/indicator/Accuracy> <http://purl.org/weso/cloudindex/ontology/defined-in> <http://csmic.org/wp-content/uploads/2011/09/SMI-Overview-110913_v1F.pdf>.
<http://purl.org/weso/cloudindex/indicator/Accuracy> <http://purl.org/weso/cloudindex/ontology/defined-by> <http://purl.org/weso/cloudindex/organization/CSMIC>.
<http://purl.org/weso/cloudindex/indicator/Accuracy> <http://purl.org/weso/cloudindex/ontology/weight> "1.0"^^<http://www.w3.org/2001/XMLSchema#double>.
<http://purl.org/weso/cloudindex/indicator/Accuracy> <http://purl.org/weso/cloudindex/ontology/pref-value> <http://purl.org/weso/cloudindex/ontology/High>.
<http://purl.org/weso/cloudindex/indicator/Accuracy> <http://www.w3.org/2004/02/skos/core#notation> "Accuracy".
<http://purl.org/weso/cloudindex/indicator/Accuracy> <http://www.w3.org/2006/time#intervalStarts> "2013"^^<http://www.w3.org/2001/XMLSchema#int>.
<http://purl.org/weso/cloudindex/indicator/Accuracy> <http://www.w3.org/2006/time#intervalFinishes> "2013"^^<http://www.w3.org/2001/XMLSchema#int>.
<http://purl.org/weso/cloudindex/indicator/Accuracy> <http://www.w3.org/2004/02/skos/core#broader> <http://purl.org/weso/cloudindex/component/Performance>.
<http://purl.org/weso/cloudindex/indicator/Functionality> <http://www.w3.org/1999/02/22-rdf-syntax-ns#type> <http://purl.org/weso/cloudindex/ontology/KPIIndicator>.
<http://purl.org/weso/cloudindex/indicator/Functionality> <http://www.w3.org/2000/01/rdf-schema#label> "Functionality"@en.
<http://purl.org/weso/cloudindex/indicator/Functionality> <http://www.w3.org/2000/01/rdf-schema#comment> "The specific features provided by a service."@en.
<http://purl.org/weso/cloudindex/indicator/Functionality> <http://www.w3.org/2004/02/skos/core#definition> "The specific features provided by a service."@en.
<http://purl.org/weso/cloudindex/indicator/Functionality> <http://purl.org/weso/cloudindex/ontology/defined-in> <http://csmic.org/wp-content/uploads/2011/09/SMI-Overview-110913_v1F.pdf>.
<http://purl.org/weso/cloudindex/indicator/Functionality> <http://purl.org/weso/cloudindex/ontology/defined-by> <http://purl.org/weso/cloudindex/organization/CSMIC>.
<http://purl.org/weso/cloudindex/indicator/Functionality> <http://purl.org/weso/cloudindex/ontology/weight> "1.0"^^<http://www.w3.org/2001/XMLSchema#double>.
<http://purl.org/weso/cloudindex/indicator/Functionality> <http://purl.org/weso/cloudindex/ontology/pref-value> <http://purl.org/weso/cloudindex/ontology/High>.
<http://purl.org/weso/cloudindex/indicator/Functionality> <http://www.w3.org/2004/02/skos/core#notation> "Functionality".
<http://purl.org/weso/cloudindex/indicator/Functionality> <http://www.w3.org/2006/time#intervalStarts> "2013"^^<http://www.w3.org/2001/XMLSchema#int>.
<http://purl.org/weso/cloudindex/indicator/Functionality> <http://www.w3.org/2006/time#intervalFinishes> "2013"^^<http://www.w3.org/2001/XMLSchema#int>.
<http://purl.org/weso/cloudindex/indicator/Functionality> <http://www.w3.org/2004/02/skos/core#broader> <http://purl.org/weso/cloudindex/component/Performance>.
<http://purl.org/weso/cloudindex/indicator/Suitability> <http://www.w3.org/1999/02/22-rdf-syntax-ns#type> <http://purl.org/weso/cloudindex/ontology/KPIIndicator>.
<http://purl.org/weso/cloudindex/indicator/Suitability> <http://www.w3.org/2000/01/rdf-schema#label> "Suitability"@en.
<http://purl.org/weso/cloudindex/indicator/Suitability> <http://www.w3.org/2000/01/rdf-schema#comment> "How closely do the capabilities of the service match the needs of the client."@en.
<http://purl.org/weso/cloudindex/indicator/Suitability> <http://www.w3.org/2004/02/skos/core#definition> "How closely do the capabilities of the service match the needs of the client."@en.
<http://purl.org/weso/cloudindex/indicator/Suitability> <http://purl.org/weso/cloudindex/ontology/defined-in> <http://csmic.org/wp-content/uploads/2011/09/SMI-Overview-110913_v1F.pdf>.
<http://purl.org/weso/cloudindex/indicator/Suitability> <http://purl.org/weso/cloudindex/ontology/defined-by> <http://purl.org/weso/cloudindex/organization/CSMIC>.
<http://purl.org/weso/cloudindex/indicator/Suitability> <http://purl.org/weso/cloudindex/ontology/weight> "1.0"^^<http://www.w3.org/2001/XMLSchema#double>.
<http://purl.org/weso/cloudindex/indicator/Suitability> <http://purl.org/weso/cloudindex/ontology/pref-value> <http://purl.org/weso/cloudindex/ontology/High>.
<http://purl.org/weso/cloudindex/indicator/Suitability> <http://www.w3.org/2004/02/skos/core#notation> "Suitability".
<http://purl.org/weso/cloudindex/indicator/Suitability> <http://www.w3.org/2006/time#intervalStarts> "2013"^^<http://www.w3.org/2001/XMLSchema#int>.
<http://purl.org/weso/cloudindex/indicator/Suitability> <http://www.w3.org/2006/time#intervalFinishes> "2013"^^<http://www.w3.org/2001/XMLSchema#int>.
<http://purl.org/weso/cloudindex/indicator/Suitability> <http://www.w3.org/2004/02/skos/core#broader> <http://purl.org/weso/cloudindex/component/Performance>.
<http://purl.org/weso/cloudindex/indicator/Interoperability> <http://www.w3.org/1999/02/22-rdf-syntax-ns#type> <http://purl.org/weso/cloudindex/ontology/KPIIndicator>.
<http://purl.org/weso/cloudindex/indicator/Interoperability> <http://www.w3.org/2000/01/rdf-schema#label> "Suitability"@en.
<http://purl.org/weso/cloudindex/indicator/Interoperability> <http://www.w3.org/2000/01/rdf-schema#comment> "The ability of a service to easily interact with other services (from the same service provider and from other service providers)."@en.
<http://purl.org/weso/cloudindex/indicator/Interoperability> <http://www.w3.org/2004/02/skos/core#definition> "The ability of a service to easily interact with other services (from the same service provider and from other service providers)."@en.
<http://purl.org/weso/cloudindex/indicator/Interoperability> <http://purl.org/weso/cloudindex/ontology/defined-in> <http://csmic.org/wp-content/uploads/2011/09/SMI-Overview-110913_v1F.pdf>.
<http://purl.org/weso/cloudindex/indicator/Interoperability> <http://purl.org/weso/cloudindex/ontology/defined-by> <http://purl.org/weso/cloudindex/organization/CSMIC>.
<http://purl.org/weso/cloudindex/indicator/Interoperability> <http://purl.org/weso/cloudindex/ontology/weight> "1.0"^^<http://www.w3.org/2001/XMLSchema#double>.
<http://purl.org/weso/cloudindex/indicator/Interoperability> <http://purl.org/weso/cloudindex/ontology/pref-value> <http://purl.org/weso/cloudindex/ontology/High>.
<http://purl.org/weso/cloudindex/indicator/Interoperability> <http://www.w3.org/2004/02/skos/core#notation> "Interoperability".
<http://purl.org/weso/cloudindex/indicator/Interoperability> <http://www.w3.org/2006/time#intervalStarts> "2013"^^<http://www.w3.org/2001/XMLSchema#int>.
<http://purl.org/weso/cloudindex/indicator/Interoperability> <http://www.w3.org/2006/time#intervalFinishes> "2013"^^<http://www.w3.org/2001/XMLSchema#int>.
<http://purl.org/weso/cloudindex/indicator/Interoperability> <http://www.w3.org/2004/02/skos/core#broader> <http://purl.org/weso/cloudindex/component/Performance>.
<http://purl.org/weso/cloudindex/indicator/ServiceResponseTime> <http://www.w3.org/1999/02/22-rdf-syntax-ns#type> <http://purl.org/weso/cloudindex/ontology/KPIIndicator>.
<http://purl.org/weso/cloudindex/indicator/ServiceResponseTime> <http://www.w3.org/2000/01/rdf-schema#label> "Service Response Time"@en.
<http://purl.org/weso/cloudindex/indicator/ServiceResponseTime> <http://www.w3.org/2000/01/rdf-schema#comment> "An indicator of the time between when a service is requested and when the response is available."@en.
<http://purl.org/weso/cloudindex/indicator/ServiceResponseTime> <http://www.w3.org/2004/02/skos/core#definition> "An indicator of the time between when a service is requested and when the response is available."@en.
<http://purl.org/weso/cloudindex/indicator/ServiceResponseTime> <http://purl.org/weso/cloudindex/ontology/defined-in> <http://csmic.org/wp-content/uploads/2011/09/SMI-Overview-110913_v1F.pdf>.
<http://purl.org/weso/cloudindex/indicator/ServiceResponseTime> <http://purl.org/weso/cloudindex/ontology/defined-by> <http://purl.org/weso/cloudindex/organization/CSMIC>.
<http://purl.org/weso/cloudindex/indicator/ServiceResponseTime> <http://purl.org/weso/cloudindex/ontology/weight> "1.0"^^<http://www.w3.org/2001/XMLSchema#double>.
<http://purl.org/weso/cloudindex/indicator/ServiceResponseTime> <http://purl.org/weso/cloudindex/ontology/pref-value> <http://purl.org/weso/cloudindex/ontology/High>.
<http://purl.org/weso/cloudindex/indicator/ServiceResponseTime> <http://www.w3.org/2004/02/skos/core#notation> "ServiceResponseTime".
<http://purl.org/weso/cloudindex/indicator/ServiceResponseTime> <http://www.w3.org/2006/time#intervalStarts> "2013"^^<http://www.w3.org/2001/XMLSchema#int>.
<http://purl.org/weso/cloudindex/indicator/ServiceResponseTime> <http://www.w3.org/2006/time#intervalFinishes> "2013"^^<http://www.w3.org/2001/XMLSchema#int>.
<http://purl.org/weso/cloudindex/indicator/ServiceResponseTime> <http://www.w3.org/2004/02/skos/core#broader> <http://purl.org/weso/cloudindex/component/Performance>.
<http://purl.org/weso/cloudindex/indicator/AccessControl> <http://www.w3.org/1999/02/22-rdf-syntax-ns#type> <http://purl.org/weso/cloudindex/ontology/KPIIndicator>.
<http://purl.org/weso/cloudindex/indicator/AccessControl> <http://www.w3.org/2000/01/rdf-schema#label> "Access Control"@en.
<http://purl.org/weso/cloudindex/indicator/AccessControl> <http://www.w3.org/2000/01/rdf-schema#comment> "Policies and processes in use by the service provider to ensure that only the provider and client personnel with appropriate status/reasons to make use of or modify data/work products may do so."@en.
<http://purl.org/weso/cloudindex/indicator/AccessControl> <http://www.w3.org/2004/02/skos/core#definition> "Policies and processes in use by the service provider to ensure that only the provider and client personnel with appropriate status/reasons to make use of or modify data/work products may do so."@en.
<http://purl.org/weso/cloudindex/indicator/AccessControl> <http://purl.org/weso/cloudindex/ontology/defined-in> <http://csmic.org/wp-content/uploads/2011/09/SMI-Overview-110913_v1F.pdf>.
<http://purl.org/weso/cloudindex/indicator/AccessControl> <http://purl.org/weso/cloudindex/ontology/defined-by> <http://purl.org/weso/cloudindex/organization/CSMIC>.
<http://purl.org/weso/cloudindex/indicator/AccessControl> <http://purl.org/weso/cloudindex/ontology/weight> "1.0"^^<http://www.w3.org/2001/XMLSchema#double>.
<http://purl.org/weso/cloudindex/indicator/AccessControl> <http://purl.org/weso/cloudindex/ontology/pref-value> <http://purl.org/weso/cloudindex/ontology/High>.
<http://purl.org/weso/cloudindex/indicator/AccessControl> <http://www.w3.org/2004/02/skos/core#notation> "AccessControl".
<http://purl.org/weso/cloudindex/indicator/AccessControl> <http://www.w3.org/2006/time#intervalStarts> "2013"^^<http://www.w3.org/2001/XMLSchema#int>.
<http://purl.org/weso/cloudindex/indicator/AccessControl> <http://www.w3.org/2006/time#intervalFinishes> "2013"^^<http://www.w3.org/2001/XMLSchema#int>.
<http://purl.org/weso/cloudindex/indicator/AccessControl> <http://www.w3.org/2004/02/skos/core#broader> <http://purl.org/weso/cloudindex/component/SecurityPrivacy>.
<http://purl.org/weso/cloudindex/indicator/GeographicalConstraint> <http://www.w3.org/1999/02/22-rdf-syntax-ns#type> <http://purl.org/weso/cloudindex/ontology/KPIIndicator>.
<http://purl.org/weso/cloudindex/indicator/GeographicalConstraint> <http://www.w3.org/2000/01/rdf-schema#label> "Geographical Constraint"@en.
<http://purl.org/weso/cloudindex/indicator/GeographicalConstraint> <http://www.w3.org/2000/01/rdf-schema#comment> "The client's constraints on service location based on geography."@en.
<http://purl.org/weso/cloudindex/indicator/GeographicalConstraint> <http://www.w3.org/2004/02/skos/core#definition> "The client's constraints on service location based on geography."@en.
<http://purl.org/weso/cloudindex/indicator/GeographicalConstraint> <http://purl.org/weso/cloudindex/ontology/defined-in> <http://csmic.org/wp-content/uploads/2011/09/SMI-Overview-110913_v1F.pdf>.
<http://purl.org/weso/cloudindex/indicator/GeographicalConstraint> <http://purl.org/weso/cloudindex/ontology/defined-by> <http://purl.org/weso/cloudindex/organization/CSMIC>.
<http://purl.org/weso/cloudindex/indicator/GeographicalConstraint> <http://purl.org/weso/cloudindex/ontology/weight> "1.0"^^<http://www.w3.org/2001/XMLSchema#double>.
<http://purl.org/weso/cloudindex/indicator/GeographicalConstraint> <http://purl.org/weso/cloudindex/ontology/pref-value> <http://purl.org/weso/cloudindex/ontology/High>.
<http://purl.org/weso/cloudindex/indicator/GeographicalConstraint> <http://www.w3.org/2004/02/skos/core#notation> "GeographicalConstraint".
<http://purl.org/weso/cloudindex/indicator/GeographicalConstraint> <http://www.w3.org/2006/time#intervalStarts> "2013"^^<http://www.w3.org/2001/XMLSchema#int>.
<http://purl.org/weso/cloudindex/indicator/GeographicalConstraint> <http://www.w3.org/2006/time#intervalFinishes> "2013"^^<http://www.w3.org/2001/XMLSchema#int>.
<http://purl.org/weso/cloudindex/indicator/GeographicalConstraint> <http://www.w3.org/2004/02/skos/core#broader> <http://purl.org/weso/cloudindex/component/SecurityPrivacy>.
<http://purl.org/weso/cloudindex/indicator/PoliticalConstraint> <http://www.w3.org/1999/02/22-rdf-syntax-ns#type> <http://purl.org/weso/cloudindex/ontology/KPIIndicator>.
<http://purl.org/weso/cloudindex/indicator/PoliticalConstraint> <http://www.w3.org/2000/01/rdf-schema#label> "Political Constraint"@en.
<http://purl.org/weso/cloudindex/indicator/PoliticalConstraint> <http://www.w3.org/2000/01/rdf-schema#comment> "The client's constraints on service location based on politics."@en.
<http://purl.org/weso/cloudindex/indicator/PoliticalConstraint> <http://www.w3.org/2004/02/skos/core#definition> "The client's constraints on service location based on geography."@en.
<http://purl.org/weso/cloudindex/indicator/PoliticalConstraint> <http://purl.org/weso/cloudindex/ontology/defined-in> <http://csmic.org/wp-content/uploads/2011/09/SMI-Overview-110913_v1F.pdf>.
<http://purl.org/weso/cloudindex/indicator/PoliticalConstraint> <http://purl.org/weso/cloudindex/ontology/defined-by> <http://purl.org/weso/cloudindex/organization/CSMIC>.
<http://purl.org/weso/cloudindex/indicator/PoliticalConstraint> <http://purl.org/weso/cloudindex/ontology/weight> "1.0"^^<http://www.w3.org/2001/XMLSchema#double>.
<http://purl.org/weso/cloudindex/indicator/PoliticalConstraint> <http://purl.org/weso/cloudindex/ontology/pref-value> <http://purl.org/weso/cloudindex/ontology/High>.
<http://purl.org/weso/cloudindex/indicator/PoliticalConstraint> <http://www.w3.org/2004/02/skos/core#notation> "PoliticalConstraint".
<http://purl.org/weso/cloudindex/indicator/PoliticalConstraint> <http://www.w3.org/2006/time#intervalStarts> "2013"^^<http://www.w3.org/2001/XMLSchema#int>.
<http://purl.org/weso/cloudindex/indicator/PoliticalConstraint> <http://www.w3.org/2006/time#intervalFinishes> "2013"^^<http://www.w3.org/2001/XMLSchema#int>.
<http://purl.org/weso/cloudindex/indicator/PoliticalConstraint> <http://www.w3.org/2004/02/skos/core#broader> <http://purl.org/weso/cloudindex/component/SecurityPrivacy>.
<http://purl.org/weso/cloudindex/indicator/DataIntegrity> <http://www.w3.org/1999/02/22-rdf-syntax-ns#type> <http://purl.org/weso/cloudindex/ontology/KPIIndicator>.
<http://purl.org/weso/cloudindex/indicator/DataIntegrity> <http://www.w3.org/2000/01/rdf-schema#label> "Data Integrity"@en.
<http://purl.org/weso/cloudindex/indicator/DataIntegrity> <http://www.w3.org/2000/01/rdf-schema#comment> "Keeping the data that is created, used, and stored in its correct form so that clients may be confident that it is accurate and valid."@en.
<http://purl.org/weso/cloudindex/indicator/DataIntegrity> <http://www.w3.org/2004/02/skos/core#definition> "Keeping the data that is created, used, and stored in its correct form so that clients may be confident that it is accurate and valid."@en.
<http://purl.org/weso/cloudindex/indicator/DataIntegrity> <http://purl.org/weso/cloudindex/ontology/defined-in> <http://csmic.org/wp-content/uploads/2011/09/SMI-Overview-110913_v1F.pdf>.
<http://purl.org/weso/cloudindex/indicator/DataIntegrity> <http://purl.org/weso/cloudindex/ontology/defined-by> <http://purl.org/weso/cloudindex/organization/CSMIC>.
<http://purl.org/weso/cloudindex/indicator/DataIntegrity> <http://purl.org/weso/cloudindex/ontology/weight> "1.0"^^<http://www.w3.org/2001/XMLSchema#double>.
<http://purl.org/weso/cloudindex/indicator/DataIntegrity> <http://purl.org/weso/cloudindex/ontology/pref-value> <http://purl.org/weso/cloudindex/ontology/High>.
<http://purl.org/weso/cloudindex/indicator/DataIntegrity> <http://www.w3.org/2004/02/skos/core#notation> "DataIntegrity".
<http://purl.org/weso/cloudindex/indicator/DataIntegrity> <http://www.w3.org/2006/time#intervalStarts> "2013"^^<http://www.w3.org/2001/XMLSchema#int>.
<http://purl.org/weso/cloudindex/indicator/DataIntegrity> <http://www.w3.org/2006/time#intervalFinishes> "2013"^^<http://www.w3.org/2001/XMLSchema#int>.
<http://purl.org/weso/cloudindex/indicator/DataIntegrity> <http://www.w3.org/2004/02/skos/core#broader> <http://purl.org/weso/cloudindex/component/SecurityPrivacy>.
<http://purl.org/weso/cloudindex/indicator/DataPrivacy> <http://www.w3.org/1999/02/22-rdf-syntax-ns#type> <http://purl.org/weso/cloudindex/ontology/KPIIndicator>.
<http://purl.org/weso/cloudindex/indicator/DataPrivacy> <http://www.w3.org/2000/01/rdf-schema#label> "Data Privacy"@en.
<http://purl.org/weso/cloudindex/indicator/DataPrivacy> <http://www.w3.org/2000/01/rdf-schema#comment> "Client restrictions on access and use of client data are enforced by the service provider. Any failures of these protections are promptly detected and reported to the client."@en.
<http://purl.org/weso/cloudindex/indicator/DataPrivacy> <http://www.w3.org/2004/02/skos/core#definition> "Client restrictions on access and use of client data are enforced by the service provider. Any failures of these protections are promptly detected and reported to the client."@en.
<http://purl.org/weso/cloudindex/indicator/DataPrivacy> <http://purl.org/weso/cloudindex/ontology/defined-in> <http://csmic.org/wp-content/uploads/2011/09/SMI-Overview-110913_v1F.pdf>.
<http://purl.org/weso/cloudindex/indicator/DataPrivacy> <http://purl.org/weso/cloudindex/ontology/defined-by> <http://purl.org/weso/cloudindex/organization/CSMIC>.
<http://purl.org/weso/cloudindex/indicator/DataPrivacy> <http://purl.org/weso/cloudindex/ontology/weight> "1.0"^^<http://www.w3.org/2001/XMLSchema#double>.
<http://purl.org/weso/cloudindex/indicator/DataPrivacy> <http://purl.org/weso/cloudindex/ontology/pref-value> <http://purl.org/weso/cloudindex/ontology/High>.
<http://purl.org/weso/cloudindex/indicator/DataPrivacy> <http://www.w3.org/2004/02/skos/core#notation> "DataPrivacy".
<http://purl.org/weso/cloudindex/indicator/DataPrivacy> <http://www.w3.org/2006/time#intervalStarts> "2013"^^<http://www.w3.org/2001/XMLSchema#int>.
<http://purl.org/weso/cloudindex/indicator/DataPrivacy> <http://www.w3.org/2006/time#intervalFinishes> "2013"^^<http://www.w3.org/2001/XMLSchema#int>.
<http://purl.org/weso/cloudindex/indicator/DataPrivacy> <http://www.w3.org/2004/02/skos/core#broader> <http://purl.org/weso/cloudindex/component/SecurityPrivacy>.
<http://purl.org/weso/cloudindex/indicator/DataLoss> <http://www.w3.org/1999/02/22-rdf-syntax-ns#type> <http://purl.org/weso/cloudindex/ontology/KPIIndicator>.
<http://purl.org/weso/cloudindex/indicator/DataLoss> <http://www.w3.org/2000/01/rdf-schema#label> "Data Loss"@en.
<http://purl.org/weso/cloudindex/indicator/DataLoss> <http://www.w3.org/2000/01/rdf-schema#comment> "Client restrictions on access and use of client data are enforced by the service provider. Any failures of these protections are promptly detected and reported to the client."@en.
<http://purl.org/weso/cloudindex/indicator/DataLoss> <http://www.w3.org/2004/02/skos/core#definition> "Client restrictions on access and use of client data are enforced by the service provider. Any failures of these protections are promptly detected and reported to the client."@en.
<http://purl.org/weso/cloudindex/indicator/DataLoss> <http://purl.org/weso/cloudindex/ontology/defined-in> <http://csmic.org/wp-content/uploads/2011/09/SMI-Overview-110913_v1F.pdf>.
<http://purl.org/weso/cloudindex/indicator/DataLoss> <http://purl.org/weso/cloudindex/ontology/defined-by> <http://purl.org/weso/cloudindex/organization/CSMIC>.
<http://purl.org/weso/cloudindex/indicator/DataLoss> <http://purl.org/weso/cloudindex/ontology/weight> "1.0"^^<http://www.w3.org/2001/XMLSchema#double>.
<http://purl.org/weso/cloudindex/indicator/DataLoss> <http://purl.org/weso/cloudindex/ontology/pref-value> <http://purl.org/weso/cloudindex/ontology/High>.
<http://purl.org/weso/cloudindex/indicator/DataLoss> <http://www.w3.org/2004/02/skos/core#notation> "DataLoss".
<http://purl.org/weso/cloudindex/indicator/DataLoss> <http://www.w3.org/2006/time#intervalStarts> "2013"^^<http://www.w3.org/2001/XMLSchema#int>.
<http://purl.org/weso/cloudindex/indicator/DataLoss> <http://www.w3.org/2006/time#intervalFinishes> "2013"^^<http://www.w3.org/2001/XMLSchema#int>.
<http://purl.org/weso/cloudindex/indicator/DataLoss> <http://www.w3.org/2004/02/skos/core#broader> <http://purl.org/weso/cloudindex/component/SecurityPrivacy>.
<http://purl.org/weso/cloudindex/indicator/EnvironmentSecurity> <http://www.w3.org/1999/02/22-rdf-syntax-ns#type> <http://purl.org/weso/cloudindex/ontology/KPIIndicator>.
<http://purl.org/weso/cloudindex/indicator/EnvironmentSecurity> <http://www.w3.org/2000/01/rdf-schema#label> "Physical & Environmental Security"@en.
<http://purl.org/weso/cloudindex/indicator/EnvironmentSecurity> <http://www.w3.org/2000/01/rdf-schema#comment> "Policies and processes in use by the service provider to protect the provider\r\nfacilities from unauthorized access, damage or interference."@en.
<http://purl.org/weso/cloudindex/indicator/EnvironmentSecurity> <http://www.w3.org/2004/02/skos/core#definition> "Policies and processes in use by the service provider to protect the provider\r\nfacilities from unauthorized access, damage or interference."@en.
<http://purl.org/weso/cloudindex/indicator/EnvironmentSecurity> <http://purl.org/weso/cloudindex/ontology/defined-in> <http://csmic.org/wp-content/uploads/2011/09/SMI-Overview-110913_v1F.pdf>.
<http://purl.org/weso/cloudindex/indicator/EnvironmentSecurity> <http://purl.org/weso/cloudindex/ontology/defined-by> <http://purl.org/weso/cloudindex/organization/CSMIC>.
<http://purl.org/weso/cloudindex/indicator/EnvironmentSecurity> <http://purl.org/weso/cloudindex/ontology/weight> "1.0"^^<http://www.w3.org/2001/XMLSchema#double>.
<http://purl.org/weso/cloudindex/indicator/EnvironmentSecurity> <http://purl.org/weso/cloudindex/ontology/pref-value> <http://purl.org/weso/cloudindex/ontology/High>.
<http://purl.org/weso/cloudindex/indicator/EnvironmentSecurity> <http://www.w3.org/2004/02/skos/core#notation> "EnvironmentSecurity".
<http://purl.org/weso/cloudindex/indicator/EnvironmentSecurity> <http://www.w3.org/2006/time#intervalStarts> "2013"^^<http://www.w3.org/2001/XMLSchema#int>.
<http://purl.org/weso/cloudindex/indicator/EnvironmentSecurity> <http://www.w3.org/2006/time#intervalFinishes> "2013"^^<http://www.w3.org/2001/XMLSchema#int>.
<http://purl.org/weso/cloudindex/indicator/EnvironmentSecurity> <http://www.w3.org/2004/02/skos/core#broader> <http://purl.org/weso/cloudindex/component/SecurityPrivacy>.
<http://purl.org/weso/cloudindex/indicator/ProactiveThreat> <http://www.w3.org/1999/02/22-rdf-syntax-ns#type> <http://purl.org/weso/cloudindex/ontology/KPIIndicator>.
<http://purl.org/weso/cloudindex/indicator/ProactiveThreat> <http://www.w3.org/2000/01/rdf-schema#label> "Proactive Threat &  Vulnerability Management"@en.
<http://purl.org/weso/cloudindex/indicator/ProactiveThreat> <http://www.w3.org/2000/01/rdf-schema#comment> "Mechanisms in place to ensure that the service is protected against know\r\nrecurring threats as well as new evolving vulnerabilities."@en.
<http://purl.org/weso/cloudindex/indicator/ProactiveThreat> <http://www.w3.org/2004/02/skos/core#definition> "Mechanisms in place to ensure that the service is protected against know\r\nrecurring threats as well as new evolving vulnerabilities."@en.
<http://purl.org/weso/cloudindex/indicator/ProactiveThreat> <http://purl.org/weso/cloudindex/ontology/defined-in> <http://csmic.org/wp-content/uploads/2011/09/SMI-Overview-110913_v1F.pdf>.
<http://purl.org/weso/cloudindex/indicator/ProactiveThreat> <http://purl.org/weso/cloudindex/ontology/defined-by> <http://purl.org/weso/cloudindex/organization/CSMIC>.
<http://purl.org/weso/cloudindex/indicator/ProactiveThreat> <http://purl.org/weso/cloudindex/ontology/weight> "1.0"^^<http://www.w3.org/2001/XMLSchema#double>.
<http://purl.org/weso/cloudindex/indicator/ProactiveThreat> <http://purl.org/weso/cloudindex/ontology/pref-value> <http://purl.org/weso/cloudindex/ontology/High>.
<http://purl.org/weso/cloudindex/indicator/ProactiveThreat> <http://www.w3.org/2004/02/skos/core#notation> "ProactiveThreat".
<http://purl.org/weso/cloudindex/indicator/ProactiveThreat> <http://www.w3.org/2006/time#intervalStarts> "2013"^^<http://www.w3.org/2001/XMLSchema#int>.
<http://purl.org/weso/cloudindex/indicator/ProactiveThreat> <http://www.w3.org/2006/time#intervalFinishes> "2013"^^<http://www.w3.org/2001/XMLSchema#int>.
<http://purl.org/weso/cloudindex/indicator/ProactiveThreat> <http://www.w3.org/2004/02/skos/core#broader> <http://purl.org/weso/cloudindex/component/SecurityPrivacy>.
<http://purl.org/weso/cloudindex/indicator/Retention> <http://www.w3.org/1999/02/22-rdf-syntax-ns#type> <http://purl.org/weso/cloudindex/ontology/KPIIndicator>.
<http://purl.org/weso/cloudindex/indicator/Retention> <http://www.w3.org/2000/01/rdf-schema#label> "Retention/Disposition"@en.
<http://purl.org/weso/cloudindex/indicator/Retention> <http://www.w3.org/2000/01/rdf-schema#comment> "The service provider\u2019s data retention and disposition processes meet the clients'\r\n requirements."@en.
<http://purl.org/weso/cloudindex/indicator/Retention> <http://www.w3.org/2004/02/skos/core#definition> "The service provider\u2019s data retention and disposition processes meet the clients'\r\n requirements."@en.
<http://purl.org/weso/cloudindex/indicator/Retention> <http://purl.org/weso/cloudindex/ontology/defined-in> <http://csmic.org/wp-content/uploads/2011/09/SMI-Overview-110913_v1F.pdf>.
<http://purl.org/weso/cloudindex/indicator/Retention> <http://purl.org/weso/cloudindex/ontology/defined-by> <http://purl.org/weso/cloudindex/organization/CSMIC>.
<http://purl.org/weso/cloudindex/indicator/Retention> <http://purl.org/weso/cloudindex/ontology/weight> "1.0"^^<http://www.w3.org/2001/XMLSchema#double>.
<http://purl.org/weso/cloudindex/indicator/Retention> <http://purl.org/weso/cloudindex/ontology/pref-value> <http://purl.org/weso/cloudindex/ontology/High>.
<http://purl.org/weso/cloudindex/indicator/Retention> <http://www.w3.org/2004/02/skos/core#notation> "Retention".
<http://purl.org/weso/cloudindex/indicator/Retention> <http://www.w3.org/2006/time#intervalStarts> "2013"^^<http://www.w3.org/2001/XMLSchema#int>.
<http://purl.org/weso/cloudindex/indicator/Retention> <http://www.w3.org/2006/time#intervalFinishes> "2013"^^<http://www.w3.org/2001/XMLSchema#int>.
<http://purl.org/weso/cloudindex/indicator/Retention> <http://www.w3.org/2004/02/skos/core#broader> <http://purl.org/weso/cloudindex/component/SecurityPrivacy>.
<http://purl.org/weso/cloudindex/indicator/Disposition> <http://www.w3.org/1999/02/22-rdf-syntax-ns#type> <http://purl.org/weso/cloudindex/ontology/KPIIndicator>.
<http://purl.org/weso/cloudindex/indicator/Disposition> <http://www.w3.org/2000/01/rdf-schema#label> "Retention/Disposition"@en.
<http://purl.org/weso/cloudindex/indicator/Disposition> <http://www.w3.org/2000/01/rdf-schema#comment> "The service provider\u2019s data retention and disposition processes meet the clients'\r\n requirements."@en.
<http://purl.org/weso/cloudindex/indicator/Disposition> <http://www.w3.org/2004/02/skos/core#definition> "The service provider\u2019s data retention and disposition processes meet the clients'\r\n requirements."@en.
<http://purl.org/weso/cloudindex/indicator/Disposition> <http://purl.org/weso/cloudindex/ontology/defined-in> <http://csmic.org/wp-content/uploads/2011/09/SMI-Overview-110913_v1F.pdf>.
<http://purl.org/weso/cloudindex/indicator/Disposition> <http://purl.org/weso/cloudindex/ontology/defined-by> <http://purl.org/weso/cloudindex/organization/CSMIC>.
<http://purl.org/weso/cloudindex/indicator/Disposition> <http://purl.org/weso/cloudindex/ontology/weight> "1.0"^^<http://www.w3.org/2001/XMLSchema#double>.
<http://purl.org/weso/cloudindex/indicator/Disposition> <http://purl.org/weso/cloudindex/ontology/pref-value> <http://purl.org/weso/cloudindex/ontology/High>.
<http://purl.org/weso/cloudindex/indicator/Disposition> <http://www.w3.org/2004/02/skos/core#notation> "Disposition".
<http://purl.org/weso/cloudindex/indicator/Disposition> <http://www.w3.org/2006/time#intervalStarts> "2013"^^<http://www.w3.org/2001/XMLSchema#int>.
<http://purl.org/weso/cloudindex/indicator/Disposition> <http://www.w3.org/2006/time#intervalFinishes> "2013"^^<http://www.w3.org/2001/XMLSchema#int>.
<http://purl.org/weso/cloudindex/indicator/Disposition> <http://www.w3.org/2004/02/skos/core#broader> <http://purl.org/weso/cloudindex/component/SecurityPrivacy>.
<http://purl.org/weso/cloudindex/indicator/Accessibility> <http://www.w3.org/1999/02/22-rdf-syntax-ns#type> <http://purl.org/weso/cloudindex/ontology/KPIIndicator>.
<http://purl.org/weso/cloudindex/indicator/Accessibility> <http://www.w3.org/2000/01/rdf-schema#label> "Accessibility"@en.
<http://purl.org/weso/cloudindex/indicator/Accessibility> <http://www.w3.org/2000/01/rdf-schema#comment> "The degree to which a service is operable by users with disabilities."@en.
<http://purl.org/weso/cloudindex/indicator/Accessibility> <http://www.w3.org/2004/02/skos/core#definition> "The degree to which a service is operable by users with disabilities."@en.
<http://purl.org/weso/cloudindex/indicator/Accessibility> <http://purl.org/weso/cloudindex/ontology/defined-in> <http://csmic.org/wp-content/uploads/2011/09/SMI-Overview-110913_v1F.pdf>.
<http://purl.org/weso/cloudindex/indicator/Accessibility> <http://purl.org/weso/cloudindex/ontology/defined-by> <http://purl.org/weso/cloudindex/organization/CSMIC>.
<http://purl.org/weso/cloudindex/indicator/Accessibility> <http://purl.org/weso/cloudindex/ontology/weight> "1.0"^^<http://www.w3.org/2001/XMLSchema#double>.
<http://purl.org/weso/cloudindex/indicator/Accessibility> <http://purl.org/weso/cloudindex/ontology/pref-value> <http://purl.org/weso/cloudindex/ontology/High>.
<http://purl.org/weso/cloudindex/indicator/Accessibility> <http://www.w3.org/2004/02/skos/core#notation> "Accessibility".
<http://purl.org/weso/cloudindex/indicator/Accessibility> <http://www.w3.org/2006/time#intervalStarts> "2013"^^<http://www.w3.org/2001/XMLSchema#int>.
<http://purl.org/weso/cloudindex/indicator/Accessibility> <http://www.w3.org/2006/time#intervalFinishes> "2013"^^<http://www.w3.org/2001/XMLSchema#int>.
<http://purl.org/weso/cloudindex/indicator/Accessibility> <http://www.w3.org/2004/02/skos/core#broader> <http://purl.org/weso/cloudindex/component/Usability>.
<http://purl.org/weso/cloudindex/indicator/ClientPersonnelRequirements> <http://www.w3.org/1999/02/22-rdf-syntax-ns#type> <http://purl.org/weso/cloudindex/ontology/KPIIndicator>.
<http://purl.org/weso/cloudindex/indicator/ClientPersonnelRequirements> <http://www.w3.org/2000/01/rdf-schema#label> "Client Personnel Requirements"@en.
<http://purl.org/weso/cloudindex/indicator/ClientPersonnelRequirements> <http://www.w3.org/2000/01/rdf-schema#comment> "The minimum number of personnel satisfying roles, skills, experience, education,\r\nand certification required of the client to effectively utilize a service."@en.
<http://purl.org/weso/cloudindex/indicator/ClientPersonnelRequirements> <http://www.w3.org/2004/02/skos/core#definition> "The minimum number of personnel satisfying roles, skills, experience, education,\r\nand certification required of the client to effectively utilize a service."@en.
<http://purl.org/weso/cloudindex/indicator/ClientPersonnelRequirements> <http://purl.org/weso/cloudindex/ontology/defined-in> <http://csmic.org/wp-content/uploads/2011/09/SMI-Overview-110913_v1F.pdf>.
<http://purl.org/weso/cloudindex/indicator/ClientPersonnelRequirements> <http://purl.org/weso/cloudindex/ontology/defined-by> <http://purl.org/weso/cloudindex/organization/CSMIC>.
<http://purl.org/weso/cloudindex/indicator/ClientPersonnelRequirements> <http://purl.org/weso/cloudindex/ontology/weight> "1.0"^^<http://www.w3.org/2001/XMLSchema#double>.
<http://purl.org/weso/cloudindex/indicator/ClientPersonnelRequirements> <http://purl.org/weso/cloudindex/ontology/pref-value> <http://purl.org/weso/cloudindex/ontology/High>.
<http://purl.org/weso/cloudindex/indicator/ClientPersonnelRequirements> <http://www.w3.org/2004/02/skos/core#notation> "ClientPersonnelRequirements".
<http://purl.org/weso/cloudindex/indicator/ClientPersonnelRequirements> <http://www.w3.org/2006/time#intervalStarts> "2013"^^<http://www.w3.org/2001/XMLSchema#int>.
<http://purl.org/weso/cloudindex/indicator/ClientPersonnelRequirements> <http://www.w3.org/2006/time#intervalFinishes> "2013"^^<http://www.w3.org/2001/XMLSchema#int>.
<http://purl.org/weso/cloudindex/indicator/ClientPersonnelRequirements> <http://www.w3.org/2004/02/skos/core#broader> <http://purl.org/weso/cloudindex/component/Usability>.
<http://purl.org/weso/cloudindex/indicator/Installability> <http://www.w3.org/1999/02/22-rdf-syntax-ns#type> <http://purl.org/weso/cloudindex/ontology/KPIIndicator>.
<http://purl.org/weso/cloudindex/indicator/Installability> <http://www.w3.org/2000/01/rdf-schema#label> "Client Personnel Requirements"@en.
<http://purl.org/weso/cloudindex/indicator/Installability> <http://www.w3.org/2000/01/rdf-schema#comment> "Installability characterizes the time and effort required to get a service ready for\r\ndelivery (where applicable)."@en.
<http://purl.org/weso/cloudindex/indicator/Installability> <http://www.w3.org/2004/02/skos/core#definition> "Installability characterizes the time and effort required to get a service ready for\r\ndelivery (where applicable)."@en.
<http://purl.org/weso/cloudindex/indicator/Installability> <http://purl.org/weso/cloudindex/ontology/defined-in> <http://csmic.org/wp-content/uploads/2011/09/SMI-Overview-110913_v1F.pdf>.
<http://purl.org/weso/cloudindex/indicator/Installability> <http://purl.org/weso/cloudindex/ontology/defined-by> <http://purl.org/weso/cloudindex/organization/CSMIC>.
<http://purl.org/weso/cloudindex/indicator/Installability> <http://purl.org/weso/cloudindex/ontology/weight> "1.0"^^<http://www.w3.org/2001/XMLSchema#double>.
<http://purl.org/weso/cloudindex/indicator/Installability> <http://purl.org/weso/cloudindex/ontology/pref-value> <http://purl.org/weso/cloudindex/ontology/High>.
<http://purl.org/weso/cloudindex/indicator/Installability> <http://www.w3.org/2004/02/skos/core#notation> "Installability".
<http://purl.org/weso/cloudindex/indicator/Installability> <http://www.w3.org/2006/time#intervalStarts> "2013"^^<http://www.w3.org/2001/XMLSchema#int>.
<http://purl.org/weso/cloudindex/indicator/Installability> <http://www.w3.org/2006/time#intervalFinishes> "2013"^^<http://www.w3.org/2001/XMLSchema#int>.
<http://purl.org/weso/cloudindex/indicator/Installability> <http://www.w3.org/2004/02/skos/core#broader> <http://purl.org/weso/cloudindex/component/Usability>.
<http://purl.org/weso/cloudindex/indicator/Learnability> <http://www.w3.org/1999/02/22-rdf-syntax-ns#type> <http://purl.org/weso/cloudindex/ontology/KPIIndicator>.
<http://purl.org/weso/cloudindex/indicator/Learnability> <http://www.w3.org/2000/01/rdf-schema#label> "Learnability"@en.
<http://purl.org/weso/cloudindex/indicator/Learnability> <http://www.w3.org/2000/01/rdf-schema#comment> "The effort required of users to learn to use the service."@en.
<http://purl.org/weso/cloudindex/indicator/Learnability> <http://www.w3.org/2004/02/skos/core#definition> "The effort required of users to learn to use the service."@en.
<http://purl.org/weso/cloudindex/indicator/Learnability> <http://purl.org/weso/cloudindex/ontology/defined-in> <http://csmic.org/wp-content/uploads/2011/09/SMI-Overview-110913_v1F.pdf>.
<http://purl.org/weso/cloudindex/indicator/Learnability> <http://purl.org/weso/cloudindex/ontology/defined-by> <http://purl.org/weso/cloudindex/organization/CSMIC>.
<http://purl.org/weso/cloudindex/indicator/Learnability> <http://purl.org/weso/cloudindex/ontology/weight> "1.0"^^<http://www.w3.org/2001/XMLSchema#double>.
<http://purl.org/weso/cloudindex/indicator/Learnability> <http://purl.org/weso/cloudindex/ontology/pref-value> <http://purl.org/weso/cloudindex/ontology/High>.
<http://purl.org/weso/cloudindex/indicator/Learnability> <http://www.w3.org/2004/02/skos/core#notation> "Learnability".
<http://purl.org/weso/cloudindex/indicator/Learnability> <http://www.w3.org/2006/time#intervalStarts> "2013"^^<http://www.w3.org/2001/XMLSchema#int>.
<http://purl.org/weso/cloudindex/indicator/Learnability> <http://www.w3.org/2006/time#intervalFinishes> "2013"^^<http://www.w3.org/2001/XMLSchema#int>.
<http://purl.org/weso/cloudindex/indicator/Learnability> <http://www.w3.org/2004/02/skos/core#broader> <http://purl.org/weso/cloudindex/component/Usability>.
<http://purl.org/weso/cloudindex/indicator/Operability> <http://www.w3.org/1999/02/22-rdf-syntax-ns#type> <http://purl.org/weso/cloudindex/ontology/KPIIndicator>.
<http://purl.org/weso/cloudindex/indicator/Operability> <http://www.w3.org/2000/01/rdf-schema#label> "Operability"@en.
<http://purl.org/weso/cloudindex/indicator/Operability> <http://www.w3.org/2000/01/rdf-schema#comment> "The ability of a service to be easily operated by users."@en.
<http://purl.org/weso/cloudindex/indicator/Operability> <http://www.w3.org/2004/02/skos/core#definition> "The ability of a service to be easily operated by users."@en.
<http://purl.org/weso/cloudindex/indicator/Operability> <http://purl.org/weso/cloudindex/ontology/defined-in> <http://csmic.org/wp-content/uploads/2011/09/SMI-Overview-110913_v1F.pdf>.
<http://purl.org/weso/cloudindex/indicator/Operability> <http://purl.org/weso/cloudindex/ontology/defined-by> <http://purl.org/weso/cloudindex/organization/CSMIC>.
<http://purl.org/weso/cloudindex/indicator/Operability> <http://purl.org/weso/cloudindex/ontology/weight> "1.0"^^<http://www.w3.org/2001/XMLSchema#double>.
<http://purl.org/weso/cloudindex/indicator/Operability> <http://purl.org/weso/cloudindex/ontology/pref-value> <http://purl.org/weso/cloudindex/ontology/High>.
<http://purl.org/weso/cloudindex/indicator/Operability> <http://www.w3.org/2004/02/skos/core#notation> "Operability".
<http://purl.org/weso/cloudindex/indicator/Operability> <http://www.w3.org/2006/time#intervalStarts> "2013"^^<http://www.w3.org/2001/XMLSchema#int>.
<http://purl.org/weso/cloudindex/indicator/Operability> <http://www.w3.org/2006/time#intervalFinishes> "2013"^^<http://www.w3.org/2001/XMLSchema#int>.
<http://purl.org/weso/cloudindex/indicator/Operability> <http://www.w3.org/2004/02/skos/core#broader> <http://purl.org/weso/cloudindex/component/Usability>.
<http://purl.org/weso/cloudindex/indicator/Suitability> <http://www.w3.org/1999/02/22-rdf-syntax-ns#type> <http://purl.org/weso/cloudindex/ontology/KPIIndicator>.
<http://purl.org/weso/cloudindex/indicator/Suitability> <http://www.w3.org/2000/01/rdf-schema#label> "Suitability"@en.
<http://purl.org/weso/cloudindex/indicator/Suitability> <http://www.w3.org/2000/01/rdf-schema#comment> "How closely do the capabilities of the service match the needs of the client."@en.
<http://purl.org/weso/cloudindex/indicator/Suitability> <http://www.w3.org/2004/02/skos/core#definition> "How closely do the capabilities of the service match the needs of the client."@en.
<http://purl.org/weso/cloudindex/indicator/Suitability> <http://purl.org/weso/cloudindex/ontology/defined-in> <http://csmic.org/wp-content/uploads/2011/09/SMI-Overview-110913_v1F.pdf>.
<http://purl.org/weso/cloudindex/indicator/Suitability> <http://purl.org/weso/cloudindex/ontology/defined-by> <http://purl.org/weso/cloudindex/organization/CSMIC>.
<http://purl.org/weso/cloudindex/indicator/Suitability> <http://purl.org/weso/cloudindex/ontology/weight> "1.0"^^<http://www.w3.org/2001/XMLSchema#double>.
<http://purl.org/weso/cloudindex/indicator/Suitability> <http://purl.org/weso/cloudindex/ontology/pref-value> <http://purl.org/weso/cloudindex/ontology/High>.
<http://purl.org/weso/cloudindex/indicator/Suitability> <http://www.w3.org/2004/02/skos/core#notation> "Suitability".
<http://purl.org/weso/cloudindex/indicator/Suitability> <http://www.w3.org/2006/time#intervalStarts> "2013"^^<http://www.w3.org/2001/XMLSchema#int>.
<http://purl.org/weso/cloudindex/indicator/Suitability> <http://www.w3.org/2006/time#intervalFinishes> "2013"^^<http://www.w3.org/2001/XMLSchema#int>.
<http://purl.org/weso/cloudindex/indicator/Suitability> <http://www.w3.org/2004/02/skos/core#broader> <http://purl.org/weso/cloudindex/component/Usability>.
<http://purl.org/weso/cloudindex/indicator/Transparency> <http://www.w3.org/1999/02/22-rdf-syntax-ns#type> <http://purl.org/weso/cloudindex/ontology/KPIIndicator>.
<http://purl.org/weso/cloudindex/indicator/Transparency> <http://www.w3.org/2000/01/rdf-schema#label> "Transparency"@en.
<http://purl.org/weso/cloudindex/indicator/Transparency> <http://www.w3.org/2000/01/rdf-schema#comment> "The extent to which users are able to determine when changes in a feature or component of the service occur and whether these changes impact usability."@en.
<http://purl.org/weso/cloudindex/indicator/Transparency> <http://www.w3.org/2004/02/skos/core#definition> "The extent to which users are able to determine when changes in a feature or component of the service occur and whether these changes impact usability."@en.
<http://purl.org/weso/cloudindex/indicator/Transparency> <http://purl.org/weso/cloudindex/ontology/defined-in> <http://csmic.org/wp-content/uploads/2011/09/SMI-Overview-110913_v1F.pdf>.
<http://purl.org/weso/cloudindex/indicator/Transparency> <http://purl.org/weso/cloudindex/ontology/defined-by> <http://purl.org/weso/cloudindex/organization/CSMIC>.
<http://purl.org/weso/cloudindex/indicator/Transparency> <http://purl.org/weso/cloudindex/ontology/weight> "1.0"^^<http://www.w3.org/2001/XMLSchema#double>.
<http://purl.org/weso/cloudindex/indicator/Transparency> <http://purl.org/weso/cloudindex/ontology/pref-value> <http://purl.org/weso/cloudindex/ontology/High>.
<http://purl.org/weso/cloudindex/indicator/Transparency> <http://www.w3.org/2004/02/skos/core#notation> "Transparency".
<http://purl.org/weso/cloudindex/indicator/Transparency> <http://www.w3.org/2006/time#intervalStarts> "2013"^^<http://www.w3.org/2001/XMLSchema#int>.
<http://purl.org/weso/cloudindex/indicator/Transparency> <http://www.w3.org/2006/time#intervalFinishes> "2013"^^<http://www.w3.org/2001/XMLSchema#int>.
<http://purl.org/weso/cloudindex/indicator/Transparency> <http://www.w3.org/2004/02/skos/core#broader> <http://purl.org/weso/cloudindex/component/Usability>.
<http://purl.org/weso/cloudindex/indicator/Understandability> <http://www.w3.org/1999/02/22-rdf-syntax-ns#type> <http://purl.org/weso/cloudindex/ontology/KPIIndicator>.
<http://purl.org/weso/cloudindex/indicator/Understandability> <http://www.w3.org/2000/01/rdf-schema#label> "Understandability"@en.
<http://purl.org/weso/cloudindex/indicator/Understandability> <http://www.w3.org/2000/01/rdf-schema#comment> "The ease with which users can understand the capabilities and operation of the service."@en.
<http://purl.org/weso/cloudindex/indicator/Understandability> <http://www.w3.org/2004/02/skos/core#definition> "The ease with which users can understand the capabilities and operation of the service."@en.
<http://purl.org/weso/cloudindex/indicator/Understandability> <http://purl.org/weso/cloudindex/ontology/defined-in> <http://csmic.org/wp-content/uploads/2011/09/SMI-Overview-110913_v1F.pdf>.
<http://purl.org/weso/cloudindex/indicator/Understandability> <http://purl.org/weso/cloudindex/ontology/defined-by> <http://purl.org/weso/cloudindex/organization/CSMIC>.
<http://purl.org/weso/cloudindex/indicator/Understandability> <http://purl.org/weso/cloudindex/ontology/weight> "1.0"^^<http://www.w3.org/2001/XMLSchema#double>.
<http://purl.org/weso/cloudindex/indicator/Understandability> <http://purl.org/weso/cloudindex/ontology/pref-value> <http://purl.org/weso/cloudindex/ontology/High>.
<http://purl.org/weso/cloudindex/indicator/Understandability> <http://www.w3.org/2004/02/skos/core#notation> "Understandability".
<http://purl.org/weso/cloudindex/indicator/Understandability> <http://www.w3.org/2006/time#intervalStarts> "2013"^^<http://www.w3.org/2001/XMLSchema#int>.
<http://purl.org/weso/cloudindex/indicator/Understandability> <http://www.w3.org/2006/time#intervalFinishes> "2013"^^<http://www.w3.org/2001/XMLSchema#int>.
<http://purl.org/weso/cloudindex/indicator/Understandability> <http://www.w3.org/2004/02/skos/core#broader> <http://purl.org/weso/cloudindex/component/Usability>.
<http://purl.org/weso/cloudindex/organization/ds> <http://www.w3.org/1999/02/22-rdf-syntax-ns#type> <http://rdfs.org/ns/void#Dataset>.
<http://purl.org/weso/cloudindex/organization/ds> <http://www.w3.org/2000/01/rdf-schema#label> "SEERC | Cloud Index | Organizations"@en.
<http://purl.org/weso/cloudindex/organization/ds> <http://purl.org/dc/terms/created> "2012-20-05"^^<http://www.w3.org/2001/XMLSchema#date>.
<http://purl.org/weso/cloudindex/organization/ds> <http://purl.org/dc/terms/modified> "2012-08-31"^^<http://www.w3.org/2001/XMLSchema#date>.
<http://purl.org/weso/cloudindex/organization/ds> <http://purl.org/dc/terms/title> "Organizations dataset involved in the development of Core CloudIndex ontology"@en.
<http://purl.org/weso/cloudindex/organization/ds> <http://purl.org/dc/terms/author> <http://purl.org/weso/cloudindex/people/Chema>.
<http://purl.org/weso/cloudindex/organization/ds> <http://purl.org/dc/terms/author> <http://purl.org/weso/rdfindex/organization/SEERC>.
<http://purl.org/weso/cloudindex/organization/ds> <http://purl.org/dc/terms/publisher> <http://purl.org/weso/cloudindex/people/Chema>.
<http://purl.org/weso/cloudindex/organization/ds> <http://purl.org/dc/terms/contributor> <http://purl.org/weso/rdfindex/organization/SEERC>.
<http://purl.org/weso/cloudindex/organization/ds> <http://purl.org/dc/terms/contributor> <http://purl.org/weso/rdfindex/project/RELATE>.
<http://purl.org/weso/cloudindex/organization/ds> <http://purl.org/dc/terms/license> <http://opendatacommons.org/licenses/by/1.0/>.
<http://purl.org/weso/cloudindex/organization/ds> <http://rdfs.org/ns/void#exampleResource> <http://purl.org/weso/cloudindex/organization/CSMIC>.
<http://purl.org/weso/cloudindex/organization/ds> <http://rdfs.org/ns/void#uriRegexPattern> "http://purl.org/weso/cloudindex/organization/.+".
<http://purl.org/weso/cloudindex/organization/ds> <http://rdfs.org/ns/void#vocabulary> <http://www.w3.org/2000/01/rdf-schema#>.
<http://purl.org/weso/cloudindex/organization/ds> <http://rdfs.org/ns/void#vocabulary> <http://xmlns.com/foaf/0.1/>.
<http://purl.org/weso/cloudindex/organization/ds> <http://xmlns.com/foaf/0.1/homepage> <http://purl.org/weso/cloudindex/>.
<http://purl.org/weso/cloudindex/organization/CSMIC> <http://www.w3.org/1999/02/22-rdf-syntax-ns#type> <http://www.w3.org/ns/org#Organization>.
<http://purl.org/weso/cloudindex/organization/CSMIC> <http://www.w3.org/2000/01/rdf-schema#label> "Service Measurement Index Version 1.0"@en.
<http://purl.org/weso/cloudindex/organization/CSMIC> <http://www.w3.org/2000/01/rdf-schema#comment> "It is a common effort for defining a Service Measurement Index"@en.
<http://purl.org/weso/cloudindex/organization/CSMIC> <http://www.w3.org/ns/org#identifier> "CSMIC".
<http://purl.org/weso/cloudindex/organization/CSMIC> <http://xmlns.com/foaf/0.1/homepage> <http://csmic.org/>.
